<?xml version="1.0" encoding="UTF-8"?>
<rdf:RDF xmlns:rdf="http://www.w3.org/1999/02/22-rdf-syntax-ns#" xmlns:dc="http://purl.org/dc/elements/1.1/" xmlns:skos="http://www.w3.org/2004/02/skos/core#">

<skos:conceptScheme rdf:about="http://rs.gbif.org/terms/dwc/dwc_translations.rdf">
<dc:title>Darwin Core terms translations</dc:title>
<dc:description>This document contains translations of the terms in the Darwin Core glossary expressed using the Simple Knowledge Organisation System (SKOS) data model. 
		Currently four languages are included: English, Spanish, Simplified Chinese and Japanese. </dc:description>
<dc:creator>GBIF</dc:creator>
<dc:created>2012-05-31</dc:created>
<dc:modified>2012-08-17</dc:modified>
<dc:contributor>Arturo Ariño, University of Navarra, Spain</dc:contributor>
<dc:contributor>Juncai Ma, Institute of Microbiology, Chinese Academy of Sciences</dc:contributor>
<dc:contributor>Hiroshi Mori, Tokyo Institute of Technology, Japan</dc:contributor>
<dc:contributor>Francisco Pando, GBIF Spain</dc:contributor>
<dc:contributor>Laura Roldan, Sistema de información sobre biodiversidad de Colombia</dc:contributor>
<dc:contributor>Hideaki Sugawara, National Institute of Genetics, Japan</dc:contributor>
<dc:contributor>William Ulate, Missouri Botanical Garden, USA</dc:contributor>
<dc:contributor>Danny Vélez, Sistema de información sobre biodiversidad de Colombia</dc:contributor>
<dc:contributor>John Wieczorek, University of California Berkeley, USA</dc:contributor>
<dc:contributor>Li Wei, Institute of Microbiology, Chinese Academy of Sciences</dc:contributor>
<dc:contributor>Linhuan Wu, Institute of Microbiology, Chinese Academy of Sciences</dc:contributor>
</skos:conceptScheme>

<skos:Concept rdf:about="http://rs.tdwg.org/dwc/terms/acceptedNameUsage">
<skos:prefLabel xml:lang="en">Accepted Name Usage</skos:prefLabel>
<skos:definition xml:lang="en">The full name, with authorship and
			date information if known, of the currently valid (zoological) or
			accepted (botanical) taxon.</skos:definition>
<skos:example xml:lang="en">Example: "Tamias
			minimus" valid name for
			"Eutamias minimus"</skos:example>
<skos:prefLabel xml:lang="es">Nombre aceptado en uso</skos:prefLabel>
<skos:definition xml:lang="es">El nombre completo, con autoría e
			información de fecha si se conoce, del taxón actualmente válido
			(zoológico) o aceptado (botánico). </skos:definition>
<skos:example xml:lang="es">Ejemplo: "Tamias minimus" nombre válido para
			"Eutamias minimus"</skos:example>
<skos:prefLabel xml:lang="zh-Hans">公认使用名称</skos:prefLabel>
<skos:definition xml:lang="zh-Hans">目前有效（动物学）的或公认（植物学）的分类单元全称，如已知来源和日期信息则需注明。</skos:definition>
<skos:example xml:lang="zh-Hans"/>
<skos:prefLabel xml:lang="ja"/>
<skos:definition xml:lang="ja">もし分かるなら著者と日付情報を付記した、現在妥当なあるいは受け入れられている（動物および植物学的な）分類群のフルネーム。</skos:definition>
<skos:example xml:lang="ja">例: "Tamias minimus" は"Eutamias
			minimus"の有効な名前である</skos:example>
<skos:inScheme rdf:resource="http://rs.gbif.org/terms/dwc/dwc_translations.rdf"/>
<rdf:type rdf:resource="http://www.w3.org/1999/02/22-rdf-syntax-ns#Property"/>
</skos:Concept>

<skos:Concept rdf:about="http://rs.tdwg.org/dwc/terms/acceptedNameUsageID">
<skos:prefLabel xml:lang="en">Accepted Name Usage ID</skos:prefLabel>
<skos:definition xml:lang="en">An identifier for the name usage
			(documented meaning of the name according to a source) of the
			currently valid (zoological) or accepted (botanical) taxon.
		</skos:definition>
<skos:example xml:lang="en">Example:
			"8fa58e08-08de-4ac1-b69c-1235340b7001"</skos:example>
<skos:prefLabel xml:lang="es">Nombre aceptado en uso - ID</skos:prefLabel>
<skos:definition xml:lang="es">Un identificador para el nombre en uso
			(significado del nombre, documentado de acuerdo con alguna fuente)
			del taxón actualmente válido (zoológico) o aceptado (botánico).   </skos:definition>
<skos:example xml:lang="es">Ejemplo:
			"8fa58e08-08de-4ac1-b69c-1235340b7001"</skos:example>
<skos:prefLabel xml:lang="zh-Hans">公认使用名称编号</skos:prefLabel>
<skos:definition xml:lang="zh-Hans">目前有效（动物学）的或公认（植物学）的分类单元的名称使用（根据来源所取名称的存档记录方法）标识符。</skos:definition>
<skos:example xml:lang="zh-Hans"/>
<skos:prefLabel xml:lang="ja"/>
<skos:definition xml:lang="ja">現在妥当なあるいは受け入れられている（動物および植物学的な）分類群の名前の使用法（情報源に従った名前に関する、文書化された意味）のID。</skos:definition>
<skos:example xml:lang="ja"/>
<skos:inScheme rdf:resource="http://rs.gbif.org/terms/dwc/dwc_translations.rdf"/>
<rdf:type rdf:resource="http://www.w3.org/1999/02/22-rdf-syntax-ns#Property"/>
</skos:Concept>

<skos:Concept rdf:about="http://rs.tdwg.org/dwc/terms/accordingTo">
<skos:prefLabel xml:lang="en">According To</skos:prefLabel>
<skos:definition xml:lang="en">Abstract term to attribute
			information
			to a source.</skos:definition>
<skos:example xml:lang="en"/>
<skos:inScheme rdf:resource="http://rs.gbif.org/terms/dwc/dwc_translations.rdf"/>
<rdf:type rdf:resource="http://www.w3.org/1999/02/22-rdf-syntax-ns#Property"/>
</skos:Concept>
<skos:Concept rdf:about="http://rs.tdwg.org/dwc/terms/associatedMedia">
<skos:prefLabel xml:lang="en">Associated Media</skos:prefLabel>
<skos:definition xml:lang="en">A list (concatenated and
			separated) of
			identifiers (publication, global unique identifier,
			URI) of media
			associated with the Occurrence.</skos:definition>
<skos:example xml:lang="en">Example:
			"http://arctos.database.museum/SpecimenImages/UAMObs/Mamm/2/P7291179.JPG"
		</skos:example>
<skos:prefLabel xml:lang="es">Medios asociados</skos:prefLabel>
<skos:definition xml:lang="es">Una lista (concatenada o delimitada)
			de identificadores (publicación, identificador único global, URI) de
			los medios asociados con el registro biológico.</skos:definition>
<skos:example xml:lang="es">Ejemplo:
			"http://arctos.database.museum/SpecimenImages/UAMObs/Mamm/2/P7291179.JPG"</skos:example>
<skos:prefLabel xml:lang="zh-Hans">相关媒介</skos:prefLabel>
<skos:definition xml:lang="zh-Hans">发现媒介的（发表、全局唯一标识符、统一资源标识符等）标识符之（连接的或分开的）列表。</skos:definition>
<skos:example xml:lang="zh-Hans"/>
<skos:prefLabel xml:lang="ja"/>
<skos:definition xml:lang="ja">関連するメディアのID（出版物、GUID、URIなど）のリスト。</skos:definition>
<skos:example xml:lang="ja"/>
<skos:inScheme rdf:resource="http://rs.gbif.org/terms/dwc/dwc_translations.rdf"/>
<rdf:type rdf:resource="http://www.w3.org/1999/02/22-rdf-syntax-ns#Property"/>
</skos:Concept>
<skos:Concept rdf:about="http://rs.tdwg.org/dwc/terms/associatedOccurrences">
<skos:prefLabel xml:lang="en">Associated Occurrences</skos:prefLabel>
<skos:definition xml:lang="en">A list (concatenated and
			separated) of
			identifiers of other Occurrence records and their
			associations to this
			Occurrence.</skos:definition>
<skos:example xml:lang="en">Example: "sibling of
			FMNH:Mammal:1234;
			sibling of FMNH:Mammal:1235"</skos:example>
<skos:prefLabel xml:lang="es"> Registros biológicos asociados</skos:prefLabel>
<skos:definition xml:lang="es">Una lista (concatenada y separada) de
			los identificadores de otros registros biológicos y su relación con
			este Registro Biológico. </skos:definition>
<skos:example xml:lang="es">Ejemplo: "hermano de
			FMNH:Mamífero:1234;hermano de FMNH:Mamífero:1235"</skos:example>
<skos:prefLabel xml:lang="zh-Hans">相关事件</skos:prefLabel>
<skos:definition xml:lang="zh-Hans">其他发现记录及其与发现信息相关联的标识符之（连接的或分开的）列表。</skos:definition>
<skos:example xml:lang="zh-Hans"/>
<skos:prefLabel xml:lang="ja"/>
<skos:definition xml:lang="ja">関連する他のレコードのIDおよびその関連性のリスト。</skos:definition>
<skos:example xml:lang="ja"/>
<skos:inScheme rdf:resource="http://rs.gbif.org/terms/dwc/dwc_translations.rdf"/>
<rdf:type rdf:resource="http://www.w3.org/1999/02/22-rdf-syntax-ns#Property"/>
</skos:Concept>
<skos:Concept rdf:about="http://rs.tdwg.org/dwc/terms/associatedReferences">
<skos:prefLabel xml:lang="en">Associated References</skos:prefLabel>
<skos:definition xml:lang="en">A list (concatenated and
			separated) of
			identifiers (publication, bibliographic reference,
			global unique
			identifier, URI) of literature associated with the
			Occurrence.</skos:definition>
<skos:example xml:lang="en">Examples:
			"http://www.sciencemag.org/cgi/content/abstract/322/5899/261",
			"Christopher J. Conroy, Jennifer L. Neuwald. 2008. Phylogeographic
			study of the California vole, Microtus californicus Journal of
			Mammalogy, 89(3):755-767."</skos:example>
<skos:prefLabel xml:lang="es">Referencias asociadas</skos:prefLabel>
<skos:definition xml:lang="es">Una lista (concatenada y separada) de
			los identificadores (publicación, referencia bibliográfica,
			identificador único global, URI) de la literatura asociada con el
			Registro Biológico. </skos:definition>
<skos:example xml:lang="es">Ejemplo:
			"http://www.sciencemag.org/cgi/content/abstract/322/5899/261",
			"Christopher J. Conroy, Jennifer L. Neuwald. 2008. Phylogeographic
			study of the California vole, Microtus californicus Journal of
			Mammalogy, 89(3):755-767."</skos:example>
<skos:prefLabel xml:lang="zh-Hans">相关参考</skos:prefLabel>
<skos:definition xml:lang="zh-Hans">与发现情况相关之文献的（发表、参考文献、全局唯一标识符、统一资源标识符等）标识符之（连接的或分开的）列表。</skos:definition>
<skos:example xml:lang="zh-Hans"/>
<skos:prefLabel xml:lang="ja"/>
<skos:definition xml:lang="ja">関連する文献のID（出版物、参考文献、GUID、URIなど）のリスト。</skos:definition>
<skos:example xml:lang="ja"/>
<skos:inScheme rdf:resource="http://rs.gbif.org/terms/dwc/dwc_translations.rdf"/>
<rdf:type rdf:resource="http://www.w3.org/1999/02/22-rdf-syntax-ns#Property"/>
</skos:Concept>
<skos:Concept rdf:about="http://rs.tdwg.org/dwc/terms/associatedSequences">
<skos:prefLabel xml:lang="en">Associated Sequences</skos:prefLabel>
<skos:definition xml:lang="en">A list (concatenated and
			separated) of
			identifiers (publication, global unique identifier,
			URI) of genetic
			sequence information associated with the Occurrence.
		</skos:definition>
<skos:example xml:lang="en">Example: "GenBank:
			U34853.1"</skos:example>
<skos:prefLabel xml:lang="es">Secuencias asociadas</skos:prefLabel>
<skos:definition xml:lang="es">Una lista (concatenada y separada) de
			los identificadores (publicación, identificador único global, URI) de
			la información de la secuencia genética asociada con el Registro
			Biológico. </skos:definition>
<skos:example xml:lang="es">Ejemplo: "Banco de Genes: U34853.1"</skos:example>
<skos:prefLabel xml:lang="zh-Hans">相关序列</skos:prefLabel>
<skos:definition xml:lang="zh-Hans">与发现情况相关之基因序列信息的（发表、全局唯一标识符、统一资源标识符等）标识符之（连接的或分开的）列表。</skos:definition>
<skos:example xml:lang="zh-Hans"/>
<skos:prefLabel xml:lang="ja"/>
<skos:definition xml:lang="ja">関連する配列情報のID（出版物、GUID、URIなど）のリスト。</skos:definition>
<skos:example xml:lang="ja"/>
<skos:inScheme rdf:resource="http://rs.gbif.org/terms/dwc/dwc_translations.rdf"/>
<rdf:type rdf:resource="http://www.w3.org/1999/02/22-rdf-syntax-ns#Property"/>
</skos:Concept>
<skos:Concept rdf:about="http://rs.tdwg.org/dwc/terms/associatedTaxa">
<skos:prefLabel xml:lang="en">Associated Taxa</skos:prefLabel>
<skos:definition xml:lang="en">A list (concatenated and
			separated) of
			identifiers or names of taxa and their associations
			with the
			Occurrence.</skos:definition>
<skos:example xml:lang="en">Example: "host:
			Quercus alba"</skos:example>
<skos:prefLabel xml:lang="es">Taxones asociados</skos:prefLabel>
<skos:definition xml:lang="es">Una lista (concatenada y separada) de
			los identificadores o nombres de taxones y su asociación con el
			Registro Biológico.</skos:definition>
<skos:example xml:lang="es">Ejemplo: "huésped: Quercus alba"</skos:example>
<skos:prefLabel xml:lang="zh-Hans">相关类群</skos:prefLabel>
<skos:definition xml:lang="zh-Hans">与发现情况相关的标识符或分类单元名称之（连接的或分开的）列表。</skos:definition>
<skos:example xml:lang="zh-Hans"/>
<skos:prefLabel xml:lang="ja"/>
<skos:definition xml:lang="ja">関連する分類群の名前またはID、およびその関連性のリスト。</skos:definition>
<skos:example xml:lang="ja"/>
<skos:inScheme rdf:resource="http://rs.gbif.org/terms/dwc/dwc_translations.rdf"/>
<rdf:type rdf:resource="http://www.w3.org/1999/02/22-rdf-syntax-ns#Property"/>
</skos:Concept>
<skos:Concept rdf:about="http://rs.tdwg.org/dwc/terms/basisOfRecord">
<skos:prefLabel xml:lang="en">Basis of Record</skos:prefLabel>
<skos:definition xml:lang="en">The specific nature of the data
			record
			- a subtype of the dcterms:type. Recommended best practice is
			to use a
			controlled vocabulary such as the Darwin Core Type
			Vocabulary
			(http://rs.tdwg.org/dwc/terms/type-vocabulary/index.htm).
		</skos:definition>
<skos:example xml:lang="en">Examples:
			"PreservedSpecimen",
			"FossilSpecimen", "LivingSpecimen",
			"HumanObservation",
			"MachineObservation"</skos:example>
<skos:prefLabel xml:lang="es">Base del registro</skos:prefLabel>
<skos:definition xml:lang="es">La naturaleza específica del registro
			de datos - un subtipo de Tipo. La práctica recomendada es el uso de
			lenguaje controlado como el vocabulario controlado para Tipo de
			Darwin Core (http://rs.tdwg.org/dwc/terms/type-vocabulary/index.htm). </skos:definition>
<skos:example xml:lang="es">Ejemplo: "Espécimen Preservado", "Espécimen
			Fósil", "Espécimen Vivo", "Observación Humana"</skos:example>
<skos:prefLabel xml:lang="zh-Hans">记录基础</skos:prefLabel>
<skos:definition xml:lang="zh-Hans">数据记录的特有属性——dcterms:type的子类。建议最好使用控制性词汇，如达尔文核心类型词汇（http://rs.tdwg.org/dwc/terms/type-vocabulary/index.htm）。</skos:definition>
<skos:example xml:lang="zh-Hans"/>
<skos:prefLabel xml:lang="ja"/>
<skos:definition xml:lang="ja">レコード情報の具体的内容（dcterms:typeのsubtype）。the
			Darwin Core Type Vocabulary
			(http://rs.tdwg.org/dwc/terms/type-vocabulary/index.htm)など、管理された語彙の使用を推奨。</skos:definition>
<skos:example xml:lang="ja"/>
<skos:inScheme rdf:resource="http://rs.gbif.org/terms/dwc/dwc_translations.rdf"/>
<rdf:type rdf:resource="http://www.w3.org/1999/02/22-rdf-syntax-ns#Property"/>
</skos:Concept>
<skos:Concept rdf:about="http://rs.tdwg.org/dwc/terms/bed">
<skos:prefLabel xml:lang="en">Bed</skos:prefLabel>
<skos:definition xml:lang="en">The full name of the
			lithostratigraphic bed from which the cataloged item was collected.
		</skos:definition>
<skos:example xml:lang="en"/>
<skos:prefLabel xml:lang="es">Capa</skos:prefLabel>
<skos:definition xml:lang="es">El nombre completo de la capa
			litoestratigráfica de la cual se colectó el elemento catalogado. </skos:definition>
<skos:example xml:lang="es"/>
<skos:prefLabel xml:lang="zh-Hans">岩床</skos:prefLabel>
<skos:definition xml:lang="zh-Hans">采集收录对象的岩床的全称。</skos:definition>
<skos:example xml:lang="zh-Hans"/>
<skos:prefLabel xml:lang="ja"/>
<skos:definition xml:lang="ja">この資料が収集された岩相層序層のフルネーム。</skos:definition>
<skos:example xml:lang="ja"/>
<skos:inScheme rdf:resource="http://rs.gbif.org/terms/dwc/dwc_translations.rdf"/>
<rdf:type rdf:resource="http://www.w3.org/1999/02/22-rdf-syntax-ns#Property"/>
</skos:Concept>
<skos:Concept rdf:about="http://rs.tdwg.org/dwc/terms/behavior">
<skos:prefLabel xml:lang="en">Behavior</skos:prefLabel>
<skos:definition xml:lang="en">A description of the behavior
			shown by
			the subject at the time the Occurrence was recorded.
			Recommended best
			practice is to use a controlled vocabulary.
		</skos:definition>
<skos:example xml:lang="en">Examples:
			"roosting", "foraging", "running"</skos:example>
<skos:prefLabel xml:lang="es">Comportamiento</skos:prefLabel>
<skos:definition xml:lang="es">Una descripción de la conducta
			mostrada por el sujeto en el momento del Registro Biológico. La
			práctica recomendada es el uso de un lenguaje controlado.</skos:definition>
<skos:example xml:lang="es">Ejemplo: "posando", "alimentándose",
			"corriendo"</skos:example>
<skos:prefLabel xml:lang="zh-Hans">行为</skos:prefLabel>
<skos:definition xml:lang="zh-Hans">对记录发现过程中目标行为的描述。建议最好使用控制性词汇。</skos:definition>
<skos:example xml:lang="zh-Hans"/>
<skos:prefLabel xml:lang="ja"/>
<skos:definition xml:lang="ja">記録時に対象が示した行動の記述。管理された語彙の使用を推奨。</skos:definition>
<skos:example xml:lang="ja"/>
<skos:inScheme rdf:resource="http://rs.gbif.org/terms/dwc/dwc_translations.rdf"/>
<rdf:type rdf:resource="http://www.w3.org/1999/02/22-rdf-syntax-ns#Property"/>
</skos:Concept>
<skos:Concept rdf:about="http://rs.tdwg.org/dwc/terms/catalogNumber">
<skos:prefLabel xml:lang="en">Catalog Number</skos:prefLabel>
<skos:definition xml:lang="en">An identifier (preferably unique)
			for
			the record within the data set or collection.</skos:definition>
<skos:example xml:lang="en">Examples:
			"2008.1334", "145732a", "145732"</skos:example>
<skos:prefLabel xml:lang="es">Número de catálogo</skos:prefLabel>
<skos:definition xml:lang="es">Un identificador (preferiblemente
			único) para el registro dentro del conjunto de datos o colección. </skos:definition>
<skos:example xml:lang="es">Ejemplos: "2008.1334", "145732a", "145732"</skos:example>
<skos:prefLabel xml:lang="zh-Hans">目录编号</skos:prefLabel>
<skos:definition xml:lang="zh-Hans">数据集或保藏信息中的记录标识符（最好是唯一的）。</skos:definition>
<skos:example xml:lang="zh-Hans"/>
<skos:prefLabel xml:lang="ja"/>
<skos:definition xml:lang="ja">データセット内のレコードについてのID（一意的なものが望ましい）。</skos:definition>
<skos:example xml:lang="ja"/>
<skos:inScheme rdf:resource="http://rs.gbif.org/terms/dwc/dwc_translations.rdf"/>
<rdf:type rdf:resource="http://www.w3.org/1999/02/22-rdf-syntax-ns#Property"/>
</skos:Concept>
<skos:Concept rdf:about="http://rs.tdwg.org/dwc/terms/class">
<skos:prefLabel xml:lang="en">Class</skos:prefLabel>
<skos:definition xml:lang="en">The full scientific name of the
			class
			in which the taxon is classified.</skos:definition>
<skos:example xml:lang="en">Example: "Mammalia",
			"Hepaticopsida"</skos:example>
<skos:prefLabel xml:lang="es">Clase</skos:prefLabel>
<skos:definition xml:lang="es">El nombre científico completo de la
			clase en la que se clasifica el taxón.</skos:definition>
<skos:example xml:lang="es">Ejemplo: "Mammalia", "Hepaticopsida"</skos:example>
<skos:prefLabel xml:lang="zh-Hans">纲</skos:prefLabel>
<skos:definition xml:lang="zh-Hans">分类单元所属纲的完整学名。</skos:definition>
<skos:example xml:lang="zh-Hans"/>
<skos:prefLabel xml:lang="ja"/>
<skos:definition xml:lang="ja">その分類群が位置づけられている、分類上の「綱」のフルネーム。</skos:definition>
<skos:example xml:lang="ja"/>
<skos:inScheme rdf:resource="http://rs.gbif.org/terms/dwc/dwc_translations.rdf"/>
<rdf:type rdf:resource="http://www.w3.org/1999/02/22-rdf-syntax-ns#Property"/>
</skos:Concept>
<skos:Concept rdf:about="http://rs.tdwg.org/dwc/terms/collectionCode">
<skos:prefLabel xml:lang="en">Collection Code</skos:prefLabel>
<skos:definition xml:lang="en">The name, acronym, coden, or
			initialism identifying the collection or data set from which the
			record was derived.</skos:definition>
<skos:example xml:lang="en">Examples: "Mammals",
			"Hildebrandt", "eBird"</skos:example>
<skos:prefLabel xml:lang="es">Código de la colección</skos:prefLabel>
<skos:definition xml:lang="es">El nombre, acrónimo, coden, o
			iniciales que identifican la colección o conjunto de datos del que
			procede el registro. </skos:definition>
<skos:example xml:lang="es">Ejemplo: "Mammals", "Hildebrandt", "eBird"</skos:example>
<skos:prefLabel xml:lang="zh-Hans">保藏代码</skos:prefLabel>
<skos:definition xml:lang="zh-Hans">标识生成记录的保藏信息或数据集的名称、首字母缩略词、分类编号或词起首字母</skos:definition>
<skos:example xml:lang="zh-Hans"/>
<skos:prefLabel xml:lang="ja"/>
<skos:definition xml:lang="ja">そのレコードが由来しているデータセットを特定する名前、頭字語、あるいはイニシャル。</skos:definition>
<skos:example xml:lang="ja"/>
<skos:inScheme rdf:resource="http://rs.gbif.org/terms/dwc/dwc_translations.rdf"/>
<rdf:type rdf:resource="http://www.w3.org/1999/02/22-rdf-syntax-ns#Property"/>
</skos:Concept>
<skos:Concept rdf:about="http://rs.tdwg.org/dwc/terms/collectionID">
<skos:prefLabel xml:lang="en">Collection ID</skos:prefLabel>
<skos:definition xml:lang="en">An identifier for the collection
			or
			dataset from which the record was derived. For physical specimens,
			the recommended best practice is to use the identifier in a
			collections registry such as the Biodiversity Collections Index
			(http://www.biodiversitycollectionsindex.org/).</skos:definition>
<skos:example xml:lang="en">Example:
			"urn:lsid:biocol.org:col:34818"</skos:example>
<skos:prefLabel xml:lang="es">ID de la colección</skos:prefLabel>
<skos:definition xml:lang="es">Un identificador de la colección o
			conjunto de datos del que procede el registro. Para especímenes
			físicos, la práctica recomendada es utilizar el identificador de un
			índice de colección tal como el Índice de Colecciones de
			Biodiversidad (http://www.biodiversitycollectionsindex.org/).</skos:definition>
<skos:example xml:lang="es">Ejemplo: "urn:lsid:biocol.org:col:34818"</skos:example>
<skos:prefLabel xml:lang="zh-Hans">保藏编号</skos:prefLabel>
<skos:definition xml:lang="zh-Hans">生成记录的保藏信息或数据集的标识符。针对实体标本，建议最好使用保藏注册标识符，如生物多样性保藏索引(http://www.biodiversitycollectionsindex.org/)。</skos:definition>
<skos:example xml:lang="zh-Hans"/>
<skos:prefLabel xml:lang="ja"/>
<skos:definition xml:lang="ja">その資料が由来したデータセットまたはコレクションのID。物質的な資料の場合、Biodiversity
			Collections Index
			(http://www.biodiversitycollectionsindex.org/)のようなコレクションレポジトリのIDの使用を推奨。</skos:definition>
<skos:example xml:lang="ja"/>
<skos:inScheme rdf:resource="http://rs.gbif.org/terms/dwc/dwc_translations.rdf"/>
<rdf:type rdf:resource="http://www.w3.org/1999/02/22-rdf-syntax-ns#Property"/>
</skos:Concept>
<skos:Concept rdf:about="http://rs.tdwg.org/dwc/terms/continent">
<skos:prefLabel xml:lang="en">Continent</skos:prefLabel>
<skos:definition xml:lang="en">The name of the continent in which
			the
			Location occurs. Recommended best practice is to use a controlled
			vocabulary such as the Getty Thesaurus of Geographic Names or the ISO
			3166 Continent code.</skos:definition>
<skos:example xml:lang="en">Example:
			"Antarctica"</skos:example>
<skos:prefLabel xml:lang="es">Continente</skos:prefLabel>
<skos:definition xml:lang="es">El nombre del continente en el que la
			ubicación ocurre. La práctica recomendada es el uso de un lenguaje
			controlado, como la norma ISO 3166 de códigos de Continente. </skos:definition>
<skos:example xml:lang="es">Ejemplo: "Antártida"</skos:example>
<skos:prefLabel xml:lang="zh-Hans">洲</skos:prefLabel>
<skos:definition xml:lang="zh-Hans">发现地点所在的大洲名。建议最好使用控制性词汇，如盖提地理名称索引典或国际标准化组织3166洲代码。</skos:definition>
<skos:example xml:lang="zh-Hans"/>
<skos:prefLabel xml:lang="ja"/>
<skos:definition xml:lang="ja">その場所が存在する大陸名。the Getty Thesaurus of
			Geographic Names あるいは ISO 3166 Continent
			code などの管理された語彙の使用を推奨。</skos:definition>
<skos:example xml:lang="ja"/>
<skos:inScheme rdf:resource="http://rs.gbif.org/terms/dwc/dwc_translations.rdf"/>
<rdf:type rdf:resource="http://www.w3.org/1999/02/22-rdf-syntax-ns#Property"/>
</skos:Concept>
<skos:Concept rdf:about="http://rs.tdwg.org/dwc/terms/coordinatePrecision">
<skos:prefLabel xml:lang="en">Coordinate Precision</skos:prefLabel>
<skos:definition xml:lang="en">A decimal representation of the
			precision of the coordinates given in the decimalLatitude and
			decimalLongitude.</skos:definition>
<skos:example xml:lang="en">Examples: "0.00001"
			(normal GPS limit for
			decimal degrees), "0.000278" (nearest second),
			"0.01667" (nearest
			minute), "1.0" (nearest degree)
		</skos:example>
<skos:prefLabel xml:lang="es">Precisión de las coordenadas</skos:prefLabel>
<skos:definition xml:lang="es">Una representación decimal de la
			precisión de las coordenadas provistas en Latitud Decimal y Longitud
			Decimal. </skos:definition>
<skos:example xml:lang="es">Ejemplo: "0.00001" (límite normal de GPS
			para grados decimales), "0.000278" (segundo más próximo), "0.01667"
			(minuto más próximo), "1.0" (grado más próximo)</skos:example>
<skos:prefLabel xml:lang="zh-Hans">坐标精度</skos:prefLabel>
<skos:definition xml:lang="zh-Hans">精确到小数的纬度和经度坐标的小数示数。</skos:definition>
<skos:example xml:lang="zh-Hans"/>
<skos:prefLabel xml:lang="ja"/>
<skos:definition xml:lang="ja">小数点表現の緯度および経度で与えられる座標の精度に関する小数点表現。</skos:definition>
<skos:example xml:lang="ja">例: "0.00001"(通常のGPSの小数点表現の限界)。 "0.000278"
			(最も近い秒), "0.01667" (最も近い分), "1.0"
			(最も近い度)</skos:example>
<skos:inScheme rdf:resource="http://rs.gbif.org/terms/dwc/dwc_translations.rdf"/>
<rdf:type rdf:resource="http://www.w3.org/1999/02/22-rdf-syntax-ns#Property"/>
</skos:Concept>
<skos:Concept rdf:about="http://rs.tdwg.org/dwc/terms/coordinateUncertaintyInMeters">
<skos:prefLabel xml:lang="en">Coordinate Uncertainty In Meters
		</skos:prefLabel>
<skos:definition xml:lang="en">The horizontal distance (in
			meters)
			from the given decimalLatitude and decimalLongitude
			describing the
			smallest circle containing the whole of the Location.
			Leave the value
			empty if the uncertainty is unknown, cannot be
			estimated, or is not
			applicable (because there are no coordinates).
			Zero is not a valid
			value for this term.</skos:definition>
<skos:example xml:lang="en">Example: "30"
			(reasonable lower limit of a
			GPS reading under good conditions if the
			actual precision was not
			recorded at the time), "71" (uncertainty for
			a UTM coordinate having
			100 meter precision and a known spatial
			reference system).</skos:example>
<skos:prefLabel xml:lang="es"> Incertidumbre de las coordenadas en metros</skos:prefLabel>
<skos:definition xml:lang="es">La distancia horizontal (en metros) de
			la Latitud Decimal y Longitud Decimal provistas describiendo el
			círculo más pequeño que contiene la totalidad de la ubicación. Deje
			el valor vacío si la incertidumbre es desconocida, no se puede
			estimar, o no es aplicable (porque no hay coordenadas). Cero no es un
			valor válido para este elemento. </skos:definition>
<skos:example xml:lang="es">Ejemplo: "30" (límite inferior razonable de
			la lectura de GPS bajo buenas condiciones si la precisión actual no
			fue registrada en el momento), "71" (incertidumbre para una
			coordenada UTM con 100 metros de precisión y un sistema de referencia
			espacial conocido).</skos:example>
<skos:prefLabel xml:lang="zh-Hans">坐标不确定性（以米为单位）</skos:prefLabel>
<skos:definition xml:lang="zh-Hans">到涵盖整个地点的最小圆形区域的小数纬度和经度的水平距离（以“米”为单位）。若未知、无法估算或不适用（由于没有坐标），则值为空。此项中0不是有效值。</skos:definition>
<skos:example xml:lang="zh-Hans"/>
<skos:prefLabel xml:lang="ja"/>
<skos:definition xml:lang="ja">小数点表現の緯度および経度で与えられる座標から実際の場所への距離(m)。誤差がよくわからない場合には、空欄にする。この欄に0とだけ入力することは許されていない。</skos:definition>
<skos:example xml:lang="ja">例: "30"
			(実際の誤差が記録されていない場合に使える、条件が良い場合にGPSで得られる場合の誤差の最小値), "71" (100
			mの精度を持つUTM座標系や空間参照システムにおける誤差)</skos:example>
<skos:inScheme rdf:resource="http://rs.gbif.org/terms/dwc/dwc_translations.rdf"/>
<rdf:type rdf:resource="http://www.w3.org/1999/02/22-rdf-syntax-ns#Property"/>
</skos:Concept>
<skos:Concept rdf:about="http://rs.tdwg.org/dwc/terms/country">
<skos:prefLabel xml:lang="en">Country</skos:prefLabel>
<skos:definition xml:lang="en">The name of the country or major
			administrative unit in which the Location occurs. Recommended best
			practice is to use a controlled vocabulary such as the Getty
			Thesaurus of Geographic Names.</skos:definition>
<skos:example xml:lang="en">Examples: "Denmark",
			"Colombia", "España"</skos:example>
<skos:prefLabel xml:lang="es">País</skos:prefLabel>
<skos:definition xml:lang="es">El nombre del país o unidad
			administrativa de mayor jerarquía de la ubicación. La práctica
			recomendada es utilizar un identificador persistente de un lenguaje
			controlado como el Tesauro Getty de Nombres Geográficos. </skos:definition>
<skos:example xml:lang="es">Ejemplo: "Denmark", "Colombia", "España"</skos:example>
<skos:prefLabel xml:lang="zh-Hans">国家</skos:prefLabel>
<skos:definition xml:lang="zh-Hans">发现地点的国家或主要行政区划名称。建议最好使用控制性词汇，如盖提地理名称索引。</skos:definition>
<skos:example xml:lang="zh-Hans"/>
<skos:prefLabel xml:lang="ja"/>
<skos:definition xml:lang="ja">その位置が存在する国名、あるいは主要な行政単位。the Getty
			Thesaurus of Geographic
			Names などの管理された語彙の使用を推奨。</skos:definition>
<skos:example xml:lang="ja"/>
<skos:inScheme rdf:resource="http://rs.gbif.org/terms/dwc/dwc_translations.rdf"/>
<rdf:type rdf:resource="http://www.w3.org/1999/02/22-rdf-syntax-ns#Property"/>
</skos:Concept>
<skos:Concept rdf:about="http://rs.tdwg.org/dwc/terms/countryCode">
<skos:prefLabel xml:lang="en">Country Code</skos:prefLabel>
<skos:definition xml:lang="en">The standard code for the country
			in
			which the Location occurs. Recommended best practice is to use ISO
			3166-1-alpha-2 country codes.</skos:definition>
<skos:example xml:lang="en">Examples: "AR" for
			Argentina, "SV" for El
			Salvador</skos:example>
<skos:prefLabel xml:lang="es">Código del país</skos:prefLabel>
<skos:definition xml:lang="es">El código estándar para el país de la
			ubicación. La práctica recomendada es el uso de ISO 3166-1-alfa-2 de
			códigos de países. </skos:definition>
<skos:example xml:lang="es">Ejemplo: "AR" para Argentina, "SV" para El
			Salvador</skos:example>
<skos:prefLabel xml:lang="zh-Hans">国家代码</skos:prefLabel>
<skos:definition xml:lang="zh-Hans">发现地点的标准国家代码。建议最好使用国际标准化组织3166-1-阿尔法-2国家代码。</skos:definition>
<skos:example xml:lang="zh-Hans"/>
<skos:prefLabel xml:lang="ja"/>
<skos:definition xml:lang="ja">その位置が存在する国の標準コード。ISO 3166-1-alpha-2
			country codes の使用を推奨。</skos:definition>
<skos:example xml:lang="ja">例: アルゼンチンの場合は"AR", エルサルバドルの場合は"SV"</skos:example>
<skos:inScheme rdf:resource="http://rs.gbif.org/terms/dwc/dwc_translations.rdf"/>
<rdf:type rdf:resource="http://www.w3.org/1999/02/22-rdf-syntax-ns#Property"/>
</skos:Concept>
<skos:Concept rdf:about="http://rs.tdwg.org/dwc/terms/county">
<skos:prefLabel xml:lang="en">County</skos:prefLabel>
<skos:definition xml:lang="en">The full, unabbreviated name of
			the
			next smaller administrative region than stateProvince (county,
			shire,
			department, etc.) in which the Location occurs.</skos:definition>
<skos:example xml:lang="en">Examples:
			"Missoula", "Los Lagos", "Mataró"</skos:example>
<skos:prefLabel xml:lang="es">Condado</skos:prefLabel>
<skos:definition xml:lang="es">El nombre completo, sin abreviar de la
			siguiente región administrativa de menor jerarquía que Estado
			Provincia (condado, departamento, etc.) de la ubicación.</skos:definition>
<skos:example xml:lang="es">Ejemplo: "Missoula", "Los Lagos", "Mataró"</skos:example>
<skos:prefLabel xml:lang="zh-Hans">郡/县</skos:prefLabel>
<skos:definition xml:lang="zh-Hans">发现地点所在的除州/省之外的次一级行政区划（县、郡、行政区等）。</skos:definition>
<skos:example xml:lang="zh-Hans"/>
<skos:prefLabel xml:lang="ja"/>
<skos:definition xml:lang="ja">その位置が存在する、州より下位の行政区分（郡、県など）の省略されていないフルネーム。</skos:definition>
<skos:example xml:lang="ja"/>
<skos:inScheme rdf:resource="http://rs.gbif.org/terms/dwc/dwc_translations.rdf"/>
<rdf:type rdf:resource="http://www.w3.org/1999/02/22-rdf-syntax-ns#Property"/>
</skos:Concept>
<skos:Concept rdf:about="http://rs.tdwg.org/dwc/terms/dataGeneralizations">
<skos:prefLabel xml:lang="en">Data Generalizations</skos:prefLabel>
<skos:definition xml:lang="en">Actions taken to make the shared
			data
			less specific or complete than in its original form. Suggests
			that
			alternative data of higher quality may be available on request.
		</skos:definition>
<skos:example xml:lang="en">Example:
			"Coordinates generalized from
			original GPS coordinates to the nearest
			half degree grid cell"</skos:example>
<skos:prefLabel xml:lang="es">Generalización de los datos</skos:prefLabel>
<skos:definition xml:lang="es">Las medidas adoptadas para que los
			datos compartidos sean menos específicos o completos que en su forma
			original. Sugiere que datos alternativos de mayor calidad pueden
			estar disponibles bajo petición.</skos:definition>
<skos:example xml:lang="es">Ejemplo: "Coordenadas generalizadas a partir
			de las coordenadas originales del GPS a la celda más cercana de la
			grilla"</skos:example>
<skos:prefLabel xml:lang="zh-Hans">数据概括</skos:prefLabel>
<skos:definition xml:lang="zh-Hans">为使共享数据较之其原始形式不那么精确或完整所采取的行动。建议以更高质量的替代数据备索。</skos:definition>
<skos:example xml:lang="zh-Hans"/>
<skos:prefLabel xml:lang="ja"/>
<skos:definition xml:lang="ja">元々のフォームよりも一般的または完全にするためのデータ共有の仕組み。要求すれば代わりとなる高精度なデータが得られる可能性がある。</skos:definition>
<skos:example xml:lang="ja"/>
<skos:inScheme rdf:resource="http://rs.gbif.org/terms/dwc/dwc_translations.rdf"/>
<rdf:type rdf:resource="http://www.w3.org/1999/02/22-rdf-syntax-ns#Property"/>
</skos:Concept>
<skos:Concept rdf:about="http://rs.tdwg.org/dwc/terms/datasetID">
<skos:prefLabel xml:lang="en">Dataset ID</skos:prefLabel>
<skos:definition xml:lang="en">An identifier for the set of data.
			May
			be a global unique identifier or an identifier specific to a
			collection or institution.</skos:definition>
<skos:example xml:lang="en"/>
<skos:prefLabel xml:lang="es">ID del conjunto de datos</skos:prefLabel>
<skos:definition xml:lang="es">Un identificador para el conjunto de
			datos. Puede ser un identificador único global o un identificador
			específico de una colección o institución.</skos:definition>
<skos:example xml:lang="es"/>
<skos:prefLabel xml:lang="zh-Hans">数据集编号</skos:prefLabel>
<skos:definition xml:lang="zh-Hans">数据集的标识符。可能是一个全局唯一标识符或一个保藏中心或研究机构的特定标识符。</skos:definition>
<skos:example xml:lang="zh-Hans"/>
<skos:prefLabel xml:lang="ja"/>
<skos:definition xml:lang="ja">データセットのID。GUIDまたは、そのコレクションや機関に固有のID。</skos:definition>
<skos:example xml:lang="ja"/>
<skos:inScheme rdf:resource="http://rs.gbif.org/terms/dwc/dwc_translations.rdf"/>
<rdf:type rdf:resource="http://www.w3.org/1999/02/22-rdf-syntax-ns#Property"/>
</skos:Concept>
<skos:Concept rdf:about="http://rs.tdwg.org/dwc/terms/datasetName">
<skos:prefLabel xml:lang="en">Dataset Name</skos:prefLabel>
<skos:definition xml:lang="en">The name identifying the data set
			from
			which the record was derived.</skos:definition>
<skos:example xml:lang="en">Examples: "Grinnell
			Resurvey Mammals", "Lacey
			Ctenomys Recaptures"</skos:example>
<skos:prefLabel xml:lang="es">Nombre del conjunto de datos</skos:prefLabel>
<skos:definition xml:lang="es">El nombre que identifica el conjunto
			de datos del cual se derivó el registro.  </skos:definition>
<skos:example xml:lang="es">Ejemplo: “Muestreo de Mamíferos de la
			Cuenca”</skos:example>
<skos:prefLabel xml:lang="zh-Hans">数据集名称</skos:prefLabel>
<skos:definition xml:lang="zh-Hans">标识生成记录的数据集的名称。</skos:definition>
<skos:example xml:lang="zh-Hans"/>
<skos:prefLabel xml:lang="ja"/>
<skos:definition xml:lang="ja">レコードが由来したデータセットを特定する名前。</skos:definition>
<skos:example xml:lang="ja"/>
<skos:inScheme rdf:resource="http://rs.gbif.org/terms/dwc/dwc_translations.rdf"/>
<rdf:type rdf:resource="http://www.w3.org/1999/02/22-rdf-syntax-ns#Property"/>
</skos:Concept>
<skos:Concept rdf:about="http://rs.tdwg.org/dwc/terms/dateIdentified">
<skos:prefLabel xml:lang="en">Date Identified</skos:prefLabel>
<skos:definition xml:lang="en">The date on which the subject was
			identified as representing the Taxon. Recommended best practice is to
			use an encoding scheme, such as ISO 8601:2004(E).</skos:definition>
<skos:example xml:lang="en">Examples:
			"1963-03-08T14:07-0600" is 8 Mar
			1963 2:07pm in the time zone six
			hours earlier than UTC,
			"2009-02-20T08:40Z" is 20 Feb 2009 8:40am
			UTC, "1809-02-12" is 12 Feb
			1809, "1906-06" is Jun 1906, "1971" is
			just that year,
			"2007-03-01T13:00:00Z/2008-05-11T15:30:00Z" is the
			interval between 1
			Mar 2007 1pm UTC and 11 May 2008 3:30pm UTC,
			"2007-11-13/15" is the
			interval between 13 Nov 2007 and 15 Nov 2007.
		</skos:example>
<skos:prefLabel xml:lang="es">Fecha de identificación</skos:prefLabel>
<skos:definition xml:lang="es">La fecha en que fue identificado el
			sujeto como representativo del taxón. La práctica recomendada es
			utilizar un esquema de codificación, como ISO 8601:2004 (E). </skos:definition>
<skos:example xml:lang="es">Ejemplo: "1963-03-08T14:07-0600" es 8 de
			marzo de 1963 2:07pm en zona horaria seis horas más temprano que UTC,
			"2009-02-20T08:40Z" es 20 de febrero 2009 8:40am UTC, "1809-02-12" es
			12 de febrero de 1809, "1906-06" es junio de 1906, "1971",
			"2007-03-01T13:00:00Z/2008-05-11T15:30:00Z" es el intervalo entre el
			1 de marzo de 2007 1pm UTC y 11 de mayo de 2008 3:30pm UTC,
			"2007-11-13/15" es el intervalo entre el 13 de noviembre de 2007 y 15
			de noviembre de 2007.</skos:example>
<skos:prefLabel xml:lang="zh-Hans">鉴定日期</skos:prefLabel>
<skos:definition xml:lang="zh-Hans">涉及被视为代表分类单元的主体的数据。建议最好使用编码方案，如ISO
			8601:2004(E)。</skos:definition>
<skos:example xml:lang="zh-Hans"/>
<skos:prefLabel xml:lang="ja"/>
<skos:definition xml:lang="ja">対象の分類群を同定した日付。 ISO
			8601:2004(E)などのスキーマの使用を推奨。</skos:definition>
<skos:example xml:lang="ja"/>
<skos:inScheme rdf:resource="http://rs.gbif.org/terms/dwc/dwc_translations.rdf"/>
<rdf:type rdf:resource="http://www.w3.org/1999/02/22-rdf-syntax-ns#Property"/>
</skos:Concept>
<skos:Concept rdf:about="http://rs.tdwg.org/dwc/terms/day">
<skos:prefLabel xml:lang="en">Day</skos:prefLabel>
<skos:definition xml:lang="en">The integer day of the month on
			which
			the Event occurred.</skos:definition>
<skos:example xml:lang="en">Example: "9", "28"
		</skos:example>
<skos:prefLabel xml:lang="es">Día</skos:prefLabel>
<skos:definition xml:lang="es">El día en números enteros, del mes en
			que ocurrió el evento. </skos:definition>
<skos:example xml:lang="es">Ejemplo: "9", "28"</skos:example>
<skos:prefLabel xml:lang="zh-Hans">天</skos:prefLabel>
<skos:definition xml:lang="zh-Hans">事件发生的整数天。</skos:definition>
<skos:example xml:lang="zh-Hans"/>
<skos:prefLabel xml:lang="ja"/>
<skos:definition xml:lang="ja">そのイベントが起きた日（整数）。</skos:definition>
<skos:example xml:lang="ja"/>
<skos:inScheme rdf:resource="http://rs.gbif.org/terms/dwc/dwc_translations.rdf"/>
<rdf:type rdf:resource="http://www.w3.org/1999/02/22-rdf-syntax-ns#Property"/>
</skos:Concept>
<skos:Concept rdf:about="http://rs.tdwg.org/dwc/terms/decimalLatitude">
<skos:prefLabel xml:lang="en">Decimal Latitude</skos:prefLabel>
<skos:definition xml:lang="en">The geographic latitude (in
			decimal
			degrees, using the spatial reference system given in
			geodeticDatum) of
			the geographic center of a Location. Positive
			values are north of the
			Equator, negative values are south of it.
			Legal values lie between -90
			and 90, inclusive.</skos:definition>
<skos:example xml:lang="en">Example:
			"-41.0983423"</skos:example>
<skos:prefLabel xml:lang="es">Latitud decimal</skos:prefLabel>
<skos:definition xml:lang="es">La latitud geográfica (en grados
			decimales, utilizando el sistema de referencia espacial provisto en
			Datum Geodésico) del centro geográfico de una ubicación. Los valores
			positivos se encuentran al norte del ecuador, los valores negativos
			están al sur del mismo. Los valores admitidos se encuentran entre -90
			y 90, ambos incluidos. </skos:definition>
<skos:example xml:lang="es">Ejemplo: "-41.0983423"</skos:example>
<skos:prefLabel xml:lang="zh-Hans">十进制纬度</skos:prefLabel>
<skos:definition xml:lang="zh-Hans">地点的地理中心的纬度（以小数表示，采用大地基准中提供的空间参照系统）。正值代表赤道以北，负值代表赤道以南。法定值介于-90至90（含）之间。</skos:definition>
<skos:example xml:lang="zh-Hans"/>
<skos:prefLabel xml:lang="ja"/>
<skos:definition xml:lang="ja">その場所の地理的な緯度(geodeticDatumによって与えられた空間参照システムによる小数点表現での緯度)。正の数は赤道より北、負の数は南をあらわす。指定できる値は-90から90まで。</skos:definition>
<skos:example xml:lang="ja"/>
<skos:inScheme rdf:resource="http://rs.gbif.org/terms/dwc/dwc_translations.rdf"/>
<rdf:type rdf:resource="http://www.w3.org/1999/02/22-rdf-syntax-ns#Property"/>
</skos:Concept>
<skos:Concept rdf:about="http://rs.tdwg.org/dwc/terms/decimalLongitude">
<skos:prefLabel xml:lang="en">Decimal Longitude</skos:prefLabel>
<skos:definition xml:lang="en">The geographic longitude (in
			decimal
			degrees, using the spatial reference system given in
			geodeticDatum) of
			the geographic center of a Location. Positive
			values are east of the
			Greenwich Meridian, negative values are west
			of it. Legal values lie
			between -180 and 180, inclusive.
		</skos:definition>
<skos:example xml:lang="en">Example:
			"-121.1761111"</skos:example>
<skos:prefLabel xml:lang="es">Longitud decimal</skos:prefLabel>
<skos:definition xml:lang="es">La longitud geográfica (en grados
			decimales, mediante el sistema de referencia espacial provisto en
			Datum Geodésico) del centro geográfico de un lugar. Los valores
			positivos se encuentran al este del meridiano de Greenwich, los
			valores negativos se encuentran al oeste de la misma. Los valores
			admitidos se encuentran entre -180 y 180, ambos incluidos. </skos:definition>
<skos:example xml:lang="es">Ejemplo: "-121.1761111"</skos:example>
<skos:prefLabel xml:lang="zh-Hans">十进制经度</skos:prefLabel>
<skos:definition xml:lang="zh-Hans">地点的地理中心的经度（以小数表示，采用大地基准中提供的空间参照系统）。正值代表格林威治子午线以西，负值代表格林威治子午线以东。法定值介于-180至180（含）之间。</skos:definition>
<skos:example xml:lang="zh-Hans"/>
<skos:prefLabel xml:lang="ja"/>
<skos:definition xml:lang="ja">その場所の地理的な経度(geodeticDatumによって与えられた空間参照システムによる小数点表現での緯度)。正の数はグリニッジ子午線より東、負の数は西をあらわす。指定できる値は-180から180まで。</skos:definition>
<skos:example xml:lang="ja"/>
<skos:inScheme rdf:resource="http://rs.gbif.org/terms/dwc/dwc_translations.rdf"/>
<rdf:type rdf:resource="http://www.w3.org/1999/02/22-rdf-syntax-ns#Property"/>
</skos:Concept>
<skos:Concept rdf:about="http://rs.tdwg.org/dwc/terms/disposition">
<skos:prefLabel xml:lang="en">Disposition</skos:prefLabel>
<skos:definition xml:lang="en">The current state of a specimen
			with
			respect to the collection identified in collectionCode or
			collectionID. Recommended best practice is to use a controlled
			vocabulary.</skos:definition>
<skos:example xml:lang="en">Examples: "in
			collection", "missing",
			"voucher elsewhere", "duplicates elsewhere"
		</skos:example>
<skos:prefLabel xml:lang="es">Disposición</skos:prefLabel>
<skos:definition xml:lang="es">El estado actual de un espécimen con
			respecto a la colección identificada en Código de la Colección o ID
			de la Colección. La práctica recomendada es el uso de un lenguaje
			controlado. </skos:definition>
<skos:example xml:lang="es">Ejemplo: "en colección", "faltante",
			"ejemplar testigo", "duplicados en otro lugar"</skos:example>
<skos:prefLabel xml:lang="zh-Hans">寄存</skos:prefLabel>
<skos:definition xml:lang="zh-Hans">与确定了保藏代码或保藏识别码的保藏物相关的标本的当前状态。推荐使用控制词表。</skos:definition>
<skos:example xml:lang="zh-Hans"/>
<skos:prefLabel xml:lang="ja"/>
<skos:definition xml:lang="ja">collectionCodeやcollectionIDで特定されるコレクションに関しての資料の現在の状態。管理された語彙の使用を推奨。</skos:definition>
<skos:example xml:lang="ja"/>
<skos:inScheme rdf:resource="http://rs.gbif.org/terms/dwc/dwc_translations.rdf"/>
<rdf:type rdf:resource="http://www.w3.org/1999/02/22-rdf-syntax-ns#Property"/>
</skos:Concept>
<skos:Concept rdf:about="http://rs.tdwg.org/dwc/terms/dynamicProperties">
<skos:prefLabel xml:lang="en">Dynamic Properties</skos:prefLabel>
<skos:definition xml:lang="en">A list (concatenated and
			separated) of
			additional measurements, facts, characteristics, or
			assertions about
			the record. Meant to provide a mechanism for
			structured content such
			as key-value pairs.</skos:definition>
<skos:example xml:lang="en">Examples:
			"tragusLengthInMeters=0.014;
			weightInGrams=120",
			"heightInMeters=1.5", "natureOfID=expert
			identification;
			identificationEvidence=cytochrome B sequence",
			"relativeHumidity=28;
			airTemperatureInC=22; sampleSizeInKilograms=10",
			"aspectHeading=277;
			slopeInDegrees=6", "iucnStatus=vulnerable;
			taxonDistribution=Neuquen,
			Argentina"</skos:example>
<skos:prefLabel xml:lang="es">Propiedades dinámicas</skos:prefLabel>
<skos:definition xml:lang="es">Una lista (concatenada y separada) de
			las medidas, hechos, características, o aseveraciones adicionales
			sobre el registro. Su intención es proporcionar un mecanismo para
			contenido estructurado como pares de valor.  </skos:definition>
<skos:example xml:lang="es">Ejemplos: "peso en gramos =120", "altura en
			metros =1,5", "naturaleza del ID =identificación de experto;
			evidencia de la identificación =secuencia de citocromo B", "humedad
			relativa =28; temperatura del aire en grados ºC =22; tamaño de la
			muestra en kilogramos =10", "estado según UICN =vulnerable;
			distribución del taxón =Neuquén, Argentina"</skos:example>
<skos:prefLabel xml:lang="zh-Hans">动态属性</skos:prefLabel>
<skos:definition xml:lang="zh-Hans">关于记录的其他测量、情况、特征、判定等信息的（连接的或分开的）列表。意在为诸如键值对等的结构化内容设立机制。</skos:definition>
<skos:example xml:lang="zh-Hans"/>
<skos:prefLabel xml:lang="ja"/>
<skos:definition xml:lang="ja">レコードに関しての付加的な測定、事実、特徴、または主張。キーと値のペアなど、構造化された内容に対する仕組みの提供を意図している。</skos:definition>
<skos:example xml:lang="ja"/>
<skos:inScheme rdf:resource="http://rs.gbif.org/terms/dwc/dwc_translations.rdf"/>
<rdf:type rdf:resource="http://www.w3.org/1999/02/22-rdf-syntax-ns#Property"/>
</skos:Concept>
<skos:Concept rdf:about="http://rs.tdwg.org/dwc/terms/earliestAgeOrLowestStage">
<skos:prefLabel xml:lang="en">Earliest Age Or Lowest Stage
		</skos:prefLabel>
<skos:definition xml:lang="en">The full name of the earliest
			possible
			geochronologic age or lowest chronostratigraphic stage
			attributable to
			the stratigraphic horizon from which the cataloged
			item was collected.</skos:definition>
<skos:example xml:lang="en">Examples:
			"Atlantic", "Boreal",
			"Skullrockian"</skos:example>
<skos:prefLabel xml:lang="es">Edad temprana o estadío inferior</skos:prefLabel>
<skos:definition xml:lang="es">El nombre completo de la edad
			geocronológica más temprana posible o la etapa cronoestratigráfica
			más baja, atribuible al horizonte estratigráfico donde se recolectó
			el objeto catalogado. </skos:definition>
<skos:example xml:lang="es">Ejemplos: "Atlántico", "Boreal"</skos:example>
<skos:prefLabel xml:lang="zh-Hans">最早地质年代或最低年代地层</skos:prefLabel>
<skos:definition xml:lang="zh-Hans">编目项所采集的地层层位所属之可能的最早的地质年代或最低的年代地层的全称。</skos:definition>
<skos:example xml:lang="zh-Hans"/>
<skos:prefLabel xml:lang="ja"/>
<skos:definition xml:lang="ja">この項目が収集された層位が帰属している、あり得る最古の地質年代学的期、または最下部の年代層序的階のフルネーム。</skos:definition>
<skos:example xml:lang="ja"/>
<skos:inScheme rdf:resource="http://rs.gbif.org/terms/dwc/dwc_translations.rdf"/>
<rdf:type rdf:resource="http://www.w3.org/1999/02/22-rdf-syntax-ns#Property"/>
</skos:Concept>
<skos:Concept rdf:about="http://rs.tdwg.org/dwc/terms/earliestEonOrLowestEonothem">
<skos:prefLabel xml:lang="en">Earliest Eon Or Lowest Eonothem
		</skos:prefLabel>
<skos:definition xml:lang="en">The full name of the earliest
			possible
			geochronologic eon or lowest chrono-stratigraphic eonothem
			or the
			informal name ("Precambrian") attributable to the
			stratigraphic
			horizon from which the cataloged item was collected.
		</skos:definition>
<skos:example xml:lang="en">Examples:
			"Phanerozoic", "Proterozoic"</skos:example>
<skos:prefLabel xml:lang="es">Eón temprano o eonotema inferior</skos:prefLabel>
<skos:definition xml:lang="es">El nombre completo del eón
			geocronológico más temprano o el eratema crono-estratigráfico más
			bajo, o el nombre informal ("Precámbrico") atribuible al horizonte
			estratigráfico donde se recolectó el objeto catalogado. </skos:definition>
<skos:example xml:lang="es">Ejemplo: "Fanerozoico", "Proterozoico"</skos:example>
<skos:prefLabel xml:lang="zh-Hans">最早地质宙或最低地层宇</skos:prefLabel>
<skos:definition xml:lang="zh-Hans">编目项所采集的地层层位所属之可能的最早的地质宙或最低的地层宇的全称或非正式名称（“前寒武纪”）。</skos:definition>
<skos:example xml:lang="zh-Hans"/>
<skos:prefLabel xml:lang="ja"/>
<skos:definition xml:lang="ja">この項目が収集された層位が帰属している、あり得る最古の地質年代学的累代、また最下部の年代層序的累界のフルネーム、または“Precambrian”のような非公式の名前。</skos:definition>
<skos:example xml:lang="ja"/>
<skos:inScheme rdf:resource="http://rs.gbif.org/terms/dwc/dwc_translations.rdf"/>
<rdf:type rdf:resource="http://www.w3.org/1999/02/22-rdf-syntax-ns#Property"/>
</skos:Concept>
<skos:Concept rdf:about="http://rs.tdwg.org/dwc/terms/earliestEpochOrLowestSeries">
<skos:prefLabel xml:lang="en">Earliest Epoch Or Lowest Series
		</skos:prefLabel>
<skos:definition xml:lang="en">The full name of the earliest
			possible
			geochronologic epoch or lowest chronostratigraphic series
			attributable to the stratigraphic horizon from which the cataloged
			item was collected.</skos:definition>
<skos:example xml:lang="en">Examples:
			"Holocene", "Pleistocene", "Ibexian
			Series"</skos:example>
<skos:prefLabel xml:lang="es">Época temprana o serie inferior</skos:prefLabel>
<skos:definition xml:lang="es">El nombre completo de la época
			geocronológica más temprana o la serie cronoestratigráfica más baja
			posible, atribuible al horizonte estratigráfico donde se recolectó el
			objeto catalogado. </skos:definition>
<skos:example xml:lang="es">Ejemplos: "Holoceno", "Pleistoceno",
			"Serie Ibexian"</skos:example>
<skos:prefLabel xml:lang="zh-Hans">最早地质世或最低地层统</skos:prefLabel>
<skos:definition xml:lang="zh-Hans">编目项所采集的地层层位所属之可能的最早的地质世或最低的地层统的全称。</skos:definition>
<skos:example xml:lang="zh-Hans"/>
<skos:prefLabel xml:lang="ja"/>
<skos:definition xml:lang="ja">この項目が収集された層位が帰属している、あり得る最古の地質年代学的世、または最下部の年代層序的統のフルネーム。</skos:definition>
<skos:example xml:lang="ja"/>
<skos:inScheme rdf:resource="http://rs.gbif.org/terms/dwc/dwc_translations.rdf"/>
<rdf:type rdf:resource="http://www.w3.org/1999/02/22-rdf-syntax-ns#Property"/>
</skos:Concept>
<skos:Concept rdf:about="http://rs.tdwg.org/dwc/terms/earliestEraOrLowestErathem">
<skos:prefLabel xml:lang="en">Earliest Era Or Lowest Erathem
		</skos:prefLabel>
<skos:definition xml:lang="en">The full name of the earliest
			possible
			geochronologic era or lowest chronostratigraphic erathem
			attributable
			to the stratigraphic horizon from which the cataloged
			item was
			collected.</skos:definition>
<skos:example xml:lang="en">Examples:
			"Cenozoic", "Mesozoic"</skos:example>
<skos:prefLabel xml:lang="es">Era temprana o eratema inferior</skos:prefLabel>
<skos:definition xml:lang="es">El nombre completo de la era
			geocronológica más temprana o el eratema crono-estratigráfico más
			bajo, atribuible al horizonte estratigráfico donde se recolectó el
			objeto catalogado. </skos:definition>
<skos:example xml:lang="es">Ejemplos: "Cenozoico", "Mesozoico"</skos:example>
<skos:prefLabel xml:lang="zh-Hans">最早地质代或最低地层界</skos:prefLabel>
<skos:definition xml:lang="zh-Hans">编目项所采集的地层层位所属之可能的最早的地质代或最低的地层界的全称。</skos:definition>
<skos:example xml:lang="zh-Hans"/>
<skos:prefLabel xml:lang="ja"/>
<skos:definition xml:lang="ja">この項目が収集された層位が帰属している、あり得る最古の地質年代学的代、または最下部の年代層序的界のフルネーム。</skos:definition>
<skos:example xml:lang="ja"/>
<skos:inScheme rdf:resource="http://rs.gbif.org/terms/dwc/dwc_translations.rdf"/>
<rdf:type rdf:resource="http://www.w3.org/1999/02/22-rdf-syntax-ns#Property"/>
</skos:Concept>
<skos:Concept rdf:about="http://rs.tdwg.org/dwc/terms/earliestPeriodOrLowestSystem">
<skos:prefLabel xml:lang="en">Earliest Period Or Lowest System
		</skos:prefLabel>
<skos:definition xml:lang="en">The full name of the earliest
			possible
			geochronologic period or lowest chronostratigraphic system
			attributable to the stratigraphic horizon from which the cataloged
			item was collected.</skos:definition>
<skos:example xml:lang="en">Examples: "Neogene",
			"Tertiary", "Quaternary"</skos:example>
<skos:prefLabel xml:lang="es">Periodo temprano o sistema inferior</skos:prefLabel>
<skos:definition xml:lang="es">Puede corresponder a: a) un indicador
			de la existencia de, b) una referencia a (publicación, URI), o c) el
			texto de las notas tomadas en campo sobre el evento.</skos:definition>
<skos:example xml:lang="es">Ejemplos: "Neógeno", "Terciario",
			"Cuaternario"</skos:example>
<skos:prefLabel xml:lang="zh-Hans">最早地质纪或最低地层系</skos:prefLabel>
<skos:definition xml:lang="zh-Hans">编目项所采集的地层层位所属之可能的最早的地质纪或最低的地层系的全称。</skos:definition>
<skos:example xml:lang="zh-Hans"/>
<skos:prefLabel xml:lang="ja"/>
<skos:definition xml:lang="ja">この項目が収集された層位が帰属している、あり得る最古の地質年代学的紀、または最下部の年代層序的系のフルネーム。</skos:definition>
<skos:example xml:lang="ja"/>
<skos:inScheme rdf:resource="http://rs.gbif.org/terms/dwc/dwc_translations.rdf"/>
<rdf:type rdf:resource="http://www.w3.org/1999/02/22-rdf-syntax-ns#Property"/>
</skos:Concept>
<skos:Concept rdf:about="http://rs.tdwg.org/dwc/terms/endDayOfYear">
<skos:prefLabel xml:lang="en">End Day Of Year</skos:prefLabel>
<skos:definition xml:lang="en">The latest ordinal day of the year
			on
			which the Event occurred (1 for January 1, 365 for December 31,
			except in a leap year, in which case it is 366).</skos:definition>
<skos:example xml:lang="en">Examples: "1" (=1
			Jan), "366" (=31 Dec),
			"365" (=30 Dec in a leap year, 31 Dec in a
			non-leap year)</skos:example>
<skos:prefLabel xml:lang="es">Día final del año</skos:prefLabel>
<skos:definition xml:lang="es">El último día ordinal del año en que
			ocurrió el evento (1 para el 1º de enero, 365 para el 31 de
			diciembre, excepto en un año bisiesto, en cuyo caso es 366).</skos:definition>
<skos:example xml:lang="es">Ejemplos: "1" (=1 enero), "365" (=31
			diciembre), "366" (=31 diciembre en año bisiesto)</skos:example>
<skos:prefLabel xml:lang="zh-Hans">当年结束日</skos:prefLabel>
<skos:definition xml:lang="zh-Hans">事件发生当年的最新日期号（除了闰年有366天的情况，1代表1月1日，365代表12月31日）。</skos:definition>
<skos:example xml:lang="zh-Hans"/>
<skos:prefLabel xml:lang="ja"/>
<skos:definition xml:lang="ja">イベントが生じた年の最も遅い日付（1月1日は1、12月31日は365とする。ただし、閏年以外。閏年の場合は12月31日が366となる）</skos:definition>
<skos:example xml:lang="ja">例: "1" (=1 Jan), "366" (=31 Dec), "365"
			(=閏年の場合30 Dec, 閏年以外の場合は31 Dec) </skos:example>
<skos:inScheme rdf:resource="http://rs.gbif.org/terms/dwc/dwc_translations.rdf"/>
<rdf:type rdf:resource="http://www.w3.org/1999/02/22-rdf-syntax-ns#Property"/>
</skos:Concept>
<skos:Concept rdf:about="http://rs.tdwg.org/dwc/terms/establishmentMeans">
<skos:prefLabel xml:lang="en">Establishment Means</skos:prefLabel>
<skos:definition xml:lang="en">The process by which the
			biological
			individual(s) represented in the Occurrence became
			established at the
			location. Recommended best practice is to use a
			controlled vocabulary.</skos:definition>
<skos:example xml:lang="en">Examples:
			"cultivated", "invasive", "escaped
			from captivity", "wild", "native"
		</skos:example>
<skos:prefLabel xml:lang="es">Medios de establecimiento</skos:prefLabel>
<skos:definition xml:lang="es">El proceso por el cual el individuo(s)
			biológico(s) representado en el Registro Biológico se estableció en
			el lugar. La práctica recomendada es el uso de un lenguaje
			controlado. </skos:definition>
<skos:example xml:lang="es">Ejemplos: "cultivado", "invasor", "fugado de
			cautiverio", "silvestre", "nativo"</skos:example>
<skos:prefLabel xml:lang="zh-Hans">确定方法</skos:prefLabel>
<skos:definition xml:lang="zh-Hans">在采集地点确定生物个体在事件中表现的过程。建议最佳做法是使用一个控制性词汇。</skos:definition>
<skos:example xml:lang="zh-Hans"/>
<skos:prefLabel xml:lang="ja"/>
<skos:definition xml:lang="ja">その位置において、生物個体を確立するために用いた処理。管理された語彙の使用を推奨。</skos:definition>
<skos:example xml:lang="ja"/>
<skos:inScheme rdf:resource="http://rs.gbif.org/terms/dwc/dwc_translations.rdf"/>
<rdf:type rdf:resource="http://www.w3.org/1999/02/22-rdf-syntax-ns#Property"/>
</skos:Concept>
<skos:Concept rdf:about="http://rs.tdwg.org/dwc/terms/eventDate">
<skos:prefLabel xml:lang="en">Event Date</skos:prefLabel>
<skos:definition xml:lang="en">The date-time or interval during
			which
			an Event occurred. For occurrences, this is the date-time when
			the
			event was recorded. Not suitable for a time in a geological
			context.
			Recommended best practice is to use an encoding scheme, such
			as ISO
			8601:2004(E).</skos:definition>
<skos:example xml:lang="en">Examples:
			"1963-03-08T14:07-0600" is 8 Mar
			1963 2:07pm in the time zone six
			hours earlier than UTC,
			"2009-02-20T08:40Z" is 20 Feb 2009 8:40am
			UTC, "1809-02-12" is 12 Feb
			1809, "1906-06" is Jun 1906, "1971" is
			just that year,
			"2007-03-01T13:00:00Z/2008-05-11T15:30:00Z" is the
			interval between 1
			Mar 2007 1pm UTC and 11 May 2008 3:30pm UTC,
			"2007-11-13/15" is the
			interval between 13 Nov 2007 and 15 Nov 2007.
		</skos:example>
<skos:prefLabel xml:lang="es">Fecha del evento</skos:prefLabel>
<skos:definition xml:lang="es">La fecha y hora o el intervalo durante
			el cual se produjo un evento. Para los registros de especies, esta es
			la fecha y hora cuando el evento se registró. No es adecuado para un
			momento en un contexto geológico. La práctica recomendada es utilizar
			un esquema de codificación, tal como ISO 8601:2004 (E). </skos:definition>
<skos:example xml:lang="es">Ejemplo: "1963-03-08T14:07-0600" es 8 de
			marzo de 1963 2:07pm en zona horaria seis horas más temprano que UTC,
			"2009-02-20T08:40Z" es 20 de febrero 2009 8:40am UTC, "1809-02-12" es
			12 de febrero de 1809, "1906-06" es junio de 1906, "1971",
			"2007-03-01T13:00:00Z/2008-05-11T15:30:00Z" es el intervalo entre el
			1 de marzo de 2007 1pm UTC y 11 de mayo de 2008 3:30pm UTC,
			"2007-11-13/15" es el intervalo entre el 13 de noviembre de 2007 y 15
			de noviembre de 2007.</skos:example>
<skos:prefLabel xml:lang="zh-Hans">事件日期</skos:prefLabel>
<skos:definition xml:lang="zh-Hans">事件发生的日期或间隔。对于已发生的事件这是被记录的日期。
			不适合地质背景时间。建议最佳做法是使用一个编码方案，例如ISO 8601:2004(E)。</skos:definition>
<skos:example xml:lang="zh-Hans"/>
<skos:prefLabel xml:lang="ja"/>
<skos:definition xml:lang="ja">イベントが生じた日付または間隔。イベントが記録された日時など。地質年代を記録する目的には使用しない。
			ISO 8601:2004(E)などのスキーマの使用を推奨。</skos:definition>
<skos:example xml:lang="ja">例:
			"1963-03-08T14:07-0600"であれば、UTCよりも6時間早いタイムゾーンにおける1963年5月8日2:07pm,
			"2009-02-20T08:40Z"であればUTCにおける2009年2月20日8:40am,
			"1809-02-12"であれば1809年の2月12日, "1906-06"であれば1906年6月, "1971"であれば1971年,
			"2007-03-01T13:00:00Z/2008-05-11T15:30:00Z"であればUTCにおける2007年3月1日1pmから2008年5月11日3:30pmまでの間,
			"2007-11-13/15"であれば2007年11月13日から15日までの間を表す。</skos:example>
<skos:inScheme rdf:resource="http://rs.gbif.org/terms/dwc/dwc_translations.rdf"/>
<rdf:type rdf:resource="http://www.w3.org/1999/02/22-rdf-syntax-ns#Property"/>
</skos:Concept>
<skos:Concept rdf:about="http://rs.tdwg.org/dwc/terms/eventID">
<skos:prefLabel xml:lang="en">Event ID</skos:prefLabel>
<skos:definition xml:lang="en">An identifier for the set of
			information associated with an Event (something that occurs at a
			place and time). May be a global unique identifier or an identifier
			specific to the data set.</skos:definition>
<skos:example xml:lang="en"/>
<skos:prefLabel xml:lang="es">ID del evento</skos:prefLabel>
<skos:definition xml:lang="es">Un identificador para el conjunto de
			la información asociada a un Evento (algo que ocurre en un lugar y
			tiempo). Puede ser un identificador único global o un identificador
			específico para el conjunto de datos. </skos:definition>
<skos:example xml:lang="es"/>
<skos:prefLabel xml:lang="zh-Hans">事件编号</skos:prefLabel>
<skos:definition xml:lang="zh-Hans">与事件相关的信息集标识符（发生在同一地点和时间）。可能是一个全局唯一标识符或特定的数据集标识符。</skos:definition>
<skos:example xml:lang="zh-Hans"/>
<skos:prefLabel xml:lang="ja"/>
<skos:definition xml:lang="ja">イベントに関連する情報セット（その場所のその時間に発生した何らかの事象）のID。GUIDあるいは、データセット固有のID。</skos:definition>
<skos:example xml:lang="ja"/>
<skos:inScheme rdf:resource="http://rs.gbif.org/terms/dwc/dwc_translations.rdf"/>
<rdf:type rdf:resource="http://www.w3.org/1999/02/22-rdf-syntax-ns#Property"/>
</skos:Concept>
<skos:Concept rdf:about="http://rs.tdwg.org/dwc/terms/eventRemarks">
<skos:prefLabel xml:lang="en">Event Remarks</skos:prefLabel>
<skos:definition xml:lang="en">Comments or notes about the Event.
		</skos:definition>
<skos:example xml:lang="en">Example: "after the
			recent rains the river is
			nearly at flood stage"
		</skos:example>
<skos:prefLabel xml:lang="es">Comentarios del evento</skos:prefLabel>
<skos:definition xml:lang="es">Comentarios o anotaciones sobre el
			evento. </skos:definition>
<skos:example xml:lang="es">Ejemplo: "después de las lluvias recientes,
			el río estuvo cercano a un estado de desbordamiento"</skos:example>
<skos:prefLabel xml:lang="zh-Hans">事件备注</skos:prefLabel>
<skos:definition xml:lang="zh-Hans">关于事件的评论或记录。</skos:definition>
<skos:example xml:lang="zh-Hans"/>
<skos:prefLabel xml:lang="ja"/>
<skos:definition xml:lang="ja">イベントに関するコメントあるいは注釈。</skos:definition>
<skos:example xml:lang="ja"/>
<skos:inScheme rdf:resource="http://rs.gbif.org/terms/dwc/dwc_translations.rdf"/>
<rdf:type rdf:resource="http://www.w3.org/1999/02/22-rdf-syntax-ns#Property"/>
</skos:Concept>
<skos:Concept rdf:about="http://rs.tdwg.org/dwc/terms/eventTime">
<skos:prefLabel xml:lang="en">Event Time</skos:prefLabel>
<skos:definition xml:lang="en">The time or interval during which
			an
			Event occurred. Recommended best practice is to use an encoding
			scheme, such as ISO 8601:2004(E).</skos:definition>
<skos:example xml:lang="en">Examples:
			"14:07-0600" is 2:07pm in the time
			zone six hours earlier than UTC,
			"08:40:21Z" is 8:40:21am UTC,
			"13:00:00Z/15:30:00Z" is the interval
			between 1pm UTC and 3:30pm UTC.</skos:example>
<skos:prefLabel xml:lang="es">Hora del evento</skos:prefLabel>
<skos:definition xml:lang="es">El tiempo o intervalo durante el cual
			se produjo un evento. La práctica recomendada es utilizar un esquema
			de codificación, tales como ISO 8601:2004 (E). </skos:definition>
<skos:example xml:lang="es">Ejemplos: "14:07-0600" es 2:07pm en zona
			horaria seis horas más temprano que UTC, "08:40:21Z" es 8:40:21am
			UTC, "13:00:00Z/15:30:00Z" es el intervalo entre 1pm UTC y 3:30pm
			UTC.</skos:example>
<skos:prefLabel xml:lang="zh-Hans">事件时间</skos:prefLabel>
<skos:definition xml:lang="zh-Hans">事件发生的时间或间隔。 建议最佳做法是使用一个编码方案，例如ISO
			8601:2004(E)。</skos:definition>
<skos:example xml:lang="zh-Hans"/>
<skos:prefLabel xml:lang="ja"/>
<skos:definition xml:lang="ja">イベントが発生した時間あるいは時間の間隔。ISO
			8601:2004(E)のようなスキーマの使用を推奨。</skos:definition>
<skos:example xml:lang="ja"/>
<skos:inScheme rdf:resource="http://rs.gbif.org/terms/dwc/dwc_translations.rdf"/>
<rdf:type rdf:resource="http://www.w3.org/1999/02/22-rdf-syntax-ns#Property"/>
</skos:Concept>
<skos:Concept rdf:about="http://rs.tdwg.org/dwc/terms/family">
<skos:prefLabel xml:lang="en">Family</skos:prefLabel>
<skos:definition xml:lang="en">The full scientific name of the
			family
			in which the taxon is classified.</skos:definition>
<skos:example xml:lang="en">Example: "Felidae",
			"Monocleaceae"</skos:example>
<skos:prefLabel xml:lang="es">Familia</skos:prefLabel>
<skos:definition xml:lang="es">El nombre científico completo de la
			familia en el que se clasifica el taxón. </skos:definition>
<skos:example xml:lang="es">Ejemplo: "Felidae", "Monocleaceae"</skos:example>
<skos:prefLabel xml:lang="zh-Hans">科</skos:prefLabel>
<skos:definition xml:lang="zh-Hans">分类单元所属科的完整学名。</skos:definition>
<skos:example xml:lang="zh-Hans"/>
<skos:prefLabel xml:lang="ja"/>
<skos:definition xml:lang="ja">その分類群が位置づけられる、分類学上の「科」のフルネーム。</skos:definition>
<skos:example xml:lang="ja"/>
<skos:inScheme rdf:resource="http://rs.gbif.org/terms/dwc/dwc_translations.rdf"/>
<rdf:type rdf:resource="http://www.w3.org/1999/02/22-rdf-syntax-ns#Property"/>
</skos:Concept>
<skos:Concept rdf:about="http://rs.tdwg.org/dwc/terms/fieldNotes">
<skos:prefLabel xml:lang="en">Field Notes</skos:prefLabel>
<skos:definition xml:lang="en">One of a) an indicator of the
			existence of, b) a reference to (publication, URI), or c) the text of
			notes taken in the field about the Event.</skos:definition>
<skos:example xml:lang="en">Example: "notes
			available in Grinnell-Miller
			Library"</skos:example>
<skos:prefLabel xml:lang="es">Notas de campo</skos:prefLabel>
<skos:definition xml:lang="es">Puede corresponder a: a) un indicador
			de la existencia de, b) una referencia a (publicación, URI), o c) el
			texto de las notas tomadas en campo sobre el evento.</skos:definition>
<skos:example xml:lang="es">Ejemplo: "notas disponibles en
			Grinnell-Miller Library"</skos:example>
<skos:prefLabel xml:lang="zh-Hans">现场记录</skos:prefLabel>
<skos:definition xml:lang="zh-Hans">有关事件的现场记录之一：a）存在标志，b）出版物、网站资源参考，c）记录文本。</skos:definition>
<skos:example xml:lang="zh-Hans"/>
<skos:prefLabel xml:lang="ja"/>
<skos:definition xml:lang="ja">イベントに関する、１）存在している場所の指示、２）出版物やURIへの参照、または、３）そのフィールドで用いられた記録のテキスト。</skos:definition>
<skos:example xml:lang="ja"/>
<skos:inScheme rdf:resource="http://rs.gbif.org/terms/dwc/dwc_translations.rdf"/>
<rdf:type rdf:resource="http://www.w3.org/1999/02/22-rdf-syntax-ns#Property"/>
</skos:Concept>
<skos:Concept rdf:about="http://rs.tdwg.org/dwc/terms/fieldNumber">
<skos:prefLabel xml:lang="en">Field Number</skos:prefLabel>
<skos:definition xml:lang="en">An identifier given to the event
			in the
			field. Often serves as a link between field notes and the
			Event.</skos:definition>
<skos:example xml:lang="en">Example: "RV Sol
			87-03-08"</skos:example>
<skos:prefLabel xml:lang="es">Número de campo</skos:prefLabel>
<skos:definition xml:lang="es">Un identificador dado en campo al
			evento. A menudo sirve como un vínculo entre las anotaciones de campo
			y el evento.</skos:definition>
<skos:example xml:lang="es">Ejemplo: "RV Sol 87-03-08"</skos:example>
<skos:prefLabel xml:lang="zh-Hans">现场编号</skos:prefLabel>
<skos:definition xml:lang="zh-Hans">现场事件标识符。通常作为现场记录和事件的联系。</skos:definition>
<skos:example xml:lang="zh-Hans"/>
<skos:prefLabel xml:lang="ja"/>
<skos:definition xml:lang="ja">フィールド上のイベントに与えられるID。しばしば、フィールドノートとイベントの間のリンクの役割を果たす。</skos:definition>
<skos:example xml:lang="ja"/>
<skos:inScheme rdf:resource="http://rs.gbif.org/terms/dwc/dwc_translations.rdf"/>
<rdf:type rdf:resource="http://www.w3.org/1999/02/22-rdf-syntax-ns#Property"/>
</skos:Concept>
<skos:Concept rdf:about="http://rs.tdwg.org/dwc/terms/footprintSpatialFit">
<skos:prefLabel xml:lang="en">Footprint Spatial Fit</skos:prefLabel>
<skos:definition xml:lang="en">The ratio of the area of the
			footprint
			(footprintWKT) to the area of the true (original, or most
			specific)
			spatial representation of the Location. Legal values are 0,
			greater
			than or equal to 1, or undefined. A value of 1 is an exact
			match or
			100% overlap. A value of 0 should be used if the given
			footprint does
			not completely contain the original representation.
			The
			footprintSpatialFit is undefined (and should be left blank) if
			the
			original representation is a point and the given georeference is
			not
			that same point. If both the original and the given georeference
			are
			the same point, the footprintSpatialFit is 1.</skos:definition>
<skos:example xml:lang="en">Detailed
			explanations with graphical examples
			can be found in the "Guide to
			Best Practices for Georeferencing",
			Chapman and Wieczorek, eds. 2006
			(http://www.gbif.org/prog/digit/Georeferencing).
		</skos:example>
<skos:prefLabel xml:lang="es">Ajuste espacial de footprint</skos:prefLabel>
<skos:definition xml:lang="es">La relación del área de footprint (WKT
			Footprint) y el área de la verdadera (original, o más específica)
			representación espacial de la ubicación. Los valores válidos son 0,
			mayor que o igual a 1, o indefinido. Un valor de 1 es una
			coincidencia exacta o superposición de 100%. Un valor de 0 debe ser
			utilizado si el footprint dado no contiene completamente la
			representación original. El Ajuste Espacial de Footprint es
			indefinido (y se debe dejar en blanco) si la representación original
			es un punto y la georreferencia dada no es ese mismo punto. Si el
			original y la georreferencia dada son el mismo punto, el Ajuste
			Espacial de Footprint es 1. </skos:definition>
<skos:example xml:lang="es">Ejemplo: Explicaciones detalladas con
			ejemplos gráficos disponibles en el documento "Guide to Best
			Practices for Georeferencing", Chapman and Wieczorek, eds. 2006
			(http://www.gbif.org/prog/digit/Georeferencing). </skos:example>
<skos:prefLabel xml:lang="zh-Hans">足迹空间拟合</skos:prefLabel>
<skos:definition xml:lang="zh-Hans">采集地点足迹区面积（footprintWKT）与真正（最初或最具体）所用空间面积的比率。合法值是0，或大于等于1，或未定义。值为1时表示两者精确匹配或100%重叠。值为0时表示给定的足迹区不完全包含最初地域。如果最初地域是一个点而给定的地理参考是另外一个点，那么足迹空间拟合值未定义（应该留白）。如果最初地域与给定的地理参考是同一个点，则足迹空间拟合值为1。</skos:definition>
<skos:example xml:lang="zh-Hans"/>
<skos:prefLabel xml:lang="ja"/>
<skos:definition xml:lang="ja">その場所の空間表現をする際の範囲(footprintWKT)の割合。値としては0,
			1または1以下1以上,未定義が入力可能。1は完全一致、0は範囲が元の位置を全くカバーしていない場合に用いる。この値は、元の位置が地理参照で全くカバーされていない場合には、値を未定義として空欄にすべきである。もし元の位置と地理参照が完全に一致した場合は、この値は1となる。</skos:definition>
<skos:example xml:lang="ja"/>
<skos:inScheme rdf:resource="http://rs.gbif.org/terms/dwc/dwc_translations.rdf"/>
<rdf:type rdf:resource="http://www.w3.org/1999/02/22-rdf-syntax-ns#Property"/>
</skos:Concept>
<skos:Concept rdf:about="http://rs.tdwg.org/dwc/terms/footprintSRS">
<skos:prefLabel xml:lang="en">Footprint SRS</skos:prefLabel>
<skos:definition xml:lang="en">A Well-Known Text (WKT)
			representation
			of the Spatial Reference System (SRS) for the
			footprintWKT of the
			Location. Do not use this term to describe the
			SRS of the
			decimalLatitude and decimalLongitude, even if it is the
			same as for
			the footprintWKT - use the geodeticDatum instead.
		</skos:definition>
<skos:example xml:lang="en">Example: The WKT for
			the standard WGS84 SRS
			(EPSG:4326) is
			"GEOGCS["GCS_WGS_1984",DATUM["D_WGS_1984",SPHEROID["WGS_1984",6378137,298.257223563]],PRIMEM["Greenwich",0],UNIT["Degree",0.0174532925199433]]"
			without the enclosing quotes.</skos:example>
<skos:prefLabel xml:lang="es">SRS footprint</skos:prefLabel>
<skos:definition xml:lang="es">Una representación Well-Known Text
			(WKT) del sistema de referencia espacial (SRS) para WKT Footprint de
			la ubicación. No utilice este elemento para describir el SRS de
			Latitud Decimal y Longitud Decimal, incluso si es la misma que para
			WKT Footprint - utilice el Datum Geodésico en su lugar. </skos:definition>
<skos:example xml:lang="es">Ejemplo: El WKT para el estándar WGS84 SRS
			(EPSG:4326) es
			"GEOGCS["GCS_WGS_1984",DATUM["D_WGS_1984",SPHEROID["WGS_1984",6378137,298.257223563]],
			PRIMEM["Greenwich",0],UNIT["Degree",0.0174532925199433]]" sin las
			comillas.</skos:example>
<skos:prefLabel xml:lang="zh-Hans">足迹空间参考系统</skos:prefLabel>
<skos:definition xml:lang="zh-Hans">采集地点足迹区空间参考系统的公认的文本表示。请勿使用这个词描述十进制经度和纬度的空间参考系统，即便它与足迹区公认文本表示相同，请用大地基准点代替。</skos:definition>
<skos:example xml:lang="zh-Hans"/>
<skos:prefLabel xml:lang="ja"/>
<skos:definition xml:lang="ja">その場所についての空間参照システムによるWell-Known Text
			(WKT) 表現。空間参照システムのタームのdecimalLatitudeやdecimalLongitudeを表すために使ってはいけない。</skos:definition>
<skos:example xml:lang="ja"/>
<skos:inScheme rdf:resource="http://rs.gbif.org/terms/dwc/dwc_translations.rdf"/>
<rdf:type rdf:resource="http://www.w3.org/1999/02/22-rdf-syntax-ns#Property"/>
</skos:Concept>
<skos:Concept rdf:about="http://rs.tdwg.org/dwc/terms/footprintWKT">
<skos:prefLabel xml:lang="en">Footprint WKT</skos:prefLabel>
<skos:definition xml:lang="en">A Well-Known Text (WKT)
			representation
			of the shape (footprint, geometry) that defines the
			Location. A
			Location may have both a point-radius representation (see
			decimalLatitude) and a footprint representation, and they may differ
			from each other.</skos:definition>
<skos:example xml:lang="en">Example: the
			one-degree bounding box with
			opposite corners at (longitude=10,
			latitude=20) and (longitude=11,
			latitude=21) would be expressed in
			well-known text as POLYGON ((10 20,
			11 20, 11 21, 10 21, 10 20))
		</skos:example>
<skos:prefLabel xml:lang="es">WKT footprint</skos:prefLabel>
<skos:definition xml:lang="es">Una representación Well-Known Text
			(WKT) de la forma (footprint, geometría) que define la ubicación. Una
			ubicación puede tener una representación de radio-punto (véase
			Latitud Decimal) y una representación de footprint, y pueden diferir
			entre sí. </skos:definition>
<skos:example xml:lang="es">Ejemplo: El cuadrante de un grado con
			esquinas opuestas (longitud=10, latitud=20) y (longitud=11,
			latitud=21) expresadas en well-known text como POLÍGONO ((10 20, 11
			20, 11 21, 10 21, 10 20))</skos:example>
<skos:prefLabel xml:lang="zh-Hans">足迹公认文本</skos:prefLabel>
<skos:definition xml:lang="zh-Hans">描述地点形状（足迹，几何）的公认文本表示。一个地点可能同时用点半径（看十进制纬度）和足迹区表示，而两者之间并不相同。</skos:definition>
<skos:example xml:lang="zh-Hans"/>
<skos:prefLabel xml:lang="ja"/>
<skos:definition xml:lang="ja">その位置を定義する形状（範囲、幾何学的形状）の、Well-Known
			Text (WKT)
			表現。ある位置は、point-radius表現（decimalLatitudeを参照）および範囲表現を持ち、それらは互いに異なる。</skos:definition>
<skos:example xml:lang="ja">例: (経度=10, 緯度=20)と (経度=11,
			緯度=21)という対角を含む辺の長さが1のバウンディングボックスは、WKTではPOLYGON((10 20, 11 20, 11 21,
			10 21,10 20))と呼ぶ。</skos:example>
<skos:inScheme rdf:resource="http://rs.gbif.org/terms/dwc/dwc_translations.rdf"/>
<rdf:type rdf:resource="http://www.w3.org/1999/02/22-rdf-syntax-ns#Property"/>
</skos:Concept>
<skos:Concept rdf:about="http://rs.tdwg.org/dwc/terms/formation">
<skos:prefLabel xml:lang="en">Formation</skos:prefLabel>
<skos:definition xml:lang="en">The full name of the
			lithostratigraphic formation from which the cataloged item was
			collected.</skos:definition>
<skos:example xml:lang="en">Examples: "Notch
			Peak Fromation", "House
			Limestone", "Fillmore Formation"
		</skos:example>
<skos:prefLabel xml:lang="es">Formación</skos:prefLabel>
<skos:definition xml:lang="es">El nombre completo de la formación
			litoestratigráfica de la cual se colectó el objeto catalogado.</skos:definition>
<skos:example xml:lang="es">Ejemplos: "Formación Notch Peak", "Formación
			Fillmore"</skos:example>
<skos:prefLabel xml:lang="zh-Hans">地层</skos:prefLabel>
<skos:definition xml:lang="zh-Hans">采集编目项所在地层的完整名称。</skos:definition>
<skos:example xml:lang="zh-Hans"/>
<skos:prefLabel xml:lang="ja"/>
<skos:definition xml:lang="ja">この項目が収集された岩相層序の累層のフルネーム。</skos:definition>
<skos:example xml:lang="ja"/>
<skos:inScheme rdf:resource="http://rs.gbif.org/terms/dwc/dwc_translations.rdf"/>
<rdf:type rdf:resource="http://www.w3.org/1999/02/22-rdf-syntax-ns#Property"/>
</skos:Concept>
<skos:Concept rdf:about="http://rs.tdwg.org/dwc/terms/genus">
<skos:prefLabel xml:lang="en">Genus</skos:prefLabel>
<skos:definition xml:lang="en">The full scientific name of the
			genus
			in which the taxon is classified.</skos:definition>
<skos:example xml:lang="en">Example: "Puma",
			"Monoclea"</skos:example>
<skos:prefLabel xml:lang="es">Género</skos:prefLabel>
<skos:definition xml:lang="es">El nombre científico completo del
			género en el que se clasifica el taxón. </skos:definition>
<skos:example xml:lang="es">Ejemplo: "Puma", "Monoclea"</skos:example>
<skos:prefLabel xml:lang="zh-Hans">属</skos:prefLabel>
<skos:definition xml:lang="zh-Hans">分类单元所属属的完整学名。</skos:definition>
<skos:example xml:lang="zh-Hans"/>
<skos:prefLabel xml:lang="ja"/>
<skos:definition xml:lang="ja">その分類群が位置づけられている、分類上の「属」のフルネーム。</skos:definition>
<skos:example xml:lang="ja"/>
<skos:inScheme rdf:resource="http://rs.gbif.org/terms/dwc/dwc_translations.rdf"/>
<rdf:type rdf:resource="http://www.w3.org/1999/02/22-rdf-syntax-ns#Property"/>
</skos:Concept>
<skos:Concept rdf:about="http://rs.tdwg.org/dwc/terms/geodeticDatum">
<skos:prefLabel xml:lang="en">Geodetic Datum</skos:prefLabel>
<skos:definition xml:lang="en">The ellipsoid, geodetic datum, or
			spatial reference system (SRS) upon which the geographic coordinates
			given in decimalLatitude and decimalLongitude as based. Recommended
			best practice is use the EPSG code as a controlled vocabulary to
			provide an SRS, if known. Otherwise use a controlled vocabulary for
			the name or code of the geodetic datum, if known. Otherwise use a
			controlled vocabulary for the name or code of the ellipsoid, if
			known. If none of these is known, use the value "unknown".
		</skos:definition>
<skos:example xml:lang="en">Examples:
			"EPSG:4326", "WGS84", "NAD27",
			"Campo Inchauspe", "European 1950",
			"Clarke 1866"</skos:example>
<skos:prefLabel xml:lang="es">Datum geodésico</skos:prefLabel>
<skos:definition xml:lang="es">El elipsoide, datum geodésico, o
			sistema de referencia espacial (SRS) en el que se basan las
			coordenadas geográficas provistas en Latitud Decimal y Longitud
			Decimal. La práctica recomendada es usar el código EPSG como un
			lenguaje controlado para proporcionar un SRS, si se conoce. Caso
			contrario, utilice un lenguaje controlado para el nombre o código del
			datum geodésico, si se conoce. Caso contrario, utilice un lenguaje
			controlado para el nombre o código del elipsoide, si se conoce. Si
			nada de esto se sabe, utilice el valor "desconocido". </skos:definition>
<skos:example xml:lang="es">Ejemplo: "EPSG:4326", "WGS84", "NAD27",
			"Campo Inchauspe", "European 1950", "Clarke 1866"</skos:example>
<skos:prefLabel xml:lang="zh-Hans">大地基准</skos:prefLabel>
<skos:definition xml:lang="zh-Hans">椭圆体、大地基准点或空间参考系统的地理坐标以十进制经度和纬度为基础。建议最佳做法是如果已知EPSG编码，使用其作为控制性词汇规定一个空间参考系统。或者使用已知的控制性词汇作为大地基准点的名称或编码。或者使用已知的控制性词汇作为椭圆体的名称或编码。如果这些都未知，则使用“未知”值。</skos:definition>
<skos:example xml:lang="zh-Hans"/>
<skos:prefLabel xml:lang="ja"/>
<skos:definition xml:lang="ja">decimalLatitudeとdecimalLongitudeで与えられる地理座標についての楕円体、経緯度原点、空間参照システム。もしわかるのであれば、空間参照システムから提供されるEPSGコードなどの管理された語彙の使用が推奨される。そうでない場合は、経緯度原点の名前またはコードについての管理された語彙の使用が推奨される。それも困難であれば、楕円体についての名前またはコードについての管理された語彙の使用が推奨される。それも無理の場合は、"unknown"を使用する。</skos:definition>
<skos:example xml:lang="ja"/>
<skos:inScheme rdf:resource="http://rs.gbif.org/terms/dwc/dwc_translations.rdf"/>
<rdf:type rdf:resource="http://www.w3.org/1999/02/22-rdf-syntax-ns#Property"/>
</skos:Concept>
<skos:Concept rdf:about="http://rs.tdwg.org/dwc/terms/geologicalContextID">
<skos:prefLabel xml:lang="en">Geological Context ID</skos:prefLabel>
<skos:definition xml:lang="en">An identifier for the set of
			information associated with a GeologicalContext (the location within
			a geological context, such as stratigraphy). May be a global unique
			identifier or an identifier specific to the data set.</skos:definition>
<skos:example xml:lang="en"/>
<skos:prefLabel xml:lang="es">ID del contexto geológico</skos:prefLabel>
<skos:definition xml:lang="es">Un identificador para el conjunto de
			la información asociada con Contexto Geológico (la ubicación dentro
			de un contexto geológico, tal como la estratigrafía). Puede ser un
			identificador único global o un identificador específico para el
			conjunto de datos.</skos:definition>
<skos:example xml:lang="es"/>
<skos:prefLabel xml:lang="zh-Hans">地质环境编号</skos:prefLabel>
<skos:definition xml:lang="zh-Hans">与地质环境（有地质环境的地点，如地层）有关的信息集标识符。可能是一个全局唯一标识符或特定的数据集标识符。</skos:definition>
<skos:example xml:lang="zh-Hans"/>
<skos:prefLabel xml:lang="ja"/>
<skos:definition xml:lang="ja">GeologicalContext
			(地層など、地質学的文脈における位置）と関連した情報セットのID。GUIDまたは、そのデータセット固有のID。</skos:definition>
<skos:example xml:lang="ja"/>
<skos:inScheme rdf:resource="http://rs.gbif.org/terms/dwc/dwc_translations.rdf"/>
<rdf:type rdf:resource="http://www.w3.org/1999/02/22-rdf-syntax-ns#Property"/>
</skos:Concept>
<skos:Concept rdf:about="http://rs.tdwg.org/dwc/terms/georeferencedBy">
<skos:prefLabel xml:lang="en">Georeferenced By</skos:prefLabel>
<skos:definition xml:lang="en">A list (concatenated and
			separated) of
			names of people, groups, or organizations who
			determined the
			georeference (spatial representation) for the
			Location.</skos:definition>
<skos:example xml:lang="en">Example: "Kristina
			Yamamoto (MVZ); Janet Fang
			(MVZ)", "Brad Millen (ROM)"
		</skos:example>
<skos:prefLabel xml:lang="es">Georreferenciado por</skos:prefLabel>
<skos:definition xml:lang="es">Una lista (concatenada y separada) de
			los nombres de las personas, grupos u organizaciones que determinan
			la georreferencia (representación espacial) para la ubicación. </skos:definition>
<skos:example xml:lang="es">Ejemplo: "Kristina Yamamoto (MVZ); Janet
			Fang (MVZ)", "Brad Millen (ROM)"</skos:example>
<skos:prefLabel xml:lang="zh-Hans">确定地理参考者</skos:prefLabel>
<skos:definition xml:lang="zh-Hans">确定地点的地理参考（空间表述）的人名、群体或组织列表（连接的或分开的）。</skos:definition>
<skos:example xml:lang="zh-Hans"/>
<skos:prefLabel xml:lang="ja"/>
<skos:definition xml:lang="ja">その位置の地理参照
			(空間表現）を決定した人物、グループ、あるいは組織の名前のリスト。</skos:definition>
<skos:example xml:lang="ja"/>
<skos:inScheme rdf:resource="http://rs.gbif.org/terms/dwc/dwc_translations.rdf"/>
<rdf:type rdf:resource="http://www.w3.org/1999/02/22-rdf-syntax-ns#Property"/>
</skos:Concept>
<skos:Concept rdf:about="http://rs.tdwg.org/dwc/terms/georeferencedDate">
<skos:prefLabel xml:lang="en">Georeferenced Date</skos:prefLabel>
<skos:definition xml:lang="en">The date on which the Location was
			georeferenced. Recommended best practice is to use an encoding
			scheme, such as ISO 8601:2004(E).</skos:definition>
<skos:example xml:lang="en">Examples:
			"1963-03-08T14:07-0600" is 8 Mar
			1963 2:07pm in the time zone six
			hours earlier than UTC,
			"2009-02-20T08:40Z" is 20 Feb 2009 8:40am
			UTC, "1809-02-12" is 12 Feb
			1809, "1906-06" is Jun 1906, "1971" is
			just that year,
			"2007-03-01T13:00:00Z/2008-05-11T15:30:00Z" is the
			interval between 1
			Mar 2007 1pm UTC and 11 May 2008 3:30pm UTC,
			"2007-11-13/15" is the
			interval between 13 Nov 2007 and 15 Nov 2007.
		</skos:example>
<skos:prefLabel xml:lang="es">Fecha de la georreferenciación</skos:prefLabel>
<skos:definition xml:lang="es">La fecha en que fue georreferenciada
			la ubicación. La práctica recomendada es utilizar un esquema de
			codificación, tal como ISO 8601:2004 (E).</skos:definition>
<skos:example xml:lang="es">Ejemplo: "1963-03-08T14:07-0600" es 8 de
			marzo de 1963 2:07pm en zona horaria seis horas más temprano que UTC,
			"2009-02-20T08:40Z" es 20 de febrero 2009 8:40am UTC, "1809-02-12" es
			12 de febrero de 1809, "1906-06" es junio de 1906, "1971",
			"2007-03-01T13:00:00Z/2008-05-11T15:30:00Z" es el intervalo entre el
			1 de marzo de 2007 1pm UTC y 11 de mayo de 2008 3:30pm UTC,
			"2007-11-13/15" es el intervalo entre el 13 de noviembre de 2007 y 15
			de noviembre de 2007.</skos:example>
<skos:prefLabel xml:lang="zh-Hans">确定地理参考日期</skos:prefLabel>
<skos:definition xml:lang="zh-Hans">确定地点的地理参考的日期。建议最佳做法是使用一个编码方案，例如ISO
			8601:2004(E)。</skos:definition>
<skos:example xml:lang="zh-Hans"/>
<skos:prefLabel xml:lang="ja"/>
<skos:definition xml:lang="ja">その位置の地理参照が決定された日付。ISO
			8601:2004(E)などのスキーマの使用を推奨。</skos:definition>
<skos:example xml:lang="ja"/>
<skos:inScheme rdf:resource="http://rs.gbif.org/terms/dwc/dwc_translations.rdf"/>
<rdf:type rdf:resource="http://www.w3.org/1999/02/22-rdf-syntax-ns#Property"/>
</skos:Concept>
<skos:Concept rdf:about="http://rs.tdwg.org/dwc/terms/georeferenceProtocol">
<skos:prefLabel xml:lang="en">Georeference Protocol</skos:prefLabel>
<skos:definition xml:lang="en">A description or reference to the
			methods used to determine the spatial footprint, coordinates, and
			uncertainties.</skos:definition>
<skos:example xml:lang="en">Examples: "Guide to
			Best Practices for
			Georeferencing" (Chapman and Wieczorek, eds.
			2006), Global
			Biodiversity Information Facility.",
			"MaNIS/HerpNet/ORNIS
			Georeferencing Guidelines", "BioGeomancer"
		</skos:example>
<skos:prefLabel xml:lang="es">Protocolo de georreferenciación</skos:prefLabel>
<skos:definition xml:lang="es">Una descripción o referencia a los
			métodos utilizados para determinar el footprint espacial,
			coordenadas, e incertidumbres. </skos:definition>
<skos:example xml:lang="es">Ejemplos: "Guide to Best Practices for
			Georeferencing" (Chapman and Wieczorek, eds. 2006), Global
			Biodiversity Information Facility.", "MaNIS/HerpNet/ORNIS
			Georeferencing Guidelines", "BioGeomancer"</skos:example>
<skos:prefLabel xml:lang="zh-Hans">地理参考草案</skos:prefLabel>
<skos:definition xml:lang="zh-Hans">用来确定空间足迹、坐标和不确定性的方法描述或参考。</skos:definition>
<skos:example xml:lang="zh-Hans"/>
<skos:prefLabel xml:lang="ja"/>
<skos:definition xml:lang="ja">空間範囲、座標、および不確実性を決定するのに用いた手法に関する参考文献の記述。</skos:definition>
<skos:example xml:lang="ja"/>
<skos:inScheme rdf:resource="http://rs.gbif.org/terms/dwc/dwc_translations.rdf"/>
<rdf:type rdf:resource="http://www.w3.org/1999/02/22-rdf-syntax-ns#Property"/>
</skos:Concept>
<skos:Concept rdf:about="http://rs.tdwg.org/dwc/terms/georeferenceRemarks">
<skos:prefLabel xml:lang="en">Georeference Remarks</skos:prefLabel>
<skos:definition xml:lang="en">Notes or comments about the
			spatial
			description determination, explaining assumptions made in
			addition or
			opposition to the those formalized in the method referred
			to in
			georeferenceProtocol.</skos:definition>
<skos:example xml:lang="en">Example: "assumed
			distance by road (Hwy.
			101)"</skos:example>
<skos:prefLabel xml:lang="es">Comentarios de la georreferenciación</skos:prefLabel>
<skos:definition xml:lang="es">Anotaciones o comentarios acerca de la
			determinación de la descripción espacial, suposiciones explicativas
			adicionales o en oposición a las formalizadas en el método referido
			en Protocolo de Georreferenciación. </skos:definition>
<skos:example xml:lang="es">Ejemplo: "distancia supuesta del camino
			(Autopista 101)"</skos:example>
<skos:prefLabel xml:lang="zh-Hans">地理参考备注</skos:prefLabel>
<skos:definition xml:lang="zh-Hans">关于为补充或反对地理参考草案中提到的那些正式的方法所做的空间描述确定、解释假设的记录或评论。</skos:definition>
<skos:example xml:lang="zh-Hans"/>
<skos:prefLabel xml:lang="ja"/>
<skos:definition xml:lang="ja">空間の記述、決定に関しての注釈あるいはコメント。georeferenceProtocolにおいて形式化された手法に対して、追加的に、あるいはそれと対立して設けられた前提を説明するもの。</skos:definition>
<skos:example xml:lang="ja"/>
<skos:inScheme rdf:resource="http://rs.gbif.org/terms/dwc/dwc_translations.rdf"/>
<rdf:type rdf:resource="http://www.w3.org/1999/02/22-rdf-syntax-ns#Property"/>
</skos:Concept>
<skos:Concept rdf:about="http://rs.tdwg.org/dwc/terms/georeferenceSources">
<skos:prefLabel xml:lang="en">Georeference Sources</skos:prefLabel>
<skos:definition xml:lang="en">A list (concatenated and
			separated) of
			maps, gazetteers, or other resources used to
			georeference the
			Location, described specifically enough to allow
			anyone in the future
			to use the same resources.</skos:definition>
<skos:example xml:lang="en">Examples: "USGS
			1:24000 Florence Montana
			Quad; Terrametrics 2008 on Google Earth"
		</skos:example>
<skos:prefLabel xml:lang="es">Fuentes de la georreferenciación</skos:prefLabel>
<skos:definition xml:lang="es">Una lista (concatenada y separada) de
			los mapas, gaceteros, u otros recursos utilizados para
			georreferenciar la ubicación, que se describe lo suficiente
			específicamente como para permitir que cualquier persona en el futuro
			utilice los mismos recursos. </skos:definition>
<skos:example xml:lang="es">Ejemplo: "USGS 1:24000 Florence Montana
			Quad; Terrametrics 2008 en Google Earth"</skos:example>
<skos:prefLabel xml:lang="zh-Hans">地理参考源</skos:prefLabel>
<skos:definition xml:lang="zh-Hans">用于对地点进行地理参考标识的地图、地名表或其他资源列表，描述具体，足以让将来任何人使用相同的资源。</skos:definition>
<skos:example xml:lang="zh-Hans"/>
<skos:prefLabel xml:lang="ja"/>
<skos:definition xml:lang="ja">その位置の地理参照を決定するのに用いた、地図、地名集、あるいはその他の情報源のリスト。将来、誰かが同じ情報源を利用することができる程度に充分に記述されたもの。</skos:definition>
<skos:example xml:lang="ja"/>
<skos:inScheme rdf:resource="http://rs.gbif.org/terms/dwc/dwc_translations.rdf"/>
<rdf:type rdf:resource="http://www.w3.org/1999/02/22-rdf-syntax-ns#Property"/>
</skos:Concept>
<skos:Concept rdf:about="http://rs.tdwg.org/dwc/terms/georeferenceVerificationStatus">
<skos:prefLabel xml:lang="en">Georeference Verification Status
		</skos:prefLabel>
<skos:definition xml:lang="en">A categorical description of the
			extent to which the georeference has been verified to represent the
			best possible spatial description. Recommended best practice is to
			use a controlled vocabulary.</skos:definition>
<skos:example xml:lang="en">Examples: "requires
			verification", "verified
			by collector", "verified by curator".
		</skos:example>
<skos:prefLabel xml:lang="es">Estado de verificación de la georreferenciación</skos:prefLabel>
<skos:definition xml:lang="es">Una descripción categórica de la
			medida en que se ha verificado la georreferencia para representar, de
			la mejor manera, la descripción espacial. La práctica recomendada es
			el uso de un lenguaje controlado. </skos:definition>
<skos:example xml:lang="es">Ejemplo: "requiere verificación",
			"verificado por colector", "verificado por curador".</skos:example>
<skos:prefLabel xml:lang="zh-Hans">地理参考确认状态</skos:prefLabel>
<skos:definition xml:lang="zh-Hans">一个已证实代表最好的空间描述的地理参考范围的分类描述。建议最佳做法是使用一个控制性词汇。</skos:definition>
<skos:example xml:lang="zh-Hans"/>
<skos:prefLabel xml:lang="ja"/>
<skos:definition xml:lang="ja">その地理参照が、どの程度有効な空間記述であるかの分類。管理された語彙の使用を推奨。</skos:definition>
<skos:example xml:lang="ja"/>
<skos:inScheme rdf:resource="http://rs.gbif.org/terms/dwc/dwc_translations.rdf"/>
<rdf:type rdf:resource="http://www.w3.org/1999/02/22-rdf-syntax-ns#Property"/>
</skos:Concept>
<skos:Concept rdf:about="http://rs.tdwg.org/dwc/terms/group">
<skos:prefLabel xml:lang="en">Group</skos:prefLabel>
<skos:definition xml:lang="en">The full name of the
			lithostratigraphic group from which the cataloged item was collected.
		</skos:definition>
<skos:example xml:lang="en"/>
<skos:prefLabel xml:lang="es">Grupo</skos:prefLabel>
<skos:definition xml:lang="es">El nombre completo del grupo
			litoestratigráfico del cual se colectó el objeto catalogado. </skos:definition>
<skos:example xml:lang="es"/>
<skos:prefLabel xml:lang="zh-Hans">组</skos:prefLabel>
<skos:definition xml:lang="zh-Hans">采集编目项所在地层组的完整名称。</skos:definition>
<skos:example xml:lang="zh-Hans"/>
<skos:prefLabel xml:lang="ja"/>
<skos:definition xml:lang="ja">この項目が収集された岩相層序の層群のフルネーム。</skos:definition>
<skos:example xml:lang="ja"/>
<skos:inScheme rdf:resource="http://rs.gbif.org/terms/dwc/dwc_translations.rdf"/>
<rdf:type rdf:resource="http://www.w3.org/1999/02/22-rdf-syntax-ns#Property"/>
</skos:Concept>
<skos:Concept rdf:about="http://rs.tdwg.org/dwc/terms/habitat">
<skos:prefLabel xml:lang="en">Habitat</skos:prefLabel>
<skos:definition xml:lang="en">A category or description of the
			habitat in which the Event occurred.</skos:definition>
<skos:example xml:lang="en">Example: "oak
			savanna", "pre-cordilleran
			steppe"</skos:example>
<skos:prefLabel xml:lang="es">Hábitat</skos:prefLabel>
<skos:definition xml:lang="es">Una categoría o la descripción del
			hábitat en el que ocurrió el evento.</skos:definition>
<skos:example xml:lang="es">Ejemplo: "sabana de roble", "estepa de la
			pre-cordillera"</skos:example>
<skos:prefLabel xml:lang="zh-Hans">栖息地</skos:prefLabel>
<skos:definition xml:lang="zh-Hans">事件发生的栖息地的类别或描述。</skos:definition>
<skos:example xml:lang="zh-Hans"/>
<skos:prefLabel xml:lang="ja"/>
<skos:definition xml:lang="ja">そのイベントが発生した生息環境の分類または記述。</skos:definition>
<skos:example xml:lang="ja"/>
<skos:inScheme rdf:resource="http://rs.gbif.org/terms/dwc/dwc_translations.rdf"/>
<rdf:type rdf:resource="http://www.w3.org/1999/02/22-rdf-syntax-ns#Property"/>
</skos:Concept>
<skos:Concept rdf:about="http://rs.tdwg.org/dwc/terms/higherClassification">
<skos:prefLabel xml:lang="en">Higher Classification</skos:prefLabel>
<skos:definition xml:lang="en">A list (concatenated and
			separated) of
			taxa names terminating at the rank immediately superior
			to the taxon
			referenced in the taxon record. Recommended best
			practice is to order
			the list starting with the highest rank and
			separating the names for
			each rank with a semi-colon (";").
		</skos:definition>
<skos:example xml:lang="en">Example:
			"Animalia;Chordata;Vertebrata;Mammalia;Theria;Eutheria;Rodentia;Hystricognatha;Hystricognathi;Ctenomyidae;Ctenomyini;Ctenomys"
		</skos:example>
<skos:prefLabel xml:lang="es">Clasificación superior</skos:prefLabel>
<skos:definition xml:lang="es">Una lista (concatenada y separada) de
			los nombres de los taxones que terminan en el nivel inmediatamente
			superior al del taxón de referencia en el registro del taxón. La
			práctica recomendada es ordenar la lista comenzando con el más alto
			nivel y separando los nombres de cada nivel, con un punto y coma
			(";").</skos:definition>
<skos:example xml:lang="es">Ejemplo:
			"Animalia;Chordata;Vertebrata;Mammalia;Theria;Eutheria;Rodentia;Hystricognatha;Hystricognathi;Ctenomyidae;Ctenomyini;Ctenomys"</skos:example>
<skos:prefLabel xml:lang="zh-Hans">较高级分类</skos:prefLabel>
<skos:definition xml:lang="zh-Hans">优于分类记录中引用的类群、在等级排列中紧接在最后的类群名称列表（连接的或分开的）。建议最佳做法是从最高分类级别开始排列，用分号（";"）分隔每个等级名称。</skos:definition>
<skos:example xml:lang="zh-Hans"/>
<skos:prefLabel xml:lang="ja"/>
<skos:definition xml:lang="ja">系統レコードによって参照されている系統より一階層上の系統名のリスト。最上位の系統階層から記述を始め、系統名は;で区切ることを推奨する。</skos:definition>
<skos:example xml:lang="ja"/>
<skos:inScheme rdf:resource="http://rs.gbif.org/terms/dwc/dwc_translations.rdf"/>
<rdf:type rdf:resource="http://www.w3.org/1999/02/22-rdf-syntax-ns#Property"/>
</skos:Concept>
<skos:Concept rdf:about="http://rs.tdwg.org/dwc/terms/higherGeography">
<skos:prefLabel xml:lang="en">Higher Geography</skos:prefLabel>
<skos:definition xml:lang="en">A list (concatenated and
			separated) of
			geographic names less specific than the information
			captured in the
			locality term.</skos:definition>
<skos:example xml:lang="en">Example: "South
			America; Argentina;
			Patagonia; Parque Nacional Nahuel Huapi; Neuquén;
			Los Lagos" with
			accompanying values "South America" in Continent,
			"Argentina" in
			Country, "Neuquén" in StateProvince, and Los Lagos in
			County.</skos:example>
<skos:prefLabel xml:lang="es">Geografía superior</skos:prefLabel>
<skos:definition xml:lang="es">Una lista (concatenada y separada) de
			los nombres geográficos menos específicos que la información
			capturada en el elemento de Localidad.</skos:definition>
<skos:example xml:lang="es">Ejemplo: "Sudamérica; Argentina; Patagonia;
			Parque Nacional Nahuel Huapi; Neuquén; Los Lagos" con valores
			acompañantes "Sudamérica" en Continente, "Argentina" en País,
			"Neuquén" en Estado/Provincia, y Los Lagos en Condado.</skos:example>
<skos:prefLabel xml:lang="zh-Hans">较高一级地区</skos:prefLabel>
<skos:definition xml:lang="zh-Hans">与在当地长期获得的信息相比不够具体的地名列表（连接的或分开的）。</skos:definition>
<skos:example xml:lang="zh-Hans"/>
<skos:prefLabel xml:lang="ja"/>
<skos:definition xml:lang="ja">地域的な用語で得られる情報よりも、もう少し漠然とした地理的名称のリスト。</skos:definition>
<skos:example xml:lang="ja"/>
<skos:inScheme rdf:resource="http://rs.gbif.org/terms/dwc/dwc_translations.rdf"/>
<rdf:type rdf:resource="http://www.w3.org/1999/02/22-rdf-syntax-ns#Property"/>
</skos:Concept>
<skos:Concept rdf:about="http://rs.tdwg.org/dwc/terms/higherGeographyID">
<skos:prefLabel xml:lang="en">Higher Geography ID</skos:prefLabel>
<skos:definition xml:lang="en">An identifier for the geographic
			region within which the Location occurred. Recommended best practice
			is to use an persistent identifier from a controlled vocabulary such
			as the Getty Thesaurus of Geographic Names.</skos:definition>
<skos:example xml:lang="en">Example: "TGN:
			1002002" for Prov. Tierra del
			Fuego, Argentina</skos:example>
<skos:prefLabel xml:lang="es">ID de la geografía superior</skos:prefLabel>
<skos:definition xml:lang="es">Un identificador de la región
			geográfica de la ubicación. La práctica recomendada es utilizar un
			identificador persistente de un lenguaje controlado como el Tesauro
			Getty de Nombres Geográficos. </skos:definition>
<skos:example xml:lang="es">Ejemplo: "TGN: 1002002" para Provincia
			Tierra del Fuego, Argentina</skos:example>
<skos:prefLabel xml:lang="zh-Hans">较高一级地区编号</skos:prefLabel>
<skos:definition xml:lang="zh-Hans">地点所在地理区域的标识符。建议最佳做法是使用一个控制性词汇中的持久标识符，如地名盖蒂词库。</skos:definition>
<skos:example xml:lang="zh-Hans"/>
<skos:prefLabel xml:lang="ja"/>
<skos:definition xml:lang="ja">その位置の地域のID。Getty Thesaurus
			of Geographic Namesなど、管理された語彙による永続的なIDの利用を推奨。</skos:definition>
<skos:example xml:lang="ja"/>
<skos:inScheme rdf:resource="http://rs.gbif.org/terms/dwc/dwc_translations.rdf"/>
<rdf:type rdf:resource="http://www.w3.org/1999/02/22-rdf-syntax-ns#Property"/>
</skos:Concept>
<skos:Concept rdf:about="http://rs.tdwg.org/dwc/terms/highestBiostratigraphicZone">
<skos:prefLabel xml:lang="en">Highest Biostratigraphic Zone
		</skos:prefLabel>
<skos:definition xml:lang="en">The full name of the highest
			possible
			geological biostratigraphic zone of the stratigraphic
			horizon from
			which the cataloged item was collected.</skos:definition>
<skos:example xml:lang="en"/>
<skos:prefLabel xml:lang="es">Zona bioestratigráfica superior</skos:prefLabel>
<skos:definition xml:lang="es">El nombre completo de la zona
			geológica bioestratigráfica más alta posible del horizonte
			estratigráfico donde se recolectó el objeto catalogado. </skos:definition>
<skos:example xml:lang="es"/>
<skos:prefLabel xml:lang="zh-Hans">最高生物地层区</skos:prefLabel>
<skos:definition xml:lang="zh-Hans">采集编目项所在地层地平线的可能最高的地质生物地层区的完整名称。</skos:definition>
<skos:example xml:lang="zh-Hans"/>
<skos:prefLabel xml:lang="ja"/>
<skos:definition xml:lang="ja">この項目が収集された層位の、あり得る最上部の地質学的な生層序学的区分のフルネーム。</skos:definition>
<skos:example xml:lang="ja"/>
<skos:inScheme rdf:resource="http://rs.gbif.org/terms/dwc/dwc_translations.rdf"/>
<rdf:type rdf:resource="http://www.w3.org/1999/02/22-rdf-syntax-ns#Property"/>
</skos:Concept>
<skos:Concept rdf:about="http://rs.tdwg.org/dwc/terms/identificationID">
<skos:prefLabel xml:lang="en">Identification ID</skos:prefLabel>
<skos:definition xml:lang="en">An identifier for the
			Identification
			(the body of information associated with the
			assignment of a
			scientific name). May be a global unique identifier
			or an identifier
			specific to the data set.</skos:definition>
<skos:example xml:lang="en"/>
<skos:prefLabel xml:lang="es">ID de la identificación</skos:prefLabel>
<skos:definition xml:lang="es">Un identificador para la
			identificación (el cuerpo de la información asociada con la
			asignación de un nombre científico). Puede ser un identificador único
			global o un identificador específico para el conjunto de datos. </skos:definition>
<skos:example xml:lang="es"/>
<skos:prefLabel xml:lang="zh-Hans">鉴定编号</skos:prefLabel>
<skos:definition xml:lang="zh-Hans">鉴定标识符（与分配学名相关的信息主体）。可能是一个全局唯一标识符或特定的数据集标识符。
		</skos:definition>
<skos:example xml:lang="zh-Hans"/>
<skos:prefLabel xml:lang="ja"/>
<skos:definition xml:lang="ja">同定（学名の同定に関連した情報の集合）のID。GUIDまたは、そのデータセットに固有のID。</skos:definition>
<skos:example xml:lang="ja"/>
<skos:inScheme rdf:resource="http://rs.gbif.org/terms/dwc/dwc_translations.rdf"/>
<rdf:type rdf:resource="http://www.w3.org/1999/02/22-rdf-syntax-ns#Property"/>
</skos:Concept>
<skos:Concept rdf:about="http://rs.tdwg.org/dwc/terms/identificationQualifier">
<skos:prefLabel xml:lang="en">Identification Qualifier</skos:prefLabel>
<skos:definition xml:lang="en">A brief phrase or a standard term
			("cf.", "aff.") to express the determiner's doubts about the
			Identification.</skos:definition>
<skos:example xml:lang="en">Examples: 1) For the
			determination "Quercus
			aff. agrifolia var. oxyadenia",
			identificationQualifier would be "aff.
			agrifolia var. oxyadenia" with
			accompanying values "Quercus" in genus,
			"agrifolia" in
			specificEpithet, "oxyadenia" in infraspecificEpithet,
			and "var." in
			rank. 2) For the determination "Quercus agrifolia cf.
			var.
			oxyadenia", identificationQualifier would be "cf. var. oxyadenia
			"
			with accompanying values "Quercus" in genus, "agrifolia" in
			specificEpithet, "oxyadenia" in infraspecificEpithet, and "var." in
			rank.</skos:example>
<skos:prefLabel xml:lang="es">Calificador de la identificación</skos:prefLabel>
<skos:definition xml:lang="es">Una breve frase o término estándar
			("cf." ,"aff.") para expresar las dudas del determinador sobre la
			identificación. </skos:definition>
<skos:example xml:lang="es">Ejemplo: 1) Para la determinación "Quercus
			aff. agrifolia var. oxyadenia", Calificador de la Identificación
			sería "aff. agrifolia var. oxyadenia" con valores acompañantes
			"Quercus" en género, "agrifolia" en Epíteto Específico, "oxyadenia"
			en Epíteto Infraspecífico, y "var." en nivel. 2) Para la
			determinación "Quercus agrifolia cf. var. oxyadenia", Calificador
			Identificación sería "cf. var. oxyadenia " con valores acompañantes
			"Quercus" en género, "agrifolia" en Epíteto Específico, "oxyadenia"
			en Epíteto Infraspecífico, y "var." en nivel.</skos:example>
<skos:prefLabel xml:lang="zh-Hans">鉴定合格者</skos:prefLabel>
<skos:definition xml:lang="zh-Hans">鉴定者对结果表示疑虑的一个简单短语或一个标准术语("cf.",
			"aff.")。</skos:definition>
<skos:example xml:lang="zh-Hans"/>
<skos:prefLabel xml:lang="ja"/>
<skos:definition xml:lang="ja">同定に関して、確実ではない、ということを表現するための簡潔な語句、または標準的な用語（“cf.“や“aff.“など）。</skos:definition>
<skos:example xml:lang="ja"/>
<skos:inScheme rdf:resource="http://rs.gbif.org/terms/dwc/dwc_translations.rdf"/>
<rdf:type rdf:resource="http://www.w3.org/1999/02/22-rdf-syntax-ns#Property"/>
</skos:Concept>
<skos:Concept rdf:about="http://rs.tdwg.org/dwc/terms/identificationReferences">
<skos:prefLabel xml:lang="en">Identification References</skos:prefLabel>
<skos:definition xml:lang="en">A list (concatenated and
			separated) of
			references (publication, global unique identifier, URI)
			used in the
			Identification.</skos:definition>
<skos:example xml:lang="en">Example: "Aves del
			Noroeste Patagonico.
			Christie et al. 2004."</skos:example>
<skos:prefLabel xml:lang="es">Referencias de la identificación</skos:prefLabel>
<skos:definition xml:lang="es">Una lista (concatenada y separada) de
			las referencias (publicación, identificador único global, URI)
			utilizadas en la identificación. </skos:definition>
<skos:example xml:lang="es">Ejemplo: "Aves del Noroeste Patagónico.
			Christie et al. 2004."</skos:example>
<skos:prefLabel xml:lang="zh-Hans">鉴定参考</skos:prefLabel>
<skos:definition xml:lang="zh-Hans">鉴定中使用的参考（出版物，全球唯一标识符，网站资源）列表（连接的或分开的）。</skos:definition>
<skos:example xml:lang="zh-Hans"/>
<skos:prefLabel xml:lang="ja"/>
<skos:definition xml:lang="ja">同定に用いた参考文献（出版物、GUID、URIなど）のリスト。</skos:definition>
<skos:example xml:lang="ja"/>
<skos:inScheme rdf:resource="http://rs.gbif.org/terms/dwc/dwc_translations.rdf"/>
<rdf:type rdf:resource="http://www.w3.org/1999/02/22-rdf-syntax-ns#Property"/>
</skos:Concept>
<skos:Concept rdf:about="http://rs.tdwg.org/dwc/terms/identificationRemarks">
<skos:prefLabel xml:lang="en">Identification Remarks</skos:prefLabel>
<skos:definition xml:lang="en">Comments or notes about the
			Identification.</skos:definition>
<skos:example xml:lang="en">Example:
			"Distinguished between Anthus
			correndera and Anthus hellmayri based
			on the comparative lengths of
			the uñas."</skos:example>
<skos:prefLabel xml:lang="es">Comentarios de la identificación</skos:prefLabel>
<skos:definition xml:lang="es">Comentarios o anotaciones sobre la
			identificación. </skos:definition>
<skos:example xml:lang="es">Ejemplo: Se distingue entre Anthus
			correndera y Anthus hellmayri basado en las longitudes comparativas
			de las uñas.</skos:example>
<skos:prefLabel xml:lang="zh-Hans">鉴定备注</skos:prefLabel>
<skos:definition xml:lang="zh-Hans">有关鉴定的评论或记录。</skos:definition>
<skos:example xml:lang="zh-Hans"/>
<skos:prefLabel xml:lang="ja"/>
<skos:definition xml:lang="ja">同定に関するコメントまたは注釈。</skos:definition>
<skos:example xml:lang="ja"/>
<skos:inScheme rdf:resource="http://rs.gbif.org/terms/dwc/dwc_translations.rdf"/>
<rdf:type rdf:resource="http://www.w3.org/1999/02/22-rdf-syntax-ns#Property"/>
</skos:Concept>
<skos:Concept rdf:about="http://rs.tdwg.org/dwc/terms/identificationVerificationStatus">
<skos:prefLabel xml:lang="en">Identification Verification Status
		</skos:prefLabel>
<skos:definition xml:lang="en">A categorical indicator of the
			extent
			to which the taxonomic identification has been verified to be
			correct. Recommended best practice is to use a controlled vocabulary
			such as that used in HISPID/ABCD.</skos:definition>
<skos:example xml:lang="en">Examples: "0", "4"
		</skos:example>
<skos:prefLabel xml:lang="es">Estado de la verificación de la identificación</skos:prefLabel>
<skos:definition xml:lang="es">Un indicador categórico del alcance de
			la verificación de la identificación taxonómica. La práctica
			recomendada es el uso de un lenguaje controlado.</skos:definition>
<skos:example xml:lang="es">Ejemplos: "0", "4"</skos:example>
<skos:prefLabel xml:lang="zh-Hans">鉴定确认状态</skos:prefLabel>
<skos:definition xml:lang="zh-Hans">分类鉴定结果经核实为正确的确切范围指标。建议最佳做法是使用一个例如用在HISPID/ABCD中的控制性词汇。</skos:definition>
<skos:example xml:lang="zh-Hans"/>
<skos:prefLabel xml:lang="ja"/>
<skos:definition xml:lang="ja">系統分類の正しさがどの程度検証されているのかを示す指標。
			HISPID/ABCD などの管理された語彙の使用を推奨。</skos:definition>
<skos:example xml:lang="ja"/>
<skos:inScheme rdf:resource="http://rs.gbif.org/terms/dwc/dwc_translations.rdf"/>
<rdf:type rdf:resource="http://www.w3.org/1999/02/22-rdf-syntax-ns#Property"/>
</skos:Concept>
<skos:Concept rdf:about="http://rs.tdwg.org/dwc/terms/identifiedBy">
<skos:prefLabel xml:lang="en">Identified By</skos:prefLabel>
<skos:definition xml:lang="en">A list (concatenated and
			separated) of
			names of people, groups, or organizations who assigned
			the Taxon to
			the subject.</skos:definition>
<skos:example xml:lang="en">Example: "James L.
			Patton", "Theodore
			Pappenfuss; Robert Macey"</skos:example>
<skos:prefLabel xml:lang="es">Identificado por</skos:prefLabel>
<skos:definition xml:lang="es">Una lista (concatenada y separada) de
			los nombres de las personas, grupos u organizaciones que asignaron el
			taxón al sujeto. </skos:definition>
<skos:example xml:lang="es">Ejemplo: "James L. Patton", "Theodore
			Pappenfuss; Robert Macey"</skos:example>
<skos:prefLabel xml:lang="zh-Hans">鉴定者</skos:prefLabel>
<skos:definition xml:lang="zh-Hans">鉴定未知对象为相关类群的人名、群体或组织列表（连接的或分开的）。</skos:definition>
<skos:example xml:lang="zh-Hans"/>
<skos:prefLabel xml:lang="ja"/>
<skos:definition xml:lang="ja">対象の系統分類を行った人物、グループ、あるいは組織の名前のリスト。</skos:definition>
<skos:example xml:lang="ja"/>
<skos:inScheme rdf:resource="http://rs.gbif.org/terms/dwc/dwc_translations.rdf"/>
<rdf:type rdf:resource="http://www.w3.org/1999/02/22-rdf-syntax-ns#Property"/>
</skos:Concept>
<skos:Concept rdf:about="http://rs.tdwg.org/dwc/terms/individualCount">
<skos:prefLabel xml:lang="en">Individual Count</skos:prefLabel>
<skos:definition xml:lang="en">The number of individuals
			represented
			present at the time of the Occurrence.</skos:definition>
<skos:example xml:lang="en">Examples: "1", "25"
		</skos:example>
<skos:prefLabel xml:lang="es">Conteo de individuos</skos:prefLabel>
<skos:definition xml:lang="es">El número de individuos representados
			presente en el momento del Registro Biológico. </skos:definition>
<skos:example xml:lang="es">Ejemplo: "1", "25"</skos:example>
<skos:prefLabel xml:lang="zh-Hans">个体计数</skos:prefLabel>
<skos:definition xml:lang="zh-Hans">当前发生时间参加的个体数量。</skos:definition>
<skos:example xml:lang="zh-Hans"/>
<skos:prefLabel xml:lang="ja"/>
<skos:definition xml:lang="ja">その時、その場に存在していた個体の数。</skos:definition>
<skos:example xml:lang="ja"/>
<skos:inScheme rdf:resource="http://rs.gbif.org/terms/dwc/dwc_translations.rdf"/>
<rdf:type rdf:resource="http://www.w3.org/1999/02/22-rdf-syntax-ns#Property"/>
</skos:Concept>
<skos:Concept rdf:about="http://rs.tdwg.org/dwc/terms/individualID">
<skos:prefLabel xml:lang="en">Individual ID</skos:prefLabel>
<skos:definition xml:lang="en">An identifier for an individual or
			named group of individual organisms represented in the Occurrence.
			Meant to accommodate resampling of the same individual or group for
			monitoring purposes. May be a global unique identifier or an
			identifier specific to a data set.</skos:definition>
<skos:example xml:lang="en">Examples: "U.amer.
			44", "Smedley", "Orca J
			23"</skos:example>
<skos:prefLabel xml:lang="es">ID del individuo</skos:prefLabel>
<skos:definition xml:lang="es">Un identificador para un individuo o
			grupo de organismos individuales representados en el Registro
			Biológico. Destinado a alojar remuestreo del mismo individuo o grupo
			con fines de monitoreo. Puede ser un identificador único global o un
			identificador específico para un conjunto de datos.</skos:definition>
<skos:example xml:lang="es">Ejemplo: "U.amer. 44", "Smedley", "Orca J
			23"</skos:example>
<skos:prefLabel xml:lang="zh-Hans">个体编号</skos:prefLabel>
<skos:definition xml:lang="zh-Hans">事件中展现的个体标识符或生物个体命名组。为以后对相同个体或组群重新采样进行检测提供方便。可能是一个全局唯一标识符或特定数据集标识符。</skos:definition>
<skos:example xml:lang="zh-Hans"/>
<skos:prefLabel xml:lang="ja"/>
<skos:definition xml:lang="ja">個々の生物の個体またはグループのID。同じ個体またはグループをモニタリング目的でもう一度サンプル出来ることを目的としている。GUIDかデータセット固有のIDなどが期待される。</skos:definition>
<skos:example xml:lang="ja"/>
<skos:inScheme rdf:resource="http://rs.gbif.org/terms/dwc/dwc_translations.rdf"/>
<rdf:type rdf:resource="http://www.w3.org/1999/02/22-rdf-syntax-ns#Property"/>
</skos:Concept>
<skos:Concept rdf:about="http://rs.tdwg.org/dwc/terms/informationWithheld">
<skos:prefLabel xml:lang="en">Information Withheld</skos:prefLabel>
<skos:definition xml:lang="en">Additional information that
			exists, but
			that has not been shared in the given record.
		</skos:definition>
<skos:example xml:lang="en">Examples: "location
			information not given for
			endangered species", "collector identities
			withheld", "ask about
			tissue samples"</skos:example>
<skos:prefLabel xml:lang="es">Información retenida</skos:prefLabel>
<skos:definition xml:lang="es">Información adicional que existe, pero
			que no ha sido compartida en el registro dado. </skos:definition>
<skos:example xml:lang="es">Ejemplo: "la información de ubicación no es
			provista para especies amenazadas", "la identidad de los colectores
			retenida", "pregunte acerca de muestras de tejido"</skos:example>
<skos:prefLabel xml:lang="zh-Hans">信息隐瞒</skos:prefLabel>
<skos:definition xml:lang="zh-Hans">存在附加信息，但没有在给定记录中共享。</skos:definition>
<skos:example xml:lang="zh-Hans"/>
<skos:prefLabel xml:lang="ja"/>
<skos:definition xml:lang="ja">そのレコード内に存在するが、共有はされない追加的な情報。</skos:definition>
<skos:example xml:lang="ja"/>
<skos:inScheme rdf:resource="http://rs.gbif.org/terms/dwc/dwc_translations.rdf"/>
<rdf:type rdf:resource="http://www.w3.org/1999/02/22-rdf-syntax-ns#Property"/>
</skos:Concept>
<skos:Concept rdf:about="http://rs.tdwg.org/dwc/terms/infraspecificEpithet">
<skos:prefLabel xml:lang="en">Infraspecific Epithet</skos:prefLabel>
<skos:definition xml:lang="en">The name of the lowest or terminal
			infraspecific epithet of the scientificName, excluding any rank
			designation.</skos:definition>
<skos:example xml:lang="en">Example: "concolor",
			"oxyadenia", "sayi"</skos:example>
<skos:prefLabel xml:lang="es">Epíteto infraespecífico</skos:prefLabel>
<skos:definition xml:lang="es">El nombre del epíteto infraespecífico
			más bajo o terminal del Nombre Científico, excluyendo cualquier otra
			denominación de nivel. </skos:definition>
<skos:example xml:lang="es">Ejemplo: "concolor", "oxyadenia", "sayi"</skos:example>
<skos:prefLabel xml:lang="zh-Hans">种内名称</skos:prefLabel>
<skos:definition xml:lang="zh-Hans">学名的最低等级或末端的种内别名，不包括任何等级名称。</skos:definition>
<skos:example xml:lang="zh-Hans"/>
<skos:prefLabel xml:lang="ja"/>
<skos:definition xml:lang="ja">最下層の、あるいは種以下の学名の別名。階層指示記号は除く。</skos:definition>
<skos:example xml:lang="ja"/>
<skos:inScheme rdf:resource="http://rs.gbif.org/terms/dwc/dwc_translations.rdf"/>
<rdf:type rdf:resource="http://www.w3.org/1999/02/22-rdf-syntax-ns#Property"/>
</skos:Concept>
<skos:Concept rdf:about="http://rs.tdwg.org/dwc/terms/institutionCode">
<skos:prefLabel xml:lang="en">Institution Code</skos:prefLabel>
<skos:definition xml:lang="en">The name (or acronym) in use by
			the
			institution having custody of the object(s) or information
			referred to
			in the record.</skos:definition>
<skos:example xml:lang="en">Examples: "MVZ",
			"FMNH", "AKN-CLO",
			"University of California Museum of Paleontology
			(UCMP)"</skos:example>
<skos:prefLabel xml:lang="es">Código de la institución</skos:prefLabel>
<skos:definition xml:lang="es">El nombre (o acrónimo) en uso por la
			institución que tenga la custodia del objeto(s) o información
			mencionada en el registro. </skos:definition>
<skos:example xml:lang="es">Ejemplo: "MVZ", "FMNH", "AKN-CLO",
			"University of California Museum of Paleontology (UCMP)"</skos:example>
<skos:prefLabel xml:lang="zh-Hans">机构编码</skos:prefLabel>
<skos:definition xml:lang="zh-Hans">记录中提到有保管的物品或资料的机构所使用的名称（或首字母缩略词）。</skos:definition>
<skos:example xml:lang="zh-Hans"/>
<skos:prefLabel xml:lang="ja"/>
<skos:definition xml:lang="ja">そのレコードの物あるいは情報を管理している機関の名前（または頭字語）。</skos:definition>
<skos:example xml:lang="ja"/>
<skos:inScheme rdf:resource="http://rs.gbif.org/terms/dwc/dwc_translations.rdf"/>
<rdf:type rdf:resource="http://www.w3.org/1999/02/22-rdf-syntax-ns#Property"/>
</skos:Concept>
<skos:Concept rdf:about="http://rs.tdwg.org/dwc/terms/institutionID">
<skos:prefLabel xml:lang="en">Institution ID</skos:prefLabel>
<skos:definition xml:lang="en">An identifier for the institution
			having custody of the object(s) or information referred to in the
			record.</skos:definition>
<skos:example xml:lang="en"/>
<skos:prefLabel xml:lang="es">ID de la institución</skos:prefLabel>
<skos:definition xml:lang="es">Un identificador de la institución que
			custodia el objeto(s) o información mencionada en el registro. </skos:definition>
<skos:example xml:lang="es"/>
<skos:prefLabel xml:lang="zh-Hans">机构编号</skos:prefLabel>
<skos:definition xml:lang="zh-Hans">记录中提到有保管的物品或资料的机构的标识符。</skos:definition>
<skos:example xml:lang="zh-Hans"/>
<skos:prefLabel xml:lang="ja"/>
<skos:definition xml:lang="ja">そのレコードの物あるいは情報を管理している機関のID。</skos:definition>
<skos:example xml:lang="ja"/>
<skos:inScheme rdf:resource="http://rs.gbif.org/terms/dwc/dwc_translations.rdf"/>
<rdf:type rdf:resource="http://www.w3.org/1999/02/22-rdf-syntax-ns#Property"/>
</skos:Concept>
<skos:Concept rdf:about="http://rs.tdwg.org/dwc/terms/island">
<skos:prefLabel xml:lang="en">Island</skos:prefLabel>
<skos:definition xml:lang="en">The name of the island on or near
			which the Location occurs. Recommended best practice is to use a
			controlled vocabulary such as the Getty Thesaurus of Geographic
			Names.</skos:definition>
<skos:example xml:lang="en">Example: "Isla
			Victoria"</skos:example>
<skos:prefLabel xml:lang="es">Isla</skos:prefLabel>
<skos:definition xml:lang="es">El nombre de la isla en o cerca de la
			ubicación. La práctica recomendada es utilizar un identificador
			persistente de un lenguaje controlado como el Tesauro Getty de
			Nombres Geográficos.</skos:definition>
<skos:example xml:lang="es">Ejemplo: "Isla Victoria"</skos:example>
<skos:prefLabel xml:lang="zh-Hans">岛屿</skos:prefLabel>
<skos:definition xml:lang="zh-Hans">事件发生地点或附近的岛屿名称。建议最佳做法是使用一个控制性词汇，如地名盖蒂词库。</skos:definition>
<skos:example xml:lang="zh-Hans"/>
<skos:prefLabel xml:lang="ja"/>
<skos:definition xml:lang="ja">その位置が存在する、あるいは近接する島の名前。the Getty
			Thesaurus of Geographic Names のような、管理された語彙の使用を推奨。</skos:definition>
<skos:example xml:lang="ja"/>
<skos:inScheme rdf:resource="http://rs.gbif.org/terms/dwc/dwc_translations.rdf"/>
<rdf:type rdf:resource="http://www.w3.org/1999/02/22-rdf-syntax-ns#Property"/>
</skos:Concept>
<skos:Concept rdf:about="http://rs.tdwg.org/dwc/terms/islandGroup">
<skos:prefLabel xml:lang="en">Island Group</skos:prefLabel>
<skos:definition xml:lang="en">The name of the island group in
			which
			the Location occurs. Recommended best practice is to use a
			controlled
			vocabulary such as the Getty Thesaurus of Geographic
			Names.</skos:definition>
<skos:example xml:lang="en">Example: "Alexander
			Archipelago"</skos:example>
<skos:prefLabel xml:lang="es">Grupo de islas</skos:prefLabel>
<skos:definition xml:lang="es">El nombre del grupo de islas de la
			ubicación. La práctica recomendada es utilizar un identificador
			persistente de un lenguaje controlado como el Tesauro Getty de
			Nombres Geográficos.</skos:definition>
<skos:example xml:lang="es">Ejemplo: "Archipiélago Alexander"</skos:example>
<skos:prefLabel xml:lang="zh-Hans">岛群</skos:prefLabel>
<skos:definition xml:lang="zh-Hans">事件发生地点的岛群名称。建议最佳做法是使用一个控制性词汇，如地名盖蒂词库。</skos:definition>
<skos:example xml:lang="zh-Hans"/>
<skos:prefLabel xml:lang="ja"/>
<skos:definition xml:lang="ja">その位置が存在する諸島の名前。the Getty Thesaurus of
			Geographic Names のような、管理された語彙の使用を推奨。</skos:definition>
<skos:example xml:lang="ja"/>
<skos:inScheme rdf:resource="http://rs.gbif.org/terms/dwc/dwc_translations.rdf"/>
<rdf:type rdf:resource="http://www.w3.org/1999/02/22-rdf-syntax-ns#Property"/>
</skos:Concept>
<skos:Concept rdf:about="http://rs.tdwg.org/dwc/terms/kingdom">
<skos:prefLabel xml:lang="en">Kingdom</skos:prefLabel>
<skos:definition xml:lang="en">The full scientific name of the
			kingdom in which the taxon is classified.</skos:definition>
<skos:example xml:lang="en">Example: "Animalia",
			"Plantae"</skos:example>
<skos:prefLabel xml:lang="es">Reino</skos:prefLabel>
<skos:definition xml:lang="es">El nombre científico completo del
			reino en el que se clasifica el taxón. </skos:definition>
<skos:example xml:lang="es">Ejemplo: "Animalia", "Plantae"</skos:example>
<skos:prefLabel xml:lang="zh-Hans">界</skos:prefLabel>
<skos:definition xml:lang="zh-Hans">分类单元所属界的完整学名。</skos:definition>
<skos:example xml:lang="zh-Hans"/>
<skos:prefLabel xml:lang="ja"/>
<skos:definition xml:lang="ja">その分類群が位置づけられている、分類上の「界」のフルネーム。</skos:definition>
<skos:example xml:lang="ja"/>
<skos:inScheme rdf:resource="http://rs.gbif.org/terms/dwc/dwc_translations.rdf"/>
<rdf:type rdf:resource="http://www.w3.org/1999/02/22-rdf-syntax-ns#Property"/>
</skos:Concept>
<skos:Concept rdf:about="http://rs.tdwg.org/dwc/terms/latestAgeOrHighestStage">
<skos:prefLabel xml:lang="en">Latest AgeOr Highest Stage
		</skos:prefLabel>
<skos:definition xml:lang="en">The full name of the latest
			possible
			geochronologic age or highest chronostratigraphic stage
			attributable
			to the stratigraphic horizon from which the cataloged
			item was
			collected.</skos:definition>
<skos:example xml:lang="en">Examples:
			"Atlantic", "Boreal",
			"Skullrockian"</skos:example>
<skos:prefLabel xml:lang="es">Edad tardía o estadío superior</skos:prefLabel>
<skos:definition xml:lang="es">El nombre completo de la edad
			geocronológica más tardía posible o etapa cronoestratigráfica más
			alta, atribuible al horizonte estratigráfico donde se recolectó el
			objeto catalogado. </skos:definition>
<skos:example xml:lang="es">Ejemplos: "Atlántico", "Boreal"</skos:example>
<skos:prefLabel xml:lang="zh-Hans">最晚地质年代或最高年代地层</skos:prefLabel>
<skos:definition xml:lang="zh-Hans">采集编目项所在地层地平线的可能最晚的地质年代或最高年代地层的完整名称。</skos:definition>
<skos:example xml:lang="zh-Hans"/>
<skos:prefLabel xml:lang="ja"/>
<skos:definition xml:lang="ja">この項目が収集された層位が帰属している、あり得る最新の地質年代学的期、または最上部の年代層序的階のフルネーム。</skos:definition>
<skos:example xml:lang="ja"/>
<skos:inScheme rdf:resource="http://rs.gbif.org/terms/dwc/dwc_translations.rdf"/>
<rdf:type rdf:resource="http://www.w3.org/1999/02/22-rdf-syntax-ns#Property"/>
</skos:Concept>
<skos:Concept rdf:about="http://rs.tdwg.org/dwc/terms/latestEonOrHighestEonothem">
<skos:prefLabel xml:lang="en">Latest Eon Or Highest Eonothem
		</skos:prefLabel>
<skos:definition xml:lang="en">The full name of the latest
			possible
			geochronologic eon or highest chrono-stratigraphic eonothem
			or the
			informal name ("Precambrian") attributable to the
			stratigraphic
			horizon from which the cataloged item was collected.
		</skos:definition>
<skos:example xml:lang="en">Examples:
			"Phanerozoic", "Proterozoic"</skos:example>
<skos:prefLabel xml:lang="es">Eón tardío o eonotema superior</skos:prefLabel>
<skos:definition xml:lang="es">El nombre completo del eón
			geocronológico más tardío o el eratema crono-estratigráfico más alto
			posible, o el nombre informal ("Precámbrico") atribuible al horizonte
			estratigráfico donde se recolectó el objeto catalogado. </skos:definition>
<skos:example xml:lang="es">Ejemplo: "Fanerozoico", "Proterozoico".</skos:example>
<skos:prefLabel xml:lang="zh-Hans">最晚地质宙或最高地层宇</skos:prefLabel>
<skos:definition xml:lang="zh-Hans">采集编目项所在地层地平线的可能最晚的地质宙或最高地层宇或非正式名称（“前寒武纪”）的完整名称。</skos:definition>
<skos:example xml:lang="zh-Hans"/>
<skos:prefLabel xml:lang="ja"/>
<skos:definition xml:lang="ja">この項目が収集された層位が帰属している、あり得る最新の地質年代学的累代、または最上部の年代層序的累界のフルネーム、あるいは“Precambrian“などの非公式な名前。</skos:definition>
<skos:example xml:lang="ja"/>
<skos:inScheme rdf:resource="http://rs.gbif.org/terms/dwc/dwc_translations.rdf"/>
<rdf:type rdf:resource="http://www.w3.org/1999/02/22-rdf-syntax-ns#Property"/>
</skos:Concept>
<skos:Concept rdf:about="http://rs.tdwg.org/dwc/terms/latestEpochOrHighestSeries">
<skos:prefLabel xml:lang="en">Latest Epoch Or Highest Series
		</skos:prefLabel>
<skos:definition xml:lang="en">The full name of the latest
			possible
			geochronologic epoch or highest chronostratigraphic series
			attributable to the stratigraphic horizon from which the cataloged
			item was collected.</skos:definition>
<skos:example xml:lang="en">Examples:
			"Holocene", "Pleistocene", "Ibexian
			Series"</skos:example>
<skos:prefLabel xml:lang="es">Época tardía o sistema superior</skos:prefLabel>
<skos:definition xml:lang="es">El nombre completo de la época
			geocronológica más tardía posible o la serie cronoestratigráfica más
			alta, atribuible al horizonte estratigráfico donde se recolectó el
			objeto catalogado.</skos:definition>
<skos:example xml:lang="es">Ejemplo: "Holoceno", "Pleistoceno",
			"Serie Ibexian"</skos:example>
<skos:prefLabel xml:lang="zh-Hans">最晚地质世或最高地层统</skos:prefLabel>
<skos:definition xml:lang="zh-Hans">采集编目项所在地层地平线的可能最晚的地质世或最高地层统的完整名称。</skos:definition>
<skos:example xml:lang="zh-Hans"/>
<skos:prefLabel xml:lang="ja"/>
<skos:definition xml:lang="ja">この項目が収集された層位が帰属している、あり得る最新の地質年代学的世、または最上部の年代層序的統のフルネーム。</skos:definition>
<skos:example xml:lang="ja"/>
<skos:inScheme rdf:resource="http://rs.gbif.org/terms/dwc/dwc_translations.rdf"/>
<rdf:type rdf:resource="http://www.w3.org/1999/02/22-rdf-syntax-ns#Property"/>
</skos:Concept>
<skos:Concept rdf:about="http://rs.tdwg.org/dwc/terms/latestEraOrHighestErathem">
<skos:prefLabel xml:lang="en">Latest Era Or Highest Erathem
		</skos:prefLabel>
<skos:definition xml:lang="en">The full name of the latest
			possible
			geochronologic era or highest chronostratigraphic erathem
			attributable to the stratigraphic horizon from which the cataloged
			item was collected.</skos:definition>
<skos:example xml:lang="en">Examples:
			"Cenozoic", "Mesozoic"</skos:example>
<skos:prefLabel xml:lang="es">Era tardía o eratema superior</skos:prefLabel>
<skos:definition xml:lang="es">El nombre completo de la era
			geocronológica más tardía o el eratema cronoestratigráfico más alto
			posible, atribuible al horizonte estratigráfico donde se recolectó el
			objeto catalogado.</skos:definition>
<skos:example xml:lang="es">Ejemplo: "Cenozoico", "Mesozoico"</skos:example>
<skos:prefLabel xml:lang="zh-Hans">最晚地质代或最高地层界</skos:prefLabel>
<skos:definition xml:lang="zh-Hans">采集编目项所在地层地平线的可能最晚的地质代或最高地层界的完整名称。</skos:definition>
<skos:example xml:lang="zh-Hans"/>
<skos:prefLabel xml:lang="ja"/>
<skos:definition xml:lang="ja">この項目が収集された層位が帰属している、あり得る最新の地質年代学的代、または最上部の年代層序的界のフルネーム。</skos:definition>
<skos:example xml:lang="ja"/>
<skos:inScheme rdf:resource="http://rs.gbif.org/terms/dwc/dwc_translations.rdf"/>
<rdf:type rdf:resource="http://www.w3.org/1999/02/22-rdf-syntax-ns#Property"/>
</skos:Concept>
<skos:Concept rdf:about="http://rs.tdwg.org/dwc/terms/latestPeriodOrHighestSystem">
<skos:prefLabel xml:lang="en">Latest Period Or Highest System
		</skos:prefLabel>
<skos:definition xml:lang="en">The full name of the latest
			possible
			geochronologic period or highest chronostratigraphic system
			attributable to the stratigraphic horizon from which the cataloged
			item was collected.</skos:definition>
<skos:example xml:lang="en">Examples: "Neogene",
			"Tertiary", "Quaternary"</skos:example>
<skos:prefLabel xml:lang="es">Periodo tardío o sistema superior</skos:prefLabel>
<skos:definition xml:lang="es">El nombre completo del período
			geocronológico más tardío posible o del sistema cronoestratigráfico
			más alto, atribuible al horizonte estratigráfico donde se recolectó
			el objeto catalogado.</skos:definition>
<skos:example xml:lang="es">Ejemplo: "Neógeno", "Terciario",
			"Cuaternario"</skos:example>
<skos:prefLabel xml:lang="zh-Hans">最晚地质纪或最高地层系</skos:prefLabel>
<skos:definition xml:lang="zh-Hans">采集编目项所在地层地平线的可能最晚的地质纪或最高地层系的完整名称。</skos:definition>
<skos:example xml:lang="zh-Hans"/>
<skos:prefLabel xml:lang="ja"/>
<skos:definition xml:lang="ja">この項目が収集された層位が帰属している、あり得る最新の地質年代学的紀、または最上部の年代層序的系のフルネーム。</skos:definition>
<skos:example xml:lang="ja"/>
<skos:inScheme rdf:resource="http://rs.gbif.org/terms/dwc/dwc_translations.rdf"/>
<rdf:type rdf:resource="http://www.w3.org/1999/02/22-rdf-syntax-ns#Property"/>
</skos:Concept>
<skos:Concept rdf:about="http://rs.tdwg.org/dwc/terms/lifeStage">
<skos:prefLabel xml:lang="en">Life Stage</skos:prefLabel>
<skos:definition xml:lang="en">The age class or life stage of the
			biological individual(s) at the time the Occurrence was recorded.
			Recommended best practice is to use a controlled vocabulary.
		</skos:definition>
<skos:example xml:lang="en">Examples: "egg",
			"eft", "juvenile", "adult",
			"2 adults 4 juveniles"
		</skos:example>
<skos:prefLabel xml:lang="es">Etapa de vida</skos:prefLabel>
<skos:definition xml:lang="es">La clase etaria o etapa de vida del
			individuo(s) biológico(s) en el momento del Registro Biológico. La
			práctica recomendada es el uso de un lenguaje controlado.</skos:definition>
<skos:example xml:lang="es">Ejemplo: "huevo", "juvenil", "adulto", "2
			adultos 4 juveniles"</skos:example>
<skos:prefLabel xml:lang="zh-Hans">生命期</skos:prefLabel>
<skos:definition xml:lang="zh-Hans">事件记录时生物个体的年龄级或生命期。建议最佳做法是使用一个控制性词汇。</skos:definition>
<skos:example xml:lang="zh-Hans"/>
<skos:prefLabel xml:lang="ja"/>
<skos:definition xml:lang="ja">レコードが記述された時点における、生物個体の齢級または世代区分。管理された語彙の使用を推奨。</skos:definition>
<skos:example xml:lang="ja"/>
<skos:inScheme rdf:resource="http://rs.gbif.org/terms/dwc/dwc_translations.rdf"/>
<rdf:type rdf:resource="http://www.w3.org/1999/02/22-rdf-syntax-ns#Property"/>
</skos:Concept>
<skos:Concept rdf:about="http://rs.tdwg.org/dwc/terms/lithostratigraphicTerms">
<skos:prefLabel xml:lang="en">Lithostratigraphic Terms</skos:prefLabel>
<skos:definition xml:lang="en">The combination of all
			litho-stratigraphic names for the rock from which the cataloged item
			was collected.</skos:definition>
<skos:example xml:lang="en"/>
<skos:prefLabel xml:lang="es">Términos litoestratigráficos</skos:prefLabel>
<skos:definition xml:lang="es">La combinación de todos los nombres
			litoestratigráficos de la roca de donde se colectó el objeto
			catalogado. </skos:definition>
<skos:example xml:lang="es"/>
<skos:prefLabel xml:lang="zh-Hans">岩性地层</skos:prefLabel>
<skos:definition xml:lang="zh-Hans">采集编目项所在岩石的所有岩性地层名称的组合。</skos:definition>
<skos:example xml:lang="zh-Hans"/>
<skos:prefLabel xml:lang="ja"/>
<skos:definition xml:lang="ja">この項目が収集された岩の、岩相層序名の組み合わせ。</skos:definition>
<skos:example xml:lang="ja"/>
<skos:inScheme rdf:resource="http://rs.gbif.org/terms/dwc/dwc_translations.rdf"/>
<rdf:type rdf:resource="http://www.w3.org/1999/02/22-rdf-syntax-ns#Property"/>
</skos:Concept>
<skos:Concept rdf:about="http://rs.tdwg.org/dwc/terms/locality">
<skos:prefLabel xml:lang="en">Locality</skos:prefLabel>
<skos:definition xml:lang="en">The specific description of the
			place.
			Less specific geographic information can be provided in other
			geographic terms (higherGeography, continent, country, stateProvince,
			county, municipality, waterBody, island, islandGroup). This term may
			contain information modified from the original to correct perceived
			errors or standardize the description.</skos:definition>
<skos:example xml:lang="en">Example: "Bariloche,
			25 km NNE via Ruta
			Nacional 40 (=Ruta 237)"</skos:example>
<skos:prefLabel xml:lang="es">Localidad</skos:prefLabel>
<skos:definition xml:lang="es">La descripción específica del
			lugar. Información geográfica de menor especificidad puede ser
			provista en otros elementos geográficos (Geografía Superior,
			Continente, País, Estado Provincia, Condado, Municipio, Cuerpo de
			Agua, Isla, Grupo Islas). Este elemento puede contener información
			modificada de la original para corregir errores o estandarizar la
			descripción. </skos:definition>
<skos:example xml:lang="es">Ejemplo: "Bariloche, 25 km NNE vía Ruta
			Nacional 40 (=Ruta 237)"</skos:example>
<skos:prefLabel xml:lang="zh-Hans">地点</skos:prefLabel>
<skos:definition xml:lang="zh-Hans">地点的具体描述。其它的地理术语几乎不提供具体地理信息（高级地域，大陆，国家，州/省，县，自治市，水体，岛屿，群岛）。这个术语可能包含由最初修改而来的信息，以纠正理解错误或规范描述。</skos:definition>
<skos:example xml:lang="zh-Hans"/>
<skos:prefLabel xml:lang="ja"/>
<skos:definition xml:lang="ja">場所に関する特別な記載。そこまで特別ではない場所に関する情報は、他の場所に関するタームにするべきである
			(higherGeography, 大陸, 国, stateProvince, 郡, 市町村, waterBody, 島,
			islandGroup)。このタームには元々のタームの間違いを直したり、標準化したことを示す情報も含むこともある。</skos:definition>
<skos:example xml:lang="ja"/>
<skos:inScheme rdf:resource="http://rs.gbif.org/terms/dwc/dwc_translations.rdf"/>
<rdf:type rdf:resource="http://www.w3.org/1999/02/22-rdf-syntax-ns#Property"/>
</skos:Concept>
<skos:Concept rdf:about="http://rs.tdwg.org/dwc/terms/locationAccordingTo">
<skos:prefLabel xml:lang="en">Location According To</skos:prefLabel>
<skos:definition xml:lang="en">Information about the source of
			this
			Location information. Could be a publication (gazetteer),
			institution, or team of individuals.</skos:definition>
<skos:example xml:lang="en">Example: "Getty
			Thesaurus of Geographic
			Names", "GADM"</skos:example>
<skos:prefLabel xml:lang="es">Ubicación de acuerdo con</skos:prefLabel>
<skos:definition xml:lang="es">La información sobre la fuente de la
			información de ubicación. Podría ser una publicación (gacetero),
			institución o grupo de individuos.</skos:definition>
<skos:example xml:lang="es">Ejemplo: "Tesauro Getty de nombres
			geográficos", "GADM"</skos:example>
<skos:prefLabel xml:lang="zh-Hans">地点依据</skos:prefLabel>
<skos:definition xml:lang="zh-Hans">地点信息源的信息，可能是出版物（地名），机构，或者团队个体。</skos:definition>
<skos:example xml:lang="zh-Hans"/>
<skos:prefLabel xml:lang="ja"/>
<skos:definition xml:lang="ja">位置情報の情報源。出版物（地名集）、機関、チームなど。</skos:definition>
<skos:example xml:lang="ja"/>
<skos:inScheme rdf:resource="http://rs.gbif.org/terms/dwc/dwc_translations.rdf"/>
<rdf:type rdf:resource="http://www.w3.org/1999/02/22-rdf-syntax-ns#Property"/>
</skos:Concept>
<skos:Concept rdf:about="http://rs.tdwg.org/dwc/terms/locationID">
<skos:prefLabel xml:lang="en">Location ID</skos:prefLabel>
<skos:definition xml:lang="en">An identifier for the set of
			location
			information (data associated with dcterms:Location). May be
			a global
			unique identifier or an identifier specific to the data set.
		</skos:definition>
<skos:example xml:lang="en"/>
<skos:prefLabel xml:lang="es">ID de la ubicación</skos:prefLabel>
<skos:definition xml:lang="es">Un identificador para el conjunto de
			información de la ubicación (los datos asociados a Ubicación). Puede
			ser un identificador único global o un identificador específico para
			el conjunto de datos. </skos:definition>
<skos:example xml:lang="es"/>
<skos:prefLabel xml:lang="zh-Hans"/>
<skos:definition xml:lang="zh-Hans"/>
<skos:example xml:lang="zh-Hans"/>
<skos:prefLabel xml:lang="ja"/>
<skos:definition xml:lang="ja">位置情報（dcterms:Locationに関連するデータ）セットのID。GUIDまたは、そのデータセット固有のID。</skos:definition>
<skos:example xml:lang="ja"/>
<skos:inScheme rdf:resource="http://rs.gbif.org/terms/dwc/dwc_translations.rdf"/>
<rdf:type rdf:resource="http://www.w3.org/1999/02/22-rdf-syntax-ns#Property"/>
</skos:Concept>
<skos:Concept rdf:about="http://rs.tdwg.org/dwc/terms/locationRemarks">
<skos:prefLabel xml:lang="en">Location Remarks</skos:prefLabel>
<skos:definition xml:lang="en">Comments or notes about the
			Location.</skos:definition>
<skos:example xml:lang="en">Example: "under
			water since 2005"</skos:example>
<skos:prefLabel xml:lang="es">Comentarios de la ubicación</skos:prefLabel>
<skos:definition xml:lang="es">Comentarios o anotaciones sobre la
			ubicación. </skos:definition>
<skos:example xml:lang="es">Ejemplo: "bajo agua desde 2005"</skos:example>
<skos:prefLabel xml:lang="zh-Hans">地点备注</skos:prefLabel>
<skos:definition xml:lang="zh-Hans">关于地点的评论或记录。</skos:definition>
<skos:example xml:lang="zh-Hans"/>
<skos:prefLabel xml:lang="ja"/>
<skos:definition xml:lang="ja">位置に関するコメントまたは注釈。</skos:definition>
<skos:example xml:lang="ja"/>
<skos:inScheme rdf:resource="http://rs.gbif.org/terms/dwc/dwc_translations.rdf"/>
<rdf:type rdf:resource="http://www.w3.org/1999/02/22-rdf-syntax-ns#Property"/>
</skos:Concept>
<skos:Concept rdf:about="http://rs.tdwg.org/dwc/terms/lowestBiostratigraphicZone">
<skos:prefLabel xml:lang="en">Lowest Biostratigraphic Zone
		</skos:prefLabel>
<skos:definition xml:lang="en">The full name of the lowest
			possible
			geological biostratigraphic zone of the stratigraphic
			horizon from
			which the cataloged item was collected.</skos:definition>
<skos:example xml:lang="en"/>
<skos:prefLabel xml:lang="es">Zona bioestatigráfica inferior</skos:prefLabel>
<skos:definition xml:lang="es">El nombre completo de la zona
			geológica bioestratigráfica más baja posible del horizonte
			estratigráfico donde se recolectó el objeto catalogado. </skos:definition>
<skos:example xml:lang="es"/>
<skos:prefLabel xml:lang="zh-Hans">最低生物地层区</skos:prefLabel>
<skos:definition xml:lang="zh-Hans">采集编目项所在地层地平线的可能最低的地质生物地层学区的完整名称。</skos:definition>
<skos:example xml:lang="zh-Hans"/>
<skos:prefLabel xml:lang="ja"/>
<skos:definition xml:lang="ja">この項目が収集された層位の、あり得る最下部の地質学的な生層序学的区分のフルネーム。</skos:definition>
<skos:example xml:lang="ja"/>
<skos:inScheme rdf:resource="http://rs.gbif.org/terms/dwc/dwc_translations.rdf"/>
<rdf:type rdf:resource="http://www.w3.org/1999/02/22-rdf-syntax-ns#Property"/>
</skos:Concept>
<skos:Concept rdf:about="http://rs.tdwg.org/dwc/terms/maximumDepthInMeters">
<skos:prefLabel xml:lang="en">Maximum Depth In Meters</skos:prefLabel>
<skos:definition xml:lang="en">The greater depth of a range of
			depth
			below the local surface, in meters.</skos:definition>
<skos:example xml:lang="en">Example: "200"
		</skos:example>
<skos:prefLabel xml:lang="es">Profundidad máxima en metros</skos:prefLabel>
<skos:definition xml:lang="es">La mayor profundidad de un rango de
			profundidad por debajo de la superficie local, en metros.</skos:definition>
<skos:example xml:lang="es">Ejemplo: "200"</skos:example>
<skos:prefLabel xml:lang="zh-Hans">最大深度（米）</skos:prefLabel>
<skos:definition xml:lang="zh-Hans">在地表一定深度范围以下的更深的深度，以“米”作单位。</skos:definition>
<skos:example xml:lang="zh-Hans"/>
<skos:prefLabel xml:lang="ja"/>
<skos:definition xml:lang="ja">地表下の、あるい深度範囲における、最大の深度（メートル表記）。</skos:definition>
<skos:example xml:lang="ja"/>
<skos:inScheme rdf:resource="http://rs.gbif.org/terms/dwc/dwc_translations.rdf"/>
<rdf:type rdf:resource="http://www.w3.org/1999/02/22-rdf-syntax-ns#Property"/>
</skos:Concept>
<skos:Concept rdf:about="http://rs.tdwg.org/dwc/terms/maximumDistanceAboveSurfaceInMeters">
<skos:prefLabel xml:lang="en">Maximum Distance Above Surface In
			Meters</skos:prefLabel>
<skos:definition xml:lang="en">The greater distance in a range of
			distance from a reference surface in the vertical direction, in
			meters. Use positive values for locations above the surface, negative
			values for locations below. If depth measures are given, the
			reference surface is the location given by the depth, otherwise the
			reference surface is the location given by the elevation.
		</skos:definition>
<skos:example xml:lang="en">Example: 1.5 meter
			sediment core from the
			bottom of a lake (at depth 20m) at 300m
			elevation; VerbatimElevation:
			"300m" MinimumElevationInMeters: "300",
			MaximumElevationInMeters:
			"300", VerbatimDepth: "20m",
			MinimumDepthInMeters: "20",
			MaximumDepthInMeters: "20",
			minimumDistanceAboveSurfaceInMeters: "0",
			maximumDistanceAboveSurfaceInMeters: "-1.5"</skos:example>
<skos:prefLabel xml:lang="es">Máxima distancia de la superficie metros</skos:prefLabel>
<skos:definition xml:lang="es">La mayor distancia en un rango de
			distancia desde una superficie de referencia en dirección vertical,
			en metros. Utilice valores positivos para las ubicaciones por encima
			de la superficie, valores negativos para las ubicaciones por
			debajo. Si las medidas de profundidad son provistas, la superficie de
			referencia es la ubicación determinada por la profundidad, de lo
			contrario la superficie de referencia es la ubicación determinada por
			la elevación. </skos:definition>
<skos:example xml:lang="es">Ejemplo: 1,5 metros de sedimento desde el
			fondo de un lago (a una profundidad de 20 metros) a una elevación de
			300m; Elevación Original: "300m" Mínima Elevación en Metros: "300",
			Máxima Elevación en Metros: "300", Profundidad Original: "20m",
			Mínima Profundidad en Metros: "20", Máxima Profundidad en Metros:
			"20", Mínima Distancia de la Superficie en Metros: "0", Máxima
			Distancia de la Superficie en Metros: "-1,5"</skos:example>
<skos:prefLabel xml:lang="zh-Hans">参考表面以上的最大距离（米）</skos:prefLabel>
<skos:definition xml:lang="zh-Hans">在垂直方向，距离参考表面更大的一个距离范围内，以米作为单位。使用正值代表表面以上的位置，负值代表表面以下的位置。如果已经给出深度的测量值，那么参考表面的位置由深度确定，否则参考表面的位置由海拔确定。</skos:definition>
<skos:example xml:lang="zh-Hans"/>
<skos:prefLabel xml:lang="ja"/>
<skos:definition xml:lang="ja">基準となる地表下の垂直方向での距離の最大値(m)。地表より上の場合は正の値を用い、地表下の場合は負の値を用いる。基準となる地表は深さで与えられる、そうでなければ標高で与えられる。</skos:definition>
<skos:example xml:lang="ja">例: 300mの標高にある湖の底(深さ20m)の1.5mの堆積物コア;
			VerbatimElevation: "300m" MinimumElevationInMeters: "300",
			MaximumElevationInMeters: "300", VerbatimDepth: "20m",
			MinimumDepthInMeters: "20", MaximumDepthInMeters: "20",
			minimumDistanceAboveSurfaceInMeters: "0",
			maximumDistanceAboveSurfaceInMeters: "-1.5"</skos:example>
<skos:inScheme rdf:resource="http://rs.gbif.org/terms/dwc/dwc_translations.rdf"/>
<rdf:type rdf:resource="http://www.w3.org/1999/02/22-rdf-syntax-ns#Property"/>
</skos:Concept>
<skos:Concept rdf:about="http://rs.tdwg.org/dwc/terms/maximumElevationInMeters">
<skos:prefLabel xml:lang="en">Maximum Elevation In Meters
		</skos:prefLabel>
<skos:definition xml:lang="en">The upper limit of the range of
			elevation (altitude, usually above sea level), in meters.
		</skos:definition>
<skos:example xml:lang="en">Example: "200"
		</skos:example>
<skos:prefLabel xml:lang="es">Elevación máxima en metros</skos:prefLabel>
<skos:definition xml:lang="es">El límite superior del rango de
			elevación (altitud, generalmente por encima del nivel del mar), en
			metros. </skos:definition>
<skos:example xml:lang="es">Ejemplo: "200"</skos:example>
<skos:prefLabel xml:lang="zh-Hans">最高海拔（米）</skos:prefLabel>
<skos:definition xml:lang="zh-Hans">海拔（海平面以上的高度）范围的上限，以“米”为单位。</skos:definition>
<skos:example xml:lang="zh-Hans"/>
<skos:prefLabel xml:lang="ja"/>
<skos:definition xml:lang="ja">ある標高の範囲（高度、大抵の場合は海抜）の中の上限値（メートル表記）。</skos:definition>
<skos:example xml:lang="ja"/>
<skos:inScheme rdf:resource="http://rs.gbif.org/terms/dwc/dwc_translations.rdf"/>
<rdf:type rdf:resource="http://www.w3.org/1999/02/22-rdf-syntax-ns#Property"/>
</skos:Concept>
<skos:Concept rdf:about="http://rs.tdwg.org/dwc/terms/measurementAccuracy">
<skos:prefLabel xml:lang="en">Measurement Accuracy</skos:prefLabel>
<skos:definition xml:lang="en">The description of the potential
			error
			associated with the measurementValue.</skos:definition>
<skos:example xml:lang="en">Examples: "0.01",
			"normal distribution with
			variation of 2 m"</skos:example>
<skos:prefLabel xml:lang="es">Precisión de la medición</skos:prefLabel>
<skos:definition xml:lang="es">La descripción de los errores
			potenciales asociados con Valor de la medición. </skos:definition>
<skos:example xml:lang="es">Ejemplo: "0.01", "distribución normal con
			variación de 2 m"</skos:example>
<skos:prefLabel xml:lang="zh-Hans">测量精度</skos:prefLabel>
<skos:definition xml:lang="zh-Hans">与测量值相关的潜在误差的描述。</skos:definition>
<skos:example xml:lang="zh-Hans"/>
<skos:prefLabel xml:lang="ja"/>
<skos:definition xml:lang="ja">measurementValueの関連する、潜在的な誤差の記述。</skos:definition>
<skos:example xml:lang="ja"/>
<skos:inScheme rdf:resource="http://rs.gbif.org/terms/dwc/dwc_translations.rdf"/>
<rdf:type rdf:resource="http://www.w3.org/1999/02/22-rdf-syntax-ns#Property"/>
</skos:Concept>
<skos:Concept rdf:about="http://rs.tdwg.org/dwc/terms/measurementDeterminedBy">
<skos:prefLabel xml:lang="en">Measurement Determined By</skos:prefLabel>
<skos:definition xml:lang="en">A list (concatenated and
			separated) of
			names of people, groups, or organizations who
			determined the value of
			the MeasurementOrFact.</skos:definition>
<skos:example xml:lang="en">Example: "Javier de
			la Torre", "Julie
			Woodruff; Eileen Lacey"</skos:example>
<skos:prefLabel xml:lang="es">Medición determinada por</skos:prefLabel>
<skos:definition xml:lang="es">Una lista (concatenada y separada) de
			los nombres de las personas, grupos u organizaciones que determinan
			el valor de Medición o Hecho. </skos:definition>
<skos:example xml:lang="es">Ejemplo: "Javier de la Torre", "Julie
			Woodruff; Eileen Lacey"</skos:example>
<skos:prefLabel xml:lang="zh-Hans">确定测量结果者</skos:prefLabel>
<skos:definition xml:lang="zh-Hans">确定“测量或事实”值的人名，群体或组织的列表（连接的或分开的）。</skos:definition>
<skos:example xml:lang="zh-Hans"/>
<skos:prefLabel xml:lang="ja"/>
<skos:definition xml:lang="ja">MeasurementOrFactの値を決定した人物、グループ、または組織の名前のリスト。</skos:definition>
<skos:example xml:lang="ja"/>
<skos:inScheme rdf:resource="http://rs.gbif.org/terms/dwc/dwc_translations.rdf"/>
<rdf:type rdf:resource="http://www.w3.org/1999/02/22-rdf-syntax-ns#Property"/>
</skos:Concept>
<skos:Concept rdf:about="http://rs.tdwg.org/dwc/terms/measurementDeterminedDate">
<skos:prefLabel xml:lang="en">Measurement Determined Date
		</skos:prefLabel>
<skos:definition xml:lang="en">The date on which the
			MeasurementOrFact was made. Recommended best practice is to use an
			encoding scheme, such as ISO 8601:2004(E).</skos:definition>
<skos:example xml:lang="en">Examples:
			"1963-03-08T14:07-0600" is 8 Mar
			1963 2:07pm in the time zone six
			hours earlier than UTC,
			"2009-02-20T08:40Z" is 20 Feb 2009 8:40am
			UTC, "1809-02-12" is 12 Feb
			1809, "1906-06" is Jun 1906, "1971" is
			just that year,
			"2007-03-01T13:00:00Z/2008-05-11T15:30:00Z" is the
			interval between 1
			Mar 2007 1pm UTC and 11 May 2008 3:30pm UTC,
			"2007-11-13/15" is the
			interval between 13 Nov 2007 and 15 Nov 2007.
		</skos:example>
<skos:prefLabel xml:lang="es">Fecha de la determinación de la medición</skos:prefLabel>
<skos:definition xml:lang="es">La fecha en que se realizó Medición o
			Hecho. La práctica recomendada es utilizar un esquema de
			codificación, como ISO 8601:2004 (E). </skos:definition>
<skos:example xml:lang="es">Ejemplo: "1963-03-08T14:07-0600" es 8 de
			marzo de 1963 2:07pm en zona horaria seis horas más temprano que UTC,
			"2009-02-20T08:40Z" es 20 de febrero 2009 8:40am UTC, "1809-02-12" es
			12 de febrero de 1809, "1906-06" es junio de 1906, "1971",
			"2007-03-01T13:00:00Z/2008-05-11T15:30:00Z" es el intervalo entre el
			1 de marzo de 2007 1pm UTC y 11 de mayo de 2008 3:30pm UTC,
			"2007-11-13/15" es el intervalo entre el 13 de noviembre de 2007 y 15
			de noviembre de 2007.</skos:example>
<skos:prefLabel xml:lang="zh-Hans">确定测量结果日期</skos:prefLabel>
<skos:definition xml:lang="zh-Hans">制定“测量或事实”的日期，建议最佳做法是使用一个编码方案，例如ISO
			8601:2004(E)。</skos:definition>
<skos:example xml:lang="zh-Hans"/>
<skos:prefLabel xml:lang="ja"/>
<skos:definition xml:lang="ja">MeasurementOrFactがなされた日付。ISO
			8601:2004(E)などのスキーマの使用を推奨。</skos:definition>
<skos:example xml:lang="ja"/>
<skos:inScheme rdf:resource="http://rs.gbif.org/terms/dwc/dwc_translations.rdf"/>
<rdf:type rdf:resource="http://www.w3.org/1999/02/22-rdf-syntax-ns#Property"/>
</skos:Concept>
<skos:Concept rdf:about="http://rs.tdwg.org/dwc/terms/measurementID">
<skos:prefLabel xml:lang="en">Measurement ID</skos:prefLabel>
<skos:definition xml:lang="en">An identifier for the
			MeasurementOrFact (information pertaining to measurements, facts,
			characteristics, or assertions). May be a global unique identifier or
			an identifier specific to the data set.</skos:definition>
<skos:example xml:lang="en"/>
<skos:prefLabel xml:lang="es">ID de la medición</skos:prefLabel>
<skos:definition xml:lang="es">Un identificador para Medición o hecho
			(la información relativa a las mediciones, hechos, características o
			aseveraciones). Puede ser un identificador único global o un
			identificador específico para el conjunto de datos. </skos:definition>
<skos:example xml:lang="es"/>
<skos:prefLabel xml:lang="zh-Hans">测量编号</skos:prefLabel>
<skos:definition xml:lang="zh-Hans">测量或事实（关于测量，事实，特征或推断的信息）的标识符，可能是一个全局唯一标识符或者一个数据集特有的标识符。</skos:definition>
<skos:example xml:lang="zh-Hans"/>
<skos:prefLabel xml:lang="ja"/>
<skos:definition xml:lang="ja">MeasurementOrFact（測定、事実、特徴、または主張に付随する情報）のID。GUIDまたは、そのデータセット固有のID。</skos:definition>
<skos:example xml:lang="ja"/>
<skos:inScheme rdf:resource="http://rs.gbif.org/terms/dwc/dwc_translations.rdf"/>
<rdf:type rdf:resource="http://www.w3.org/1999/02/22-rdf-syntax-ns#Property"/>
</skos:Concept>
<skos:Concept rdf:about="http://rs.tdwg.org/dwc/terms/measurementMethod">
<skos:prefLabel xml:lang="en">Measurement Method</skos:prefLabel>
<skos:definition xml:lang="en">A description of or reference to
			(publication, URI) the method or protocol used to determine the
			measurement, fact, characteristic, or assertion.</skos:definition>
<skos:example xml:lang="en">Examples: "minimum
			convex polygon around
			burrow entrances" for a home range area,
			"barometric altimeter" for an
			elevation</skos:example>
<skos:prefLabel xml:lang="es">Método de medición</skos:prefLabel>
<skos:definition xml:lang="es">Una descripción o referencia
			(publicación, URI) del método o protocolo utilizado para determinar
			la medición, hecho, característica o aseveración. </skos:definition>
<skos:example xml:lang="es">Ejemplos: "mínimo polígono convexo alrededor
			de las entradas de la madriguera" para rango de hábitat, "altímetro
			barométrico" para una elevación</skos:example>
<skos:prefLabel xml:lang="zh-Hans">测量方法</skos:prefLabel>
<skos:definition xml:lang="zh-Hans">用来确定测量，事实，特征或者推断的方法或草案的描述或者参考。</skos:definition>
<skos:example xml:lang="zh-Hans"/>
<skos:prefLabel xml:lang="ja"/>
<skos:definition xml:lang="ja">測定、事実、特徴、または主張を決定するのに用いた手法または手順の参考文献（出版物、URIなど）の記述。</skos:definition>
<skos:example xml:lang="ja"/>
<skos:inScheme rdf:resource="http://rs.gbif.org/terms/dwc/dwc_translations.rdf"/>
<rdf:type rdf:resource="http://www.w3.org/1999/02/22-rdf-syntax-ns#Property"/>
</skos:Concept>
<skos:Concept rdf:about="http://rs.tdwg.org/dwc/terms/measurementRemarks">
<skos:prefLabel xml:lang="en">Measurement Remarks</skos:prefLabel>
<skos:definition xml:lang="en">Comments or notes accompanying the
			MeasurementOrFact.</skos:definition>
<skos:example xml:lang="en">Example: "tip of
			tail missing"</skos:example>
<skos:prefLabel xml:lang="es">Comentarios de la medición</skos:prefLabel>
<skos:definition xml:lang="es">Comentarios o anotaciones que
			acompañan a Medición o hecho. </skos:definition>
<skos:example xml:lang="es">Ejemplo: "falta la punta de la cola"</skos:example>
<skos:prefLabel xml:lang="zh-Hans">测量备注</skos:prefLabel>
<skos:definition xml:lang="zh-Hans">附在“测量或事实”上的评论和注释。</skos:definition>
<skos:example xml:lang="zh-Hans"/>
<skos:prefLabel xml:lang="ja"/>
<skos:definition xml:lang="ja">MeasurementOrFactに付随するコメントまたは注釈。</skos:definition>
<skos:example xml:lang="ja"/>
<skos:inScheme rdf:resource="http://rs.gbif.org/terms/dwc/dwc_translations.rdf"/>
<rdf:type rdf:resource="http://www.w3.org/1999/02/22-rdf-syntax-ns#Property"/>
</skos:Concept>
<skos:Concept rdf:about="http://rs.tdwg.org/dwc/terms/measurementType">
<skos:prefLabel xml:lang="en">Measurement Type</skos:prefLabel>
<skos:definition xml:lang="en">The nature of the measurement,
			fact,
			characteristic, or assertion. Recommended best practice is to
			use a
			controlled vocabulary.</skos:definition>
<skos:example xml:lang="en">Examples: "tail
			length", "temperature", "trap
			line length", "survey area", "trap
			type"</skos:example>
<skos:prefLabel xml:lang="es">Tipo de medición</skos:prefLabel>
<skos:definition xml:lang="es">La naturaleza de la medición, hecho,
			característica o aseveración. La práctica recomendada es el uso de un
			lenguaje controlado. </skos:definition>
<skos:example xml:lang="es">Ejemplo: "longitud de la cola",
			"temperatura", "área de muestreo", "tipo trampa"</skos:example>
<skos:prefLabel xml:lang="zh-Hans">测量类型</skos:prefLabel>
<skos:definition xml:lang="zh-Hans">测量，事实，特征，和推断的性质。最好的做法是使用一个控制性词汇。</skos:definition>
<skos:example xml:lang="zh-Hans"/>
<skos:prefLabel xml:lang="ja"/>
<skos:definition xml:lang="ja">測定、事実、特徴、または主張の特性。管理された語彙の使用を推奨。</skos:definition>
<skos:example xml:lang="ja"/>
<skos:inScheme rdf:resource="http://rs.gbif.org/terms/dwc/dwc_translations.rdf"/>
<rdf:type rdf:resource="http://www.w3.org/1999/02/22-rdf-syntax-ns#Property"/>
</skos:Concept>
<skos:Concept rdf:about="http://rs.tdwg.org/dwc/terms/measurementUnit">
<skos:prefLabel xml:lang="en">Measurement Unit</skos:prefLabel>
<skos:definition xml:lang="en">The units associated with the
			measurementValue. Recommended best practice is to use the
			International System of Units (SI).</skos:definition>
<skos:example xml:lang="en">Examples: "mm", "C",
			"km", "ha"</skos:example>
<skos:prefLabel xml:lang="es">Unidad de medición</skos:prefLabel>
<skos:definition xml:lang="es">Las unidades asociadas con Valor de la
			Medición. La práctica recomendada es utilizar el Sistema
			Internacional de Unidades (SI). </skos:definition>
<skos:example xml:lang="es">Ejemplo: "mm", "C", "km", "ha"</skos:example>
<skos:prefLabel xml:lang="zh-Hans">测量单位</skos:prefLabel>
<skos:definition xml:lang="zh-Hans">与测量值相关的单位最好采用国际单位系统（SI）。</skos:definition>
<skos:example xml:lang="zh-Hans"/>
<skos:prefLabel xml:lang="ja"/>
<skos:definition xml:lang="ja">measurementValueに関連する単位。国際単位系（SI）の使用を推奨。</skos:definition>
<skos:example xml:lang="ja"/>
<skos:inScheme rdf:resource="http://rs.gbif.org/terms/dwc/dwc_translations.rdf"/>
<rdf:type rdf:resource="http://www.w3.org/1999/02/22-rdf-syntax-ns#Property"/>
</skos:Concept>
<skos:Concept rdf:about="http://rs.tdwg.org/dwc/terms/measurementValue">
<skos:prefLabel xml:lang="en">Measurement Value</skos:prefLabel>
<skos:definition xml:lang="en">The value of the measurement,
			fact,
			characteristic, or assertion.</skos:definition>
<skos:example xml:lang="en">Examples: "45",
			"20", "1", "14.5", "UV-light"</skos:example>
<skos:prefLabel xml:lang="es">Valor de la medición</skos:prefLabel>
<skos:definition xml:lang="es">El valor de la medición, hecho,
			característica o aseveración. </skos:definition>
<skos:example xml:lang="es">Ejemplo: "45", "20", "1", "14.5", "Luz UV"</skos:example>
<skos:prefLabel xml:lang="zh-Hans">测量值</skos:prefLabel>
<skos:definition xml:lang="zh-Hans">测量，事实，特征，和推断的值。</skos:definition>
<skos:example xml:lang="zh-Hans"/>
<skos:prefLabel xml:lang="ja"/>
<skos:definition xml:lang="ja">測定、事実、特徴、または主張の値。</skos:definition>
<skos:example xml:lang="ja"/>
<skos:inScheme rdf:resource="http://rs.gbif.org/terms/dwc/dwc_translations.rdf"/>
<rdf:type rdf:resource="http://www.w3.org/1999/02/22-rdf-syntax-ns#Property"/>
</skos:Concept>
<skos:Concept rdf:about="http://rs.tdwg.org/dwc/terms/member">
<skos:prefLabel xml:lang="en">Member</skos:prefLabel>
<skos:definition xml:lang="en">The full name of the
			lithostratigraphic member from which the cataloged item was
			collected.</skos:definition>
<skos:example xml:lang="en">Examples: "Lava Dam
			Member", "Hellnmaria
			Member"</skos:example>
<skos:prefLabel xml:lang="es">Miembro</skos:prefLabel>
<skos:definition xml:lang="es">El nombre completo del miembro
			litoestratigráfico del cual se colectó el elemento catalogado. </skos:definition>
<skos:example xml:lang="es">Ejemplos: "Miembro Lava Dam", "Miembro
			Hellnmaria"</skos:example>
<skos:prefLabel xml:lang="zh-Hans">成员</skos:prefLabel>
<skos:definition xml:lang="zh-Hans">采集编目项所在地层成员的完整名称。</skos:definition>
<skos:example xml:lang="zh-Hans"/>
<skos:prefLabel xml:lang="ja"/>
<skos:definition xml:lang="ja">この項目が収集された岩相層序メンバーのフルネーム。</skos:definition>
<skos:example xml:lang="ja"/>
<skos:inScheme rdf:resource="http://rs.gbif.org/terms/dwc/dwc_translations.rdf"/>
<rdf:type rdf:resource="http://www.w3.org/1999/02/22-rdf-syntax-ns#Property"/>
</skos:Concept>
<skos:Concept rdf:about="http://rs.tdwg.org/dwc/terms/minimumDepthInMeters">
<skos:prefLabel xml:lang="en">Minimum Depth In Meters</skos:prefLabel>
<skos:definition xml:lang="en">The lesser depth of a range of
			depth
			below the local surface, in meters.</skos:definition>
<skos:example xml:lang="en">Example: "100"
		</skos:example>
<skos:prefLabel xml:lang="es">Profundidad mínima en metros</skos:prefLabel>
<skos:definition xml:lang="es">La menor profundidad de un rango de
			profundidad por debajo de la superficie local, en metros. </skos:definition>
<skos:example xml:lang="es">Ejemplo: "100"</skos:example>
<skos:prefLabel xml:lang="zh-Hans">最小深度（米）</skos:prefLabel>
<skos:definition xml:lang="zh-Hans">地表以下较低的深度，以“米”为单位。</skos:definition>
<skos:example xml:lang="zh-Hans"/>
<skos:prefLabel xml:lang="ja"/>
<skos:definition xml:lang="ja">地表下の、あるいは深度範囲における、最小の深度（メートル表記）。</skos:definition>
<skos:example xml:lang="ja"/>
<skos:inScheme rdf:resource="http://rs.gbif.org/terms/dwc/dwc_translations.rdf"/>
<rdf:type rdf:resource="http://www.w3.org/1999/02/22-rdf-syntax-ns#Property"/>
</skos:Concept>
<skos:Concept rdf:about="http://rs.tdwg.org/dwc/terms/minimumDistanceAboveSurfaceInMeters">
<skos:prefLabel xml:lang="en">Minimum Distance Above Surface In
			Meters</skos:prefLabel>
<skos:definition xml:lang="en">The lesser distance in a range of
			distance from a reference surface in the vertical direction, in
			meters. Use positive values for locations above the surface, negative
			values for locations below. If depth measures are given, the
			reference surface is the location given by the depth, otherwise the
			reference surface is the location given by the elevation.
		</skos:definition>
<skos:example xml:lang="en">Example: 1.5 meter
			sediment core from the
			bottom of a lake (at depth 20m) at 300m
			elevation; VerbatimElevation:
			"300m" MinimumElevationInMeters: "300",
			MaximumElevationInMeters:
			"300", VerbatimDepth: "20m",
			MinimumDepthInMeters: "20",
			MaximumDepthInMeters: "20",
			minimumDistanceAboveSurfaceInMeters: "0",
			maximumDistanceAboveSurfaceInMeters: "-1.5"</skos:example>
<skos:prefLabel xml:lang="es">Mínima distancia de la superficie en metros</skos:prefLabel>
<skos:definition xml:lang="es">La menor distancia en un rango de
			distancia desde una superficie de referencia en dirección vertical,
			en metros. Utilice valores positivos para las ubicaciones por encima
			de la superficie, valores negativos para ubicaciones por debajo. Si
			las medidas de profundidad son provistas, la superficie de referencia
			es la ubicación determinada por la profundidad, de lo contrario la
			superficie de referencia es la ubicación dada por la elevación. </skos:definition>
<skos:example xml:lang="es">Ejemplo: 1,5 metros de sedimento desde el
			fondo de un lago (a una profundidad de 20 metros) a una elevación de
			300m; Elevación Original: "300m" Mínima Elevación en Metros: "300",
			Máxima Elevación en Metros: "300", Profundidad Original: "20m",
			Mínima Profundidad en Metros: "20", Máxima Profundidad en Metros:
			"20", Mínima Distancia de la Superficie en Metros: "0", Máxima
			Distancia de la Superficie en Metros: "-1,5"</skos:example>
<skos:prefLabel xml:lang="zh-Hans">参考表面以上的最小距离（米）</skos:prefLabel>
<skos:definition xml:lang="zh-Hans">在垂直方向，距离参考表面较小的距离范围内的距离，以“米”为单位。使用正值代表表面以上的位置，负值代表表面以下的位置。如果已经给出深度的测量值，那么参考表面的位置由深度确定，否则参考表面的位置由海拔确定。</skos:definition>
<skos:example xml:lang="zh-Hans"/>
<skos:prefLabel xml:lang="ja"/>
<skos:definition xml:lang="ja">基準となる地表下の垂直方向での距離の最小値(m)。地表より上の場合は正の値を用い、地表下の場合は負の値を用いる。基準となる地表は深さで与えられる、そうでなければ標高で与えられる。</skos:definition>
<skos:example xml:lang="ja"/>
<skos:inScheme rdf:resource="http://rs.gbif.org/terms/dwc/dwc_translations.rdf"/>
<rdf:type rdf:resource="http://www.w3.org/1999/02/22-rdf-syntax-ns#Property"/>
</skos:Concept>
<skos:Concept rdf:about="http://rs.tdwg.org/dwc/terms/minimumElevationInMeters">
<skos:prefLabel xml:lang="en">Minimum Elevation In Meters
		</skos:prefLabel>
<skos:definition xml:lang="en">The lower limit of the range of
			elevation (altitude, usually above sea level), in meters.
		</skos:definition>
<skos:example xml:lang="en">Example: "100"
		</skos:example>
<skos:prefLabel xml:lang="es">Elevación mínima en metros</skos:prefLabel>
<skos:definition xml:lang="es">El límite inferior del rango de
			elevación (altitud, generalmente por encima del nivel del mar), en
			metros. </skos:definition>
<skos:example xml:lang="es">Ejemplo: "100"</skos:example>
<skos:prefLabel xml:lang="zh-Hans">最低海拔（米）</skos:prefLabel>
<skos:definition xml:lang="zh-Hans">海拔（海平面以上的高度）范围的下限，以“米”为单位。</skos:definition>
<skos:example xml:lang="zh-Hans"/>
<skos:prefLabel xml:lang="ja"/>
<skos:definition xml:lang="ja">ある標高の範囲（高度、大抵の場合は海抜）の中の下限値（メートル表記）。</skos:definition>
<skos:example xml:lang="ja"/>
<skos:inScheme rdf:resource="http://rs.gbif.org/terms/dwc/dwc_translations.rdf"/>
<rdf:type rdf:resource="http://www.w3.org/1999/02/22-rdf-syntax-ns#Property"/>
</skos:Concept>
<skos:Concept rdf:about="http://rs.tdwg.org/dwc/terms/month">
<skos:prefLabel xml:lang="en">Month</skos:prefLabel>
<skos:definition xml:lang="en">The ordinal month in which the
			Event
			occurred.</skos:definition>
<skos:example xml:lang="en">Examples: "1"
			(=January), "10" (=October)</skos:example>
<skos:prefLabel xml:lang="es">Mes</skos:prefLabel>
<skos:definition xml:lang="es">El mes ordinal en que ocurrió el
			evento. </skos:definition>
<skos:example xml:lang="es">Ejemplo: "1" (=enero), "10" (=octubre)</skos:example>
<skos:prefLabel xml:lang="zh-Hans">月份</skos:prefLabel>
<skos:definition xml:lang="zh-Hans">事件发生的月份序号。</skos:definition>
<skos:example xml:lang="zh-Hans"/>
<skos:prefLabel xml:lang="ja"/>
<skos:definition xml:lang="ja">イベントが発生した月の序数。</skos:definition>
<skos:example xml:lang="ja"/>
<skos:inScheme rdf:resource="http://rs.gbif.org/terms/dwc/dwc_translations.rdf"/>
<rdf:type rdf:resource="http://www.w3.org/1999/02/22-rdf-syntax-ns#Property"/>
</skos:Concept>
<skos:Concept rdf:about="http://rs.tdwg.org/dwc/terms/municipality">
<skos:prefLabel xml:lang="en">Municipality</skos:prefLabel>
<skos:definition xml:lang="en">The full, unabbreviated name of
			the
			next smaller administrative region than county (city,
			municipality,
			etc.) in which the Location occurs. Do not use this
			term for a nearby
			named place that does not contain the actual
			location.</skos:definition>
<skos:example xml:lang="en">Examples:
			"Holzminden"</skos:example>
<skos:prefLabel xml:lang="es">Municipio</skos:prefLabel>
<skos:definition xml:lang="es">El nombre completo, sin abreviar de la
			siguiente región administrativa de menor jerarquía que condado
			(ciudad, municipio, etc.) en el que la ubicación se produce. No
			utilice este elemento para el nombre de un lugar cercano que no
			contiene la ubicación real. </skos:definition>
<skos:example xml:lang="es">Ejemplo: "Holzminden"</skos:example>
<skos:prefLabel xml:lang="zh-Hans">自治市</skos:prefLabel>
<skos:definition xml:lang="zh-Hans">事件发生的完整、未缩写的地点名称，比县（市、自治区等）更小的行政区域。对于附近不包含实际地点的已命名地区不要使用这个词语。</skos:definition>
<skos:example xml:lang="zh-Hans"/>
<skos:prefLabel xml:lang="ja"/>
<skos:definition xml:lang="ja">その位置が存在する、郡の下位の行政区分（市町村など）の省略されていないフルネーム。実際の位置が含まれない、近接した場所の名前を用いないこと。</skos:definition>
<skos:example xml:lang="ja"/>
<skos:inScheme rdf:resource="http://rs.gbif.org/terms/dwc/dwc_translations.rdf"/>
<rdf:type rdf:resource="http://www.w3.org/1999/02/22-rdf-syntax-ns#Property"/>
</skos:Concept>
<skos:Concept rdf:about="http://rs.tdwg.org/dwc/terms/nameAccordingTo">
<skos:prefLabel xml:lang="en">Name According To</skos:prefLabel>
<skos:definition xml:lang="en">The reference to the source in
			which
			the specific taxon concept circumscription is defined or
			implied -
			traditionally signified by the Latin "sensu" or "sec."
			(from secundum,
			meaning "according to"). For taxa that result from
			identifications, a
			reference to the keys, monographs, experts and
			other sources should be
			given.</skos:definition>
<skos:example xml:lang="en">Example: "McCranie,
			J. R., D. B. Wake, and L.
			D. Wilson. 1996. The taxonomic status of
			Bolitoglossa schmidti, with
			comments on the biology of the
			Mesoamerican salamander Bolitoglossa
			dofleini (Caudata:
			Plethodontidae). Carib. J. Sci. 32:395-398.",
			"Werner Greuter 2008",
			"Lilljeborg 1861, Upsala Univ. Arsskrift, Math.
			Naturvet., pp. 4, 5"
		</skos:example>
<skos:prefLabel xml:lang="es">Nombre de acuerdo con</skos:prefLabel>
<skos:definition xml:lang="es">La referencia a la fuente en la que
			está definida o implícita la circunscripción conceptual del taxón -
			tradicionalmente representado por el Latín "sensu" o "sec." (de
			secundum, que significa "según"). Para los taxones que resultan de
			las identificaciones, una referencia a las claves, monografías,
			expertos y otras fuentes debe ser provista. </skos:definition>
<skos:example xml:lang="es">Ejemplo: "McCranie, J. R., D. B. Wake, and
			L. D. Wilson. 1996. The taxonomic status of Bolitoglossa schmidti,
			with comments on the biology of the Mesoamerican salamander
			Bolitoglossa dofleini (Caudata: Plethodontidae). Carib. J. Sci.
			32:395-398.", "Werner Greuter 2008", "Lilljeborg 1861, Upsala Univ.
			Arsskrift, Math. Naturvet., pp. 4, 5"</skos:example>
<skos:prefLabel xml:lang="zh-Hans">名称依据</skos:prefLabel>
<skos:definition xml:lang="zh-Hans">参考源中定义或暗示了具体类群的概念界限，照惯例表示为拉丁语"sensu"或"sec."（按照依据，意思是“根据”）。对于一个鉴定结果的类群，应给出参考关键词，专题论文，专家及其他资源。</skos:definition>
<skos:example xml:lang="zh-Hans"/>
<skos:prefLabel xml:lang="ja"/>
<skos:definition xml:lang="ja">特定の分類概念の範囲が定義されている、あるいは示唆されている情報源
			(伝統的にラテン語の"sensu"か"sec"("sec"はsecundumの略であり、"according
			to"の意味である)。系統を同定した結果である場合には、その鍵となる文献等を示すべきである。</skos:definition>
<skos:example xml:lang="ja"/>
<skos:inScheme rdf:resource="http://rs.gbif.org/terms/dwc/dwc_translations.rdf"/>
<rdf:type rdf:resource="http://www.w3.org/1999/02/22-rdf-syntax-ns#Property"/>
</skos:Concept>
<skos:Concept rdf:about="http://rs.tdwg.org/dwc/terms/nameAccordingToID">
<skos:prefLabel xml:lang="en">Name According To ID</skos:prefLabel>
<skos:definition xml:lang="en">An identifier for the source in
			which
			the specific taxon concept circumscription is defined or
			implied. See
			nameAccordingTo.</skos:definition>
<skos:example xml:lang="en">Example:
			"doi:10.1016/S0269-915X(97)80026-2"</skos:example>
<skos:prefLabel xml:lang="es">ID nombre de acuerdo con</skos:prefLabel>
<skos:definition xml:lang="es">Un identificador de la fuente en la
			que está definida o implícita la circunscripción conceptual del taxón
			específico. Ver Nombre de acuerdo con. Ejemplo:
			"doi:10.1016/S0269-915X(97)80026-2".</skos:definition>
<skos:example xml:lang="es">Ejemplo: "doi:10.1016/S0269-915X(97)80026-2"</skos:example>
<skos:prefLabel xml:lang="zh-Hans">名称依据编号</skos:prefLabel>
<skos:definition xml:lang="zh-Hans">参考源中定义或暗示具体类群概念界限的标识符，参见“名称依据”。</skos:definition>
<skos:example xml:lang="zh-Hans"/>
<skos:prefLabel xml:lang="ja"/>
<skos:definition xml:lang="ja">特定の分類概念の範囲が定義されている、あるいは示唆されている情報源のID。
			nameAccordingTo を参照のこと。</skos:definition>
<skos:example xml:lang="ja"/>
<skos:inScheme rdf:resource="http://rs.gbif.org/terms/dwc/dwc_translations.rdf"/>
<rdf:type rdf:resource="http://www.w3.org/1999/02/22-rdf-syntax-ns#Property"/>
</skos:Concept>
<skos:Concept rdf:about="http://rs.tdwg.org/dwc/terms/namePublishedIn">
<skos:prefLabel xml:lang="en">Name Published In</skos:prefLabel>
<skos:definition xml:lang="en">A reference for the publication in
			which the scientificName was originally established under the rules
			of the associated nomenclaturalCode.</skos:definition>
<skos:example xml:lang="en">Examples: "Pearson
			O. P., and M. I. Christie.
			1985. Historia Natural, 5(37):388",
			"Forel, Auguste, Diagnosies
			provisoires de quelques espèces nouvelles
			de fourmis de Madagascar,
			récoltées par M. Grandidier., Annales de la
			Societe Entomologique de
			Belgique, Comptes-rendus des Seances 30,
			1886"</skos:example>
<skos:prefLabel xml:lang="es">Nombre publicado en  </skos:prefLabel>
<skos:definition xml:lang="es">Una referencia para la publicación en
			que se estableció originalmente Nombre Científico bajo las reglas del
			Código Nomenclatural asociado. </skos:definition>
<skos:example xml:lang="es">Ejemplo: "Pearson O. P., and M. I. Christie.
			1985. Historia Natural, 5(37):388", "Forel, Auguste, Diagnosies
			provisoires de quelques espèces nouvelles de fourmis de Madagascar,
			récoltées par M. Grandidier., Annales de la Societe Entomologique de
			Belgique, Comptes-rendus des Seances 30, 1886"</skos:example>
<skos:prefLabel xml:lang="zh-Hans">发布名称</skos:prefLabel>
<skos:definition xml:lang="zh-Hans">在相关的命名规则下，确定最初学名的出版参考物。</skos:definition>
<skos:example xml:lang="zh-Hans"/>
<skos:prefLabel xml:lang="ja"/>
<skos:definition xml:lang="ja">関連する nomenclaturalCode
			の規定に従って、その学名が最初に確立された文献への参照。</skos:definition>
<skos:example xml:lang="ja"/>
<skos:inScheme rdf:resource="http://rs.gbif.org/terms/dwc/dwc_translations.rdf"/>
<rdf:type rdf:resource="http://www.w3.org/1999/02/22-rdf-syntax-ns#Property"/>
</skos:Concept>
<skos:Concept rdf:about="http://rs.tdwg.org/dwc/terms/namePublishedInID">
<skos:prefLabel xml:lang="en">Name Published In ID</skos:prefLabel>
<skos:definition xml:lang="en">An identifier for the publication
			in
			which the scientificName was originally established under the
			rules of
			the associated nomenclaturalCode.</skos:definition>
<skos:example xml:lang="en">Example:
			"http://hdl.handle.net/10199/7"</skos:example>
<skos:prefLabel xml:lang="es">ID del nombre publicado en</skos:prefLabel>
<skos:definition xml:lang="es">Un identificador de la publicación en
			que se estableció originalmente Nombre científico bajo las reglas del
			Código nomenclatural asociado. </skos:definition>
<skos:example xml:lang="es">Ejemplo: "http://hdl.handle.net/10199/7"</skos:example>
<skos:prefLabel xml:lang="zh-Hans">名称发布编号</skos:prefLabel>
<skos:definition xml:lang="zh-Hans">在相关的命名规则下，确定最初学名的出版物标识符。</skos:definition>
<skos:example xml:lang="zh-Hans"/>
<skos:prefLabel xml:lang="ja"/>
<skos:definition xml:lang="ja">関連する nomenclaturalCode
			の規定に従って、その学名が最初に確立された文献のID。</skos:definition>
<skos:example xml:lang="ja"/>
<skos:inScheme rdf:resource="http://rs.gbif.org/terms/dwc/dwc_translations.rdf"/>
<rdf:type rdf:resource="http://www.w3.org/1999/02/22-rdf-syntax-ns#Property"/>
</skos:Concept>
<skos:Concept rdf:about="http://rs.tdwg.org/dwc/terms/namePublishedInYear">
<skos:prefLabel xml:lang="en">Name Published In Year</skos:prefLabel>
<skos:definition xml:lang="en">The four-digit year in which the
			scientificName was published.</skos:definition>
<skos:example xml:lang="en">Examples: "1915",
			"2008"</skos:example>
<skos:prefLabel xml:lang="es">Nombre publicado en año</skos:prefLabel>
<skos:definition xml:lang="es">El año de cuatro dígitos en el que se
			publicó el Nombre científico. </skos:definition>
<skos:example xml:lang="es">Ejemplo: "1915", "2008"</skos:example>
<skos:prefLabel xml:lang="zh-Hans">名称发布年份</skos:prefLabel>
<skos:definition xml:lang="zh-Hans">学名发布的四位公历年份。</skos:definition>
<skos:example xml:lang="zh-Hans"/>
<skos:prefLabel xml:lang="ja"/>
<skos:definition xml:lang="ja">その学名が出版された西暦。</skos:definition>
<skos:example xml:lang="ja"/>
<skos:inScheme rdf:resource="http://rs.gbif.org/terms/dwc/dwc_translations.rdf"/>
<rdf:type rdf:resource="http://www.w3.org/1999/02/22-rdf-syntax-ns#Property"/>
</skos:Concept>
<skos:Concept rdf:about="http://rs.tdwg.org/dwc/terms/nomenclaturalCode">
<skos:prefLabel xml:lang="en">Nomenclatural Code</skos:prefLabel>
<skos:definition xml:lang="en">The nomenclatural code (or codes
			in the
			case of an ambiregnal name) under which the scientificName is
			constructed. Recommended best practice is to use a controlled
			vocabulary.</skos:definition>
<skos:example xml:lang="en">Examples: "ICBN",
			"ICZN", "BC", "ICNCP",
			"BioCode", "ICZN; ICBN"</skos:example>
<skos:prefLabel xml:lang="es">Código nomenclatural</skos:prefLabel>
<skos:definition xml:lang="es">El código de nomenclatura (o códigos
			en el caso de un nombre ambireinal) en virtud del cual se construye
			el Nombre Científico. La práctica recomendada es el uso de un
			lenguaje controlado. </skos:definition>
<skos:example xml:lang="es">Ejemplo: "ICBN", "ICZN", "BC", "ICNCP",
			"BioCode", "ICZN; ICBN"</skos:example>
<skos:prefLabel xml:lang="zh-Hans">命名准则</skos:prefLabel>
<skos:definition xml:lang="zh-Hans">创建学名所遵循的命名准则。建议最佳做法是使用一个控制性词汇。</skos:definition>
<skos:example xml:lang="zh-Hans"/>
<skos:prefLabel xml:lang="ja"/>
<skos:definition xml:lang="ja">学名の構成に使用した命名コード（あるいは、ambiregnalな名前の場合は複数のコード）。管理された語彙の使用を推奨。</skos:definition>
<skos:example xml:lang="ja"/>
<skos:inScheme rdf:resource="http://rs.gbif.org/terms/dwc/dwc_translations.rdf"/>
<rdf:type rdf:resource="http://www.w3.org/1999/02/22-rdf-syntax-ns#Property"/>
</skos:Concept>
<skos:Concept rdf:about="http://rs.tdwg.org/dwc/terms/nomenclaturalStatus">
<skos:prefLabel xml:lang="en">Nomenclatural Status</skos:prefLabel>
<skos:definition xml:lang="en">The status related to the original
			publication of the name and its conformance to the relevant rules of
			nomenclature. It is based essentially on an algorithm according to
			the business rules of the code. It requires no taxonomic opinion.
		</skos:definition>
<skos:example xml:lang="en">Examples: "nom.
			ambig.", "nom. illeg.", "nom.
			subnud."</skos:example>
<skos:prefLabel xml:lang="es">Estado nomenclatural</skos:prefLabel>
<skos:definition xml:lang="es">El estatus relacionado con la
			publicación original del nombre y su conformidad con las normas
			pertinentes de nomenclatura. Se basa esencialmente en un algoritmo de
			acuerdo a las reglas de negociación del código. No requiere opinión
			taxonómica. </skos:definition>
<skos:example xml:lang="es">Ejemplos: "nom. ambig.", "nom. illeg.",
			"nom. subnud."</skos:example>
<skos:prefLabel xml:lang="zh-Hans">命名状态</skos:prefLabel>
<skos:definition xml:lang="zh-Hans">与名称的最初出版物相关的状态及与命名相关规则的一致性。本质上基于一个根据业务规则代码的算法，不需要分类的意见。</skos:definition>
<skos:example xml:lang="zh-Hans"/>
<skos:prefLabel xml:lang="ja"/>
<skos:definition xml:lang="ja">名前の最初の出版および、関係のある命名規則との一致に関連した状態。基本的に、コードの業務規則に従ったアルゴリズムに基づくもの。分類に関する意見は不要。</skos:definition>
<skos:example xml:lang="ja"/>
<skos:inScheme rdf:resource="http://rs.gbif.org/terms/dwc/dwc_translations.rdf"/>
<rdf:type rdf:resource="http://www.w3.org/1999/02/22-rdf-syntax-ns#Property"/>
</skos:Concept>
<skos:Concept rdf:about="http://rs.tdwg.org/dwc/terms/occurrenceID">
<skos:prefLabel xml:lang="en">Occurrence ID</skos:prefLabel>
<skos:definition xml:lang="en">An identifier for the Occurrence
			(as
			opposed to a particular digital record of the occurrence). In the
			absence of a persistent global unique identifier, construct one from
			a combination of identifiers in the record that will most closely
			make the occurrenceID globally unique.</skos:definition>
<skos:example xml:lang="en">For a specimen in
			the absence of a bona fide
			global unique identifier, for example, use
			the form:
			"urn:catalog:[institutionCode]:[collectionCode]:[catalogNumber].
			Examples: "urn:lsid:nhm.ku.edu:Herps:32",
			"urn:catalog:FMNH:Mammal:145732"</skos:example>
<skos:prefLabel xml:lang="es">ID del registro biológico</skos:prefLabel>
<skos:definition xml:lang="es">Un identificador del Registro
			biológico (a cambio de un registro digital particular del Registro
			biológico). En ausencia de un identificador único global persistente,
			se debe construir uno a partir de una combinación de identificadores
			en el registro de manera que el ID del registro biológico se aproxime
			a un identificador persistente.</skos:definition>
<skos:example xml:lang="es">En ausencia de un identificador único
			global, puede utilizar la forma: "urn:catálogo:[código
			institución]:[código colección]:[número catálogo]. Ejemplos:
			"urn:lsid:nhm.ku.edu:Herps:32", "urn:catalog:FMNH:Mammal:145732"</skos:example>
<skos:prefLabel xml:lang="zh-Hans">事件编号</skos:prefLabel>
<skos:definition xml:lang="zh-Hans">一个事件的标识符（并非一个事件的具体数字记录）。在缺乏全局唯一标识符的情况下，从最接近全局唯一事件编号的记录中构建一个标识符。</skos:definition>
<skos:example xml:lang="zh-Hans"/>
<skos:prefLabel xml:lang="ja"/>
<skos:definition xml:lang="ja">出来事についてのID
			(特定の電子レコードに対する)。GUIDが存在しない場合には、出来るだけグローバルにユニークになるようにレコードのIDを組み合わせたものを作成する。</skos:definition>
<skos:example xml:lang="ja">真なるGUIDが無い表hん野場合には、例えば以下のようなフォームを使う:
			"urn:catalog:[institutionCode]:[collectionCode]:[catalogNumber].
			Examples: "urn:lsid:nhm.ku.edu:Herps:32",
			"urn:catalog:FMNH:Mammal:145732"</skos:example>
<skos:inScheme rdf:resource="http://rs.gbif.org/terms/dwc/dwc_translations.rdf"/>
<rdf:type rdf:resource="http://www.w3.org/1999/02/22-rdf-syntax-ns#Property"/>
</skos:Concept>
<skos:Concept rdf:about="http://rs.tdwg.org/dwc/terms/occurrenceRemarks">
<skos:prefLabel xml:lang="en">Occurrence Remarks</skos:prefLabel>
<skos:definition xml:lang="en">Comments or notes about the
			Occurrence.</skos:definition>
<skos:example xml:lang="en">Example: "found dead
			on road"</skos:example>
<skos:prefLabel xml:lang="es">Comentarios del registro biológico</skos:prefLabel>
<skos:definition xml:lang="es">Comentarios o anotaciones sobre el
			Registro Biológico. </skos:definition>
<skos:example xml:lang="es">Ejemplo: "muerto en la vía"</skos:example>
<skos:prefLabel xml:lang="zh-Hans">事件备注</skos:prefLabel>
<skos:definition xml:lang="zh-Hans">关于这个事件的评论和注释。</skos:definition>
<skos:example xml:lang="zh-Hans"/>
<skos:prefLabel xml:lang="ja"/>
<skos:definition xml:lang="ja">出来事についてのコメントまたは注釈。</skos:definition>
<skos:example xml:lang="ja"/>
<skos:inScheme rdf:resource="http://rs.gbif.org/terms/dwc/dwc_translations.rdf"/>
<rdf:type rdf:resource="http://www.w3.org/1999/02/22-rdf-syntax-ns#Property"/>
</skos:Concept>
<skos:Concept rdf:about="http://rs.tdwg.org/dwc/terms/occurrenceStatus">
<skos:prefLabel xml:lang="en">Occurrence Status</skos:prefLabel>
<skos:definition xml:lang="en">A statement about the presence or
			absence of a Taxon at a Location. Recommended best practice is to use
			a controlled vocabulary.</skos:definition>
<skos:example xml:lang="en">Examples: "present",
			"absent"</skos:example>
<skos:prefLabel xml:lang="es">Estado del registro biológico</skos:prefLabel>
<skos:definition xml:lang="es">Una declaración sobre la presencia o
			ausencia de un taxón en una ubicación. La práctica recomendada es el
			uso de un lenguaje controlado. </skos:definition>
<skos:example xml:lang="es">Ejemplo: "presente", "ausente"</skos:example>
<skos:prefLabel xml:lang="zh-Hans">事件状态</skos:prefLabel>
<skos:definition xml:lang="zh-Hans">关于一个类群在一个地点存在或者不存在的声明。建议最佳做法是使用一个控制性词汇。</skos:definition>
<skos:example xml:lang="zh-Hans"/>
<skos:prefLabel xml:lang="ja"/>
<skos:definition xml:lang="ja">その位置における、ある分類群の存在または不在についての声明。管理された語彙の使用を推奨。</skos:definition>
<skos:example xml:lang="ja"/>
<skos:inScheme rdf:resource="http://rs.gbif.org/terms/dwc/dwc_translations.rdf"/>
<rdf:type rdf:resource="http://www.w3.org/1999/02/22-rdf-syntax-ns#Property"/>
</skos:Concept>
<skos:Concept rdf:about="http://rs.tdwg.org/dwc/terms/order">
<skos:prefLabel xml:lang="en">Order</skos:prefLabel>
<skos:definition xml:lang="en">The full scientific name of the
			order
			in which the taxon is classified.</skos:definition>
<skos:example xml:lang="en">Example:
			"Carnivora", "Monocleales"</skos:example>
<skos:prefLabel xml:lang="es">Orden</skos:prefLabel>
<skos:definition xml:lang="es">El nombre científico completo del
			orden en el que se clasifica el taxón. </skos:definition>
<skos:example xml:lang="es">Ejemplo: "Carnivora", "Monocleales"</skos:example>
<skos:prefLabel xml:lang="zh-Hans">目</skos:prefLabel>
<skos:definition xml:lang="zh-Hans">分类单元所属目的完整学名。</skos:definition>
<skos:example xml:lang="zh-Hans"/>
<skos:prefLabel xml:lang="ja"/>
<skos:definition xml:lang="ja">その分類群が位置づけられている、分類上の「目」のフルネーム。</skos:definition>
<skos:example xml:lang="ja"/>
<skos:inScheme rdf:resource="http://rs.gbif.org/terms/dwc/dwc_translations.rdf"/>
<rdf:type rdf:resource="http://www.w3.org/1999/02/22-rdf-syntax-ns#Property"/>
</skos:Concept>
<skos:Concept rdf:about="http://rs.tdwg.org/dwc/terms/originalNameUsage">
<skos:prefLabel xml:lang="en">Original Name Usage</skos:prefLabel>
<skos:definition xml:lang="en">The taxon name, with authorship
			and
			date information if known, as it originally appeared when first
			established under the rules of the associated nomenclaturalCode. The
			basionym (botany) or basonym (bacteriology) of the scientificName or
			the senior/earlier homonym for replaced names.</skos:definition>
<skos:example xml:lang="en">Example: "Pinus
			abies", "Gasterosteus
			saltatrix Linnaeus 1768"</skos:example>
<skos:prefLabel xml:lang="es">Uso del nombre original</skos:prefLabel>
<skos:definition xml:lang="es">El nombre del taxón, con información
			de autoría y fecha si se conoce, tal como apareció originalmente
			cuando se estableció por primera vez bajo las reglas del Código
			Nomenclatural asociadas. El basiónimo (botánica) o basiónimo
			(bacteriología) de Nombre Científico o el homónimo anterior de los
			nombres sustituidos. </skos:definition>
<skos:example xml:lang="es">Ejemplo: "Pinus abies", "Gasterosteus
			saltatrix Linnaeus 1768"</skos:example>
<skos:prefLabel xml:lang="zh-Hans">最初使用名称</skos:prefLabel>
<skos:definition xml:lang="zh-Hans">在相关的命名规则下第一次被建立的最初出现的类群名称，如果知道的话，附作者和日期信息。学名的异名或基名，或用来替换名称的同音词。</skos:definition>
<skos:example xml:lang="zh-Hans"/>
<skos:prefLabel xml:lang="ja"/>
<skos:definition xml:lang="ja">関連するnomenclaturalCodeの規定に従って最初に記述された系統名と著者、日付の情報。植物学か微生物学におけるscientificNameか、取って代わられた同音異義語など。</skos:definition>
<skos:example xml:lang="ja"/>
<skos:inScheme rdf:resource="http://rs.gbif.org/terms/dwc/dwc_translations.rdf"/>
<rdf:type rdf:resource="http://www.w3.org/1999/02/22-rdf-syntax-ns#Property"/>
</skos:Concept>
<skos:Concept rdf:about="http://rs.tdwg.org/dwc/terms/originalNameUsageID">
<skos:prefLabel xml:lang="en">Original Name Usage ID</skos:prefLabel>
<skos:definition xml:lang="en">An identifier for the name usage
			(documented meaning of the name according to a source) in which the
			terminal element of the scientificName was originally established
			under the rules of the associated nomenclaturalCode.</skos:definition>
<skos:example xml:lang="en">Example:
			"http://species.gbif.org/abies_alba_1753"</skos:example>
<skos:prefLabel xml:lang="es">ID del uso del nombre original</skos:prefLabel>
<skos:definition xml:lang="es">Un identificador para el uso del
			nombre (significado documentado del nombre de acuerdo a una fuente)
			en el que se estableció originalmente, el elemento terminal de Nombre
			Científico bajo las reglas del Código Nomenclatural asociado. </skos:definition>
<skos:example xml:lang="es">Ejemplo:
			"http://species.gbif.org/abies_alba_1753"</skos:example>
<skos:prefLabel xml:lang="zh-Hans">最初使用名称编号</skos:prefLabel>
<skos:definition xml:lang="zh-Hans">学名在相关命名规则下最初建立时，学名的末端组成上的名称使用标识符。</skos:definition>
<skos:example xml:lang="zh-Hans"/>
<skos:prefLabel xml:lang="ja"/>
<skos:definition xml:lang="ja">関連する nomencluaturalCode
			に従って学名の末端要素が最初に確立されたときに使用された、名前の使用法（情報源に従った名前の、文書化された意味）のID。</skos:definition>
<skos:example xml:lang="ja"/>
<skos:inScheme rdf:resource="http://rs.gbif.org/terms/dwc/dwc_translations.rdf"/>
<rdf:type rdf:resource="http://www.w3.org/1999/02/22-rdf-syntax-ns#Property"/>
</skos:Concept>
<skos:Concept rdf:about="http://rs.tdwg.org/dwc/terms/otherCatalogNumbers">
<skos:prefLabel xml:lang="en">Other Catalog Numbers</skos:prefLabel>
<skos:definition xml:lang="en">A list (concatenated and
			separated) of
			previous or alternate fully qualified catalog numbers
			or other
			human-used identifiers for the same Occurrence, whether in
			the current
			or any other data set or collection.</skos:definition>
<skos:example xml:lang="en">Example:
			"FMNH:Mammal:1234", "NPS YELLO6778;
			MBG 33424"</skos:example>
<skos:prefLabel xml:lang="es">Otros números de catálogo</skos:prefLabel>
<skos:definition xml:lang="es">Una lista (concatenada y separada) de
			números de catálogos anteriores o alternativos, calificados, u otros
			identificadores de uso humano para el mismo Registro Biológico, ya
			sea en el actual o cualquier otro conjunto de datos o colección. </skos:definition>
<skos:example xml:lang="es">Ejemplo: "FMNH:Mammal:1234", "NPS YELLO6778;
			MBG 33424"</skos:example>
<skos:prefLabel xml:lang="zh-Hans">其它目录编号</skos:prefLabel>
<skos:definition xml:lang="zh-Hans">无论在当前或其他任何数据集，同一事件中以前或备用的完全合格的目录号或其他人使用的标识符列表（连接的或分开的）。</skos:definition>
<skos:example xml:lang="zh-Hans"/>
<skos:prefLabel xml:lang="ja"/>
<skos:definition xml:lang="ja">同じ出来事（現在のものであっても、他のデータセットやコレクションであっても）に関する、以前の、または代わりのカタログナンバー（省略なし）、あるいは他のIDのリスト。</skos:definition>
<skos:example xml:lang="ja"/>
<skos:inScheme rdf:resource="http://rs.gbif.org/terms/dwc/dwc_translations.rdf"/>
<rdf:type rdf:resource="http://www.w3.org/1999/02/22-rdf-syntax-ns#Property"/>
</skos:Concept>
<skos:Concept rdf:about="http://rs.tdwg.org/dwc/terms/ownerInstitutionCode">
<skos:prefLabel xml:lang="en">Owner Institution Code</skos:prefLabel>
<skos:definition xml:lang="en">The name (or acronym) in use by
			the
			institution having ownership of the object(s) or information
			referred
			to in the record.</skos:definition>
<skos:example xml:lang="en">Examples: "NPS",
			"APN", "InBio"</skos:example>
<skos:prefLabel xml:lang="es">Código de la institución propietaria</skos:prefLabel>
<skos:definition xml:lang="es">El nombre (o acrónimo) en uso por la
			institución que tiene la propiedad del objeto(s) o información
			referida en el registro. </skos:definition>
<skos:example xml:lang="es">Ejemplo: "NPS", "APN", "InBio"</skos:example>
<skos:prefLabel xml:lang="zh-Hans">所有者机构代码</skos:prefLabel>
<skos:definition xml:lang="zh-Hans">记录中显示的对物品或信息享有所有权的机构名称（或缩写）。</skos:definition>
<skos:example xml:lang="zh-Hans"/>
<skos:prefLabel xml:lang="ja"/>
<skos:definition xml:lang="ja">そのレコードの物あるいは情報を所有している機関の名前（または頭字語）。</skos:definition>
<skos:example xml:lang="ja"/>
<skos:inScheme rdf:resource="http://rs.gbif.org/terms/dwc/dwc_translations.rdf"/>
<rdf:type rdf:resource="http://www.w3.org/1999/02/22-rdf-syntax-ns#Property"/>
</skos:Concept>
<skos:Concept rdf:about="http://rs.tdwg.org/dwc/terms/parentNameUsage">
<skos:prefLabel xml:lang="en">Parent Name Usage</skos:prefLabel>
<skos:definition xml:lang="en">The full name, with authorship and
			date information if known, of the direct, most proximate higher-rank
			parent taxon (in a classification) of the most specific element of
			the scientificName.</skos:definition>
<skos:example xml:lang="en">Examples:
			"Rubiaceae", "Gruiformes",
			"Testudinae"</skos:example>
<skos:prefLabel xml:lang="es">Uso del nombre parental</skos:prefLabel>
<skos:definition xml:lang="es">El nombre completo, con información de
			autoría y fecha si se conoce, del taxón parental directo más próximo
			de nivel superior (en una clasificación) del elemento más específico
			de Nombre Científico. </skos:definition>
<skos:example xml:lang="es">Ejemplo: "Rubiaceae", "Gruiformes",
			"Testudinae"</skos:example>
<skos:prefLabel xml:lang="zh-Hans">上一级使用名称</skos:prefLabel>
<skos:definition xml:lang="zh-Hans">学名的最直接的上一级母类别的完整名称，如果已知，附带作者和日期信息。</skos:definition>
<skos:example xml:lang="zh-Hans"/>
<skos:prefLabel xml:lang="ja"/>
<skos:definition xml:lang="ja">学名の特有の要素に対する、直接かつ最も近縁な上位階層の分類群のフルネーム（もし分かるなら著者と日付情報を付記したもの）。</skos:definition>
<skos:example xml:lang="ja"/>
<skos:inScheme rdf:resource="http://rs.gbif.org/terms/dwc/dwc_translations.rdf"/>
<rdf:type rdf:resource="http://www.w3.org/1999/02/22-rdf-syntax-ns#Property"/>
</skos:Concept>
<skos:Concept rdf:about="http://rs.tdwg.org/dwc/terms/parentNameUsageID">
<skos:prefLabel xml:lang="en">Parent Name Usage ID</skos:prefLabel>
<skos:definition xml:lang="en">An identifier for the name usage
			(documented meaning of the name according to a source) of the direct,
			most proximate higher-rank parent taxon (in a classification) of the
			most specific element of the scientificName.</skos:definition>
<skos:example xml:lang="en">Example:
			"8fa58e08-08de-4ac1-b69c-1235340b7001"</skos:example>
<skos:prefLabel xml:lang="es">ID del uso del nombre parental</skos:prefLabel>
<skos:definition xml:lang="es">Un identificador para el uso del
			nombre (significado documentado del nombre de acuerdo a una fuente)
			del taxón parental directo, más próximo de nivel superior (en una
			clasificación) del elemento más específico de Nombre Científico. </skos:definition>
<skos:example xml:lang="es">Ejemplo:
			"8fa58e08-08de-4ac1-b69c-1235340b7001"</skos:example>
<skos:prefLabel xml:lang="zh-Hans">上一级使用名称编号</skos:prefLabel>
<skos:definition xml:lang="zh-Hans">学名最直接的上一级母类别的名称用法的标识符。</skos:definition>
<skos:example xml:lang="zh-Hans"/>
<skos:prefLabel xml:lang="ja"/>
<skos:definition xml:lang="ja">学名の特有の要素に対する、直接かつ最も近縁な高位の分類群の名前使用法（情報源に従った名前の、文書化された意味）のID。</skos:definition>
<skos:example xml:lang="ja"/>
<skos:inScheme rdf:resource="http://rs.gbif.org/terms/dwc/dwc_translations.rdf"/>
<rdf:type rdf:resource="http://www.w3.org/1999/02/22-rdf-syntax-ns#Property"/>
</skos:Concept>
<skos:Concept rdf:about="http://rs.tdwg.org/dwc/terms/phylum">
<skos:prefLabel xml:lang="en">Phylum</skos:prefLabel>
<skos:definition xml:lang="en">The full scientific name of the
			phylum
			or division in which the taxon is classified.</skos:definition>
<skos:example xml:lang="en">Example: "Chordata"
			(phylum), "Bryophyta"
			(division)</skos:example>
<skos:prefLabel xml:lang="es">Filo</skos:prefLabel>
<skos:definition xml:lang="es">El nombre científico completo del filo
			o división en el que se clasifica el taxón. </skos:definition>
<skos:example xml:lang="es">Ejemplo: "Chordata" (filo), "Bryophyta"
			(división)</skos:example>
<skos:prefLabel xml:lang="zh-Hans">门</skos:prefLabel>
<skos:definition xml:lang="zh-Hans">分类单元所属门的完整学名。</skos:definition>
<skos:example xml:lang="zh-Hans"/>
<skos:prefLabel xml:lang="ja"/>
<skos:definition xml:lang="ja">その分類群が位置づけられている、分類上の「門」（phylumまたはdivision）のフルネーム。</skos:definition>
<skos:example xml:lang="ja"/>
<skos:inScheme rdf:resource="http://rs.gbif.org/terms/dwc/dwc_translations.rdf"/>
<rdf:type rdf:resource="http://www.w3.org/1999/02/22-rdf-syntax-ns#Property"/>
</skos:Concept>
<skos:Concept rdf:about="http://rs.tdwg.org/dwc/terms/pointRadiusSpatialFit">
<skos:prefLabel xml:lang="en">Point Radius Spatial Fit</skos:prefLabel>
<skos:definition xml:lang="en">The ratio of the area of the
			point-radius (decimalLatitude, decimalLongitude,
			coordinateUncertaintyInMeters) to the area of the true (original, or
			most specific) spatial representation of the Location. Legal values
			are 0, greater than or equal to 1, or undefined. A value of 1 is an
			exact match or 100% overlap. A value of 0 should be used if the given
			point-radius does not completely contain the original representation.
			The pointRadiusSpatialFit is undefined (and should be left blank) if
			the original representation is a point without uncertainty and the
			given georeference is not that same point (without uncertainty). If
			both the original and the given georeference are the same point, the
			pointRadiusSpatialFit is 1.</skos:definition>
<skos:example xml:lang="en">Detailed
			explanations with graphical examples
			can be found in the "Guide to
			Best Practices for Georeferencing",
			Chapman and Wieczorek, eds. 2006
			(http://www.gbif.org/prog/digit/Georeferencing).
		</skos:example>
<skos:prefLabel xml:lang="es">Ajuste espacial del radio-punto</skos:prefLabel>
<skos:definition xml:lang="es">La relación entre el área del
			radio-punto (Latitud Decimal, Longitud Decimal e Incertidumbre
			Coordenadas en Metros) y el área de la verdadera (original, o de
			mayor especificidad) representación espacial de la ubicación. Los
			valores válidos son 0, mayor que o igual a 1, o indefinido. Un valor
			de 1 es una coincidencia exacta o superposición de 100%. Un valor de
			0 se debe utilizar si el radio-punto dado no contiene por completo la
			representación original. El Ajuste Espacial de Radio-Punto no está
			definido (y se debe dejar en blanco) si la representación original es
			un punto sin incertidumbre y la georreferencia dada no es ese mismo
			punto (sin incertidumbre). Si tanto el original como la
			georreferencia dada están en el mismo punto, el Ajuste Espacial de
			Radio-Punto es 1. </skos:definition>
<skos:example xml:lang="es">Explicaciones detalladas con ejemplos
			gráficos disponibles en el documento "Guide to Best Practices for
			Georeferencing", Chapman and Wieczorek, eds. 2006
			(http://www.gbif.org/prog/digit/Georeferencing). </skos:example>
<skos:prefLabel xml:lang="zh-Hans">点半径空间拟合</skos:prefLabel>
<skos:definition xml:lang="zh-Hans">采集地点点半径（十进制纬度，十进制经度，以米为单位的坐标不确定性）面积与真正（最初或最具体）所用空间面积的比率。合法值是0，或大于等于1，或未定义。值为1时表示两者精确匹配或100%重叠。值为0时表示给定的点半径不完全包含最初地域。如果最初地域是一个点而给定的地理参考是另外一个点，那么点半径空间拟合值未定义（应该留白）。如果最初地域与给定的地理参考是同一个点，则点半径空间拟合值为1。</skos:definition>
<skos:example xml:lang="zh-Hans"/>
<skos:prefLabel xml:lang="ja"/>
<skos:definition xml:lang="ja">その場所の空間表現をする際の等半径点(decimalLatitude,
			decimalLongitude, coordinateUncertaintyInMeters)の領域の割合。値としては0,
			1または1以下1以上,未定義が入力可能。1は完全一致、0は等半径点が元の位置を全くカバーしていない場合に用いる。この値は、元の位置が地理参照で全くカバーされていない場合には、値を未定義として空欄にすべきである。もし元の位置と地理参照が完全に一致した場合は、この値は1となる。</skos:definition>
<skos:example xml:lang="ja">視覚的な例つきの詳細な説明は "Guide to Best Practices for
			Georeferencing", Chapman and
			Wieczorek, eds. 2006 (http://www.gbif.org/prog/digit/Georeferencing).</skos:example>
<skos:inScheme rdf:resource="http://rs.gbif.org/terms/dwc/dwc_translations.rdf"/>
<rdf:type rdf:resource="http://www.w3.org/1999/02/22-rdf-syntax-ns#Property"/>
</skos:Concept>
<skos:Concept rdf:about="http://rs.tdwg.org/dwc/terms/preparations">
<skos:prefLabel xml:lang="en">Preparations</skos:prefLabel>
<skos:definition xml:lang="en">A list (concatenated and
			separated) of
			preparations and preservation methods for a specimen.
		</skos:definition>
<skos:example xml:lang="en">Examples: "skin;
			skull; skeleton", "whole
			animal (ETOH); tissue (EDTA)", "fossil",
			"cast", "photograph", "DNA
			extract"</skos:example>
<skos:prefLabel xml:lang="es">Preparaciones</skos:prefLabel>
<skos:definition xml:lang="es">Una lista (concatenada y separada) de
			las preparaciones y los métodos de conservación de una muestra. </skos:definition>
<skos:example xml:lang="es">Ejemplo: "piel; cráneo; esqueleto", "animal
			entero (ETOH - Etanol); tejido (EDTA - ácido
			etilendiaminotetraacético)", "fósil", "molde", "fotografía",
			"extracto de ADN"</skos:example>
<skos:prefLabel xml:lang="zh-Hans">准备</skos:prefLabel>
<skos:definition xml:lang="zh-Hans">关于样本的准备和保存的列表(连接的或分开的)。</skos:definition>
<skos:example xml:lang="zh-Hans"/>
<skos:prefLabel xml:lang="ja"/>
<skos:definition xml:lang="ja">標本の調整および保存方法のリスト。</skos:definition>
<skos:example xml:lang="ja"/>
<skos:inScheme rdf:resource="http://rs.gbif.org/terms/dwc/dwc_translations.rdf"/>
<rdf:type rdf:resource="http://www.w3.org/1999/02/22-rdf-syntax-ns#Property"/>
</skos:Concept>
<skos:Concept rdf:about="http://rs.tdwg.org/dwc/terms/previousIdentifications">
<skos:prefLabel xml:lang="en">Previous Identifications</skos:prefLabel>
<skos:definition xml:lang="en">A list (concatenated and
			separated) of
			previous assignments of names to the Occurrence.
		</skos:definition>
<skos:example xml:lang="en">Example: "Anthus
			sp., field ID by G.
			Iglesias; Anthus correndera, expert ID by C.
			Cicero 2009-02-12 based
			on morphology"</skos:example>
<skos:prefLabel xml:lang="es">Identificaciones previas</skos:prefLabel>
<skos:definition xml:lang="es">Una lista (concatenada y separada) de
			asignaciones anteriores de nombres al Registro Biológico. </skos:definition>
<skos:example xml:lang="es">Ejemplo: "Anthus sp., identificado en campo
			por G. Iglesias; Anthus correndera, ID del experto por C. Cicero
			2009-02-12 basado en morfología"</skos:example>
<skos:prefLabel xml:lang="zh-Hans">以前的鉴定</skos:prefLabel>
<skos:definition xml:lang="zh-Hans">事件的以前鉴定的名称列表(连接的或分开的)。</skos:definition>
<skos:example xml:lang="zh-Hans"/>
<skos:prefLabel xml:lang="ja"/>
<skos:definition xml:lang="ja">その出来事に以前割り当てられた名前のリスト。</skos:definition>
<skos:example xml:lang="ja"/>
<skos:inScheme rdf:resource="http://rs.gbif.org/terms/dwc/dwc_translations.rdf"/>
<rdf:type rdf:resource="http://www.w3.org/1999/02/22-rdf-syntax-ns#Property"/>
</skos:Concept>
<skos:Concept rdf:about="http://rs.tdwg.org/dwc/terms/recordedBy">
<skos:prefLabel xml:lang="en">Recorded By</skos:prefLabel>
<skos:definition xml:lang="en">A list (concatenated and
			separated) of
			names of people, groups, or organizations responsible
			for recording
			the original Occurrence. The primary collector or
			observer, especially
			one who applies a personal identifier
			(recordNumber), should be listed
			first.</skos:definition>
<skos:example xml:lang="en">Example: "Oliver P.
			Pearson; Anita K.
			Pearson" where the value in recordNumber "OPP 7101"
			corresponds to the
			number for the specimen in the field catalog
			(collector number) of
			Oliver P. Pearson.</skos:example>
<skos:prefLabel xml:lang="es">Registrado por</skos:prefLabel>
<skos:definition xml:lang="es">Una lista (concatenada y separada) de
			los nombres de las personas, grupos u organizaciones responsables de
			registrar el Registro Biológico. El colector u observador principal,
			especialmente uno que aplica un identificador personal (Número del
			Registro), se debe listar en primer lugar. </skos:definition>
<skos:example xml:lang="es">Ejemplo: "Oliver P. Pearson; Anita K.
			Pearson" donde el valor en Número del Registro "OPP 7101" corresponde
			al número para el espécimen en el catálogo de campo (número de
			colector) de Oliver P. Pearson.</skos:example>
<skos:prefLabel xml:lang="zh-Hans">记录者</skos:prefLabel>
<skos:definition xml:lang="zh-Hans">记录原始事件中的人名，群体或者组织的列表（连接的或分开的）。主要的采集员或者观察员，尤其是申请了个人标识符（纪录号）的应列在第一位。</skos:definition>
<skos:example xml:lang="zh-Hans"/>
<skos:prefLabel xml:lang="ja"/>
<skos:definition xml:lang="ja">その出来事を記録したことについて責任を持つ人の名前またはグループ、組織のリスト。実際に収集した人や観察した人、特にrecordNumberを割り振った人等は最初に記述されるべきである。</skos:definition>
<skos:example xml:lang="ja"/>
<skos:inScheme rdf:resource="http://rs.gbif.org/terms/dwc/dwc_translations.rdf"/>
<rdf:type rdf:resource="http://www.w3.org/1999/02/22-rdf-syntax-ns#Property"/>
</skos:Concept>
<skos:Concept rdf:about="http://rs.tdwg.org/dwc/terms/recordNumber">
<skos:prefLabel xml:lang="en">Record Number</skos:prefLabel>
<skos:definition xml:lang="en">An identifier given to the
			Occurrence
			at the time it was recorded. Often serves as a link
			between field
			notes and an Occurrence record, such as a specimen
			collector's number.</skos:definition>
<skos:example xml:lang="en">Example: "OPP 7101"
		</skos:example>
<skos:prefLabel xml:lang="es">Número de registro</skos:prefLabel>
<skos:definition xml:lang="es">Un identificador dado al Registro
			Biológico en el momento en que fue registrada. A menudo sirve como un
			vínculo entre las anotaciones de campo y el registro de un Registro
			Biológico, como el número de un colector de especímenes. </skos:definition>
<skos:example xml:lang="es">Ejemplo: "OPP 7101"</skos:example>
<skos:prefLabel xml:lang="zh-Hans">记录号</skos:prefLabel>
<skos:definition xml:lang="zh-Hans">给出事件被纪录的时间的标识符，通常是现场纪录和事件纪录的联系，例如样本采集者的编号。</skos:definition>
<skos:example xml:lang="zh-Hans"/>
<skos:prefLabel xml:lang="ja"/>
<skos:definition xml:lang="ja">その出来事のレコードが作成されたときに与えられるID。標本所持者の番号など、フィールドノートと出来事のレコード間をリンクする役割を果たすもの。</skos:definition>
<skos:example xml:lang="ja"/>
<skos:inScheme rdf:resource="http://rs.gbif.org/terms/dwc/dwc_translations.rdf"/>
<rdf:type rdf:resource="http://www.w3.org/1999/02/22-rdf-syntax-ns#Property"/>
</skos:Concept>
<skos:Concept rdf:about="http://rs.tdwg.org/dwc/terms/relatedResourceID">
<skos:prefLabel xml:lang="en">Related Resource ID</skos:prefLabel>
<skos:definition xml:lang="en">An identifier for a related
			resource
			(the object, rather than the subject of the relationship).
		</skos:definition>
<skos:example xml:lang="en"/>
<skos:prefLabel xml:lang="es">ID del recurso relacionado</skos:prefLabel>
<skos:definition xml:lang="es">Un identificador para un recurso
			relacionado (el objeto, en lugar del sujeto de la relación). </skos:definition>
<skos:example xml:lang="es"/>
<skos:prefLabel xml:lang="zh-Hans">相关资源编号</skos:prefLabel>
<skos:definition xml:lang="zh-Hans">相关资源的标识符（客体，而非关系主体）。</skos:definition>
<skos:example xml:lang="zh-Hans"/>
<skos:prefLabel xml:lang="ja"/>
<skos:definition xml:lang="ja">関連する資料関係性の主語ではなく、目的語）のID。</skos:definition>
<skos:example xml:lang="ja"/>
<skos:inScheme rdf:resource="http://rs.gbif.org/terms/dwc/dwc_translations.rdf"/>
<rdf:type rdf:resource="http://www.w3.org/1999/02/22-rdf-syntax-ns#Property"/>
</skos:Concept>
<skos:Concept rdf:about="http://rs.tdwg.org/dwc/terms/relationshipAccordingTo">
<skos:prefLabel xml:lang="en">Relationship According To</skos:prefLabel>
<skos:definition xml:lang="en">The source (person, organization,
			publication, reference) establishing the relationship between the two
			resources.</skos:definition>
<skos:example xml:lang="en">Example: "Julie
			Woodruff"</skos:example>
<skos:prefLabel xml:lang="es">Relación de acuerdo con</skos:prefLabel>
<skos:definition xml:lang="es">La fuente (persona, organización,
			publicación, referencia) que establece la relación entre los dos
			recursos. </skos:definition>
<skos:example xml:lang="es">Ejemplo: "Julie Woodruff"</skos:example>
<skos:prefLabel xml:lang="zh-Hans">关系依据</skos:prefLabel>
<skos:definition xml:lang="zh-Hans">在两种资源间建立关系的来源（人，组织，出版物，参考）。</skos:definition>
<skos:example xml:lang="zh-Hans"/>
<skos:prefLabel xml:lang="ja"/>
<skos:definition xml:lang="ja">２つの資料間の関係性を確立した情報源（人物、組織、出版物、参考文献など）。</skos:definition>
<skos:example xml:lang="ja"/>
<skos:inScheme rdf:resource="http://rs.gbif.org/terms/dwc/dwc_translations.rdf"/>
<rdf:type rdf:resource="http://www.w3.org/1999/02/22-rdf-syntax-ns#Property"/>
</skos:Concept>
<skos:Concept rdf:about="http://rs.tdwg.org/dwc/terms/relationshipEstablishedDate">
<skos:prefLabel xml:lang="en">Relationship Established Date
		</skos:prefLabel>
<skos:definition xml:lang="en">The date-time on which the
			relationship between the two resources was established. Recommended
			best practice is to use an encoding scheme, such as ISO 8601:2004(E).
		</skos:definition>
<skos:example xml:lang="en">Examples:
			"1963-03-08T14:07-0600" is 8 Mar
			1963 2:07pm in the time zone six
			hours earlier than UTC,
			"2009-02-20T08:40Z" is 20 Feb 2009 8:40am
			UTC, "1809-02-12" is 12 Feb
			1809, "1906-06" is Jun 1906, "1971" is
			just that year,
			"2007-03-01T13:00:00Z/2008-05-11T15:30:00Z" is the
			interval between 1
			Mar 2007 1pm UTC and 11 May 2008 3:30pm UTC,
			"2007-11-13/15" is the
			interval between 13 Nov 2007 and 15 Nov 2007.
		</skos:example>
<skos:prefLabel xml:lang="es">Fecha de establecimiento de la relación</skos:prefLabel>
<skos:definition xml:lang="es">La fecha y hora en que se estableció
			la relación entre los dos recursos. La práctica recomendada es
			utilizar un esquema de codificación, tal como ISO 8601:2004 (E). </skos:definition>
<skos:example xml:lang="es">Ejemplos: "1963-03-08T14:07-0600" es 8 de
			marzo de 1963 2:07pm en zona horaria seis horas más temprano que UTC,
			"2009-02-20T08:40Z" es 20 de febrero 2009 8:40am UTC, "1809-02-12" es
			12 de febrero de 1809, "1906-06" es junio de 1906, "1971",
			"2007-03-01T13:00:00Z/2008-05-11T15:30:00Z" es el intervalo entre el
			1 de marzo de 2007 1pm UTC y 11 de mayo de 2008 3:30pm UTC,
			"2007-11-13/15" es el intervalo entre el 13 de noviembre de 2007 y 15
			de noviembre de 2007.</skos:example>
<skos:prefLabel xml:lang="zh-Hans">关系确定日期</skos:prefLabel>
<skos:definition xml:lang="zh-Hans">在两种资源间建立的关系的日期。建议最佳做法是使用一个编码方案，例如ISO
			8601:2004(E)。</skos:definition>
<skos:example xml:lang="zh-Hans"/>
<skos:prefLabel xml:lang="ja"/>
<skos:definition xml:lang="ja">２つの資料間の関係性を確立した日時。 ISO
			8601:2004(E)などのスキーマの使用を推奨。</skos:definition>
<skos:example xml:lang="ja"/>
<skos:inScheme rdf:resource="http://rs.gbif.org/terms/dwc/dwc_translations.rdf"/>
<rdf:type rdf:resource="http://www.w3.org/1999/02/22-rdf-syntax-ns#Property"/>
</skos:Concept>
<skos:Concept rdf:about="http://rs.tdwg.org/dwc/terms/relationshipOfResource">
<skos:prefLabel xml:lang="en">Relationship Of Resource</skos:prefLabel>
<skos:definition xml:lang="en">The relationship of the resource
			identified by relatedResourceID to the subject (optionally identified
			by the resourceID). Recommended best practice is to use a controlled
			vocabulary.</skos:definition>
<skos:example xml:lang="en">Examples: "duplicate
			of", "mother of",
			"endoparasite of", "host to", "sibling of", "valid
			synonym of",
			"located within"</skos:example>
<skos:prefLabel xml:lang="es">Recurso de la relación</skos:prefLabel>
<skos:definition xml:lang="es">La relación del recurso identificado
			por ID del Recurso Relacionado con el sujeto (opcionalmente
			identificado por ID del Recurso). La práctica recomendada es el uso
			de un lenguaje controlado. </skos:definition>
<skos:example xml:lang="es">Ejemplos: "duplicado de", "madre de",
			"endoparásito de", "huésped de", "hermano de", "sinonimia válida de",
			"ubicado dentro de"</skos:example>
<skos:prefLabel xml:lang="zh-Hans">资源关系</skos:prefLabel>
<skos:definition xml:lang="zh-Hans">由相关资源编号确定的资源之间的关系。建议最佳做法是使用控制性词汇。</skos:definition>
<skos:example xml:lang="zh-Hans"/>
<skos:prefLabel xml:lang="ja"/>
<skos:definition xml:lang="ja">relatedResourceIDで特定される資料と、対象との関係性（resourceIDによる特定も可）。管理された語彙の使用を推奨。</skos:definition>
<skos:example xml:lang="ja"/>
<skos:inScheme rdf:resource="http://rs.gbif.org/terms/dwc/dwc_translations.rdf"/>
<rdf:type rdf:resource="http://www.w3.org/1999/02/22-rdf-syntax-ns#Property"/>
</skos:Concept>
<skos:Concept rdf:about="http://rs.tdwg.org/dwc/terms/relationshipRemarks">
<skos:prefLabel xml:lang="en">Relationship Remarks</skos:prefLabel>
<skos:definition xml:lang="en">Comments or notes about the
			relationship between the two resources.</skos:definition>
<skos:example xml:lang="en">Examples: "mother
			and offspring collected
			from the same nest", "pollinator captured in
			the act"</skos:example>
<skos:prefLabel xml:lang="es">Comentarios de la relación</skos:prefLabel>
<skos:definition xml:lang="es">Comentarios o anotaciones sobre la
			relación entre los dos recursos. </skos:definition>
<skos:example xml:lang="es">Ejemplos: "madre y cría colectadas del mismo
			nido" "polinizador capturado en el acto"</skos:example>
<skos:prefLabel xml:lang="zh-Hans">关系备注</skos:prefLabel>
<skos:definition xml:lang="zh-Hans">关于两种资源关系的评论或注释。</skos:definition>
<skos:example xml:lang="zh-Hans"/>
<skos:prefLabel xml:lang="ja"/>
<skos:definition xml:lang="ja">２つの資料間の関係性についてのコメントまたは注釈。</skos:definition>
<skos:example xml:lang="ja"/>
<skos:inScheme rdf:resource="http://rs.gbif.org/terms/dwc/dwc_translations.rdf"/>
<rdf:type rdf:resource="http://www.w3.org/1999/02/22-rdf-syntax-ns#Property"/>
</skos:Concept>
<skos:Concept rdf:about="http://rs.tdwg.org/dwc/terms/reproductiveCondition">
<skos:prefLabel xml:lang="en">Reproductive Condition</skos:prefLabel>
<skos:definition xml:lang="en">The reproductive condition of the
			biological individual(s) represented in the Occurrence. Recommended
			best practice is to use a controlled vocabulary.</skos:definition>
<skos:example xml:lang="en">Examples"
			"non-reproductive", "pregnant", "in
			bloom", "fruit-bearing"
		</skos:example>
<skos:prefLabel xml:lang="es">Condición reproductiva</skos:prefLabel>
<skos:definition xml:lang="es">La condición reproductiva del
			individuo(s) biológico s) representado en el Registro Biológico. La
			práctica recomendada es el uso de un lenguaje controlado. </skos:definition>
<skos:example xml:lang="es">Ejemplo: "no reproductiva", "en gestación",
			"floración", "fructificación"</skos:example>
<skos:prefLabel xml:lang="zh-Hans">繁殖状况</skos:prefLabel>
<skos:definition xml:lang="zh-Hans">生物个体在事件中表现的繁殖状况。建议最佳做法是使用一个控制性词汇。</skos:definition>
<skos:example xml:lang="zh-Hans"/>
<skos:prefLabel xml:lang="ja"/>
<skos:definition xml:lang="ja">その出来事を代表する生物個体の生殖条件。管理された語彙の使用を推奨。</skos:definition>
<skos:example xml:lang="ja"/>
<skos:inScheme rdf:resource="http://rs.gbif.org/terms/dwc/dwc_translations.rdf"/>
<rdf:type rdf:resource="http://www.w3.org/1999/02/22-rdf-syntax-ns#Property"/>
</skos:Concept>
<skos:Concept rdf:about="http://rs.tdwg.org/dwc/terms/resourceID">
<skos:prefLabel xml:lang="en">Resource ID</skos:prefLabel>
<skos:definition xml:lang="en">An identifier for the resource
			that is
			the subject of the relationship.</skos:definition>
<skos:example xml:lang="en"/>
<skos:prefLabel xml:lang="es">ID del recurso</skos:prefLabel>
<skos:definition xml:lang="es">Un identificador para el recurso que
			es el sujeto de la relación. </skos:definition>
<skos:example xml:lang="es"/>
<skos:prefLabel xml:lang="zh-Hans">资源编号</skos:prefLabel>
<skos:definition xml:lang="zh-Hans">表示关系主体的资源的标识符。</skos:definition>
<skos:example xml:lang="zh-Hans"/>
<skos:prefLabel xml:lang="ja"/>
<skos:definition xml:lang="ja">関係性の主語となる資源のID。</skos:definition>
<skos:example xml:lang="ja"/>
<skos:inScheme rdf:resource="http://rs.gbif.org/terms/dwc/dwc_translations.rdf"/>
<rdf:type rdf:resource="http://www.w3.org/1999/02/22-rdf-syntax-ns#Property"/>
</skos:Concept>
<skos:Concept rdf:about="http://rs.tdwg.org/dwc/terms/resourceRelationshipID">
<skos:prefLabel xml:lang="en">Resource Relationship ID</skos:prefLabel>
<skos:definition xml:lang="en">An identifier for an instance of
			relationship between one resource (the subject) and another
			(relatedResource, the object).</skos:definition>
<skos:example xml:lang="en"/>
<skos:prefLabel xml:lang="es">ID de la relación del recurso</skos:prefLabel>
<skos:definition xml:lang="es">Un identificador para una instancia de
			relación entre un recurso (el sujeto) y otro (Recurso Relacionado, el
			objeto). </skos:definition>
<skos:example xml:lang="es"/>
<skos:prefLabel xml:lang="zh-Hans">资源关系编号</skos:prefLabel>
<skos:definition xml:lang="zh-Hans">一个资源（主体）和另一个资源（相关的资源，客体）之间的关系实例标识符。</skos:definition>
<skos:example xml:lang="zh-Hans"/>
<skos:prefLabel xml:lang="ja"/>
<skos:definition xml:lang="ja">ある資料（主語）と他の資料（relatedResource,
			目的語）の間の関係性の例のID。</skos:definition>
<skos:example xml:lang="ja"/>
<skos:inScheme rdf:resource="http://rs.gbif.org/terms/dwc/dwc_translations.rdf"/>
<rdf:type rdf:resource="http://www.w3.org/1999/02/22-rdf-syntax-ns#Property"/>
</skos:Concept>
<skos:Concept rdf:about="http://rs.tdwg.org/dwc/terms/samplingEffort">
<skos:prefLabel xml:lang="en">Sampling Effort</skos:prefLabel>
<skos:definition xml:lang="en">The amount of effort expended
			during an
			Event.</skos:definition>
<skos:example xml:lang="en">Example: "40
			trap-nights", "10
			observer-hours; 10 km by foot; 30 km by car"
		</skos:example>
<skos:prefLabel xml:lang="es">Esfuerzo de muestreo</skos:prefLabel>
<skos:definition xml:lang="es">La cantidad de esfuerzo realizado
			durante un evento. </skos:definition>
<skos:example xml:lang="es">Ejemplo: "40 noches de trampeo", "10 horas
			de observador; 10 km caminando; 30 km en carro"</skos:example>
<skos:prefLabel xml:lang="zh-Hans">取样工作</skos:prefLabel>
<skos:definition xml:lang="zh-Hans">在事件中耗费的工作总量。</skos:definition>
<skos:example xml:lang="zh-Hans"/>
<skos:prefLabel xml:lang="ja"/>
<skos:definition xml:lang="ja">イベントの間に費やされた労力の量。</skos:definition>
<skos:example xml:lang="ja"/>
<skos:inScheme rdf:resource="http://rs.gbif.org/terms/dwc/dwc_translations.rdf"/>
<rdf:type rdf:resource="http://www.w3.org/1999/02/22-rdf-syntax-ns#Property"/>
</skos:Concept>
<skos:Concept rdf:about="http://rs.tdwg.org/dwc/terms/samplingProtocol">
<skos:prefLabel xml:lang="en">Sampling Protocol</skos:prefLabel>
<skos:definition xml:lang="en">The name of, reference to, or
			description of the method or protocol used during an Event.
		</skos:definition>
<skos:example xml:lang="en">Examples: "UV light
			trap", "mist net",
			"bottom trawl", "ad hoc observation", "point
			count", "Penguins from
			space: faecal stains reveal the location of
			emperor penguin colonies,
			http://dx.doi.org/10.1111/j.1466-8238.2009.00467.x", "Takats et al.
			2001. Guidelines for Nocturnal Owl Monitoring in North America.
			Beaverhill Bird Observatory and Bird Studies Canada, Edmonton,
			Alberta. 32 pp.", "http://www.bsc-eoc.org/download/Owl.pdf"
		</skos:example>
<skos:prefLabel xml:lang="es">Protocolo de muestreo</skos:prefLabel>
<skos:definition xml:lang="es">El nombre de, la referencia a, o la
			descripción del método o protocolo que se utiliza durante un evento. </skos:definition>
<skos:example xml:lang="es">Ejemplo: "trampa UV", "red de niebla",
			"observación ad hoc", "punto de conteo", "Penguins from space: faecal
			stains reveal the location of emperor penguin colonies,
			http://dx.doi.org/10.1111/j.1466-8238.2009.00467.x", "Takats et al.
			2001. Guidelines for Nocturnal Owl Monitoring in North America.
			Beaverhill Bird Observatory and Bird Studies Canada, Edmonton,
			Alberta. 32 pp.", "http://www.bsc-eoc.org/download/Owl.pdf"</skos:example>
<skos:prefLabel xml:lang="zh-Hans">取样草案</skos:prefLabel>
<skos:definition xml:lang="zh-Hans">事件中使用的方法或草案的名称，参考或者描述。</skos:definition>
<skos:example xml:lang="zh-Hans"/>
<skos:prefLabel xml:lang="ja"/>
<skos:definition xml:lang="ja">イベントの間に用いられた手法や手順の名前、参照、または記述。</skos:definition>
<skos:example xml:lang="ja"/>
<skos:inScheme rdf:resource="http://rs.gbif.org/terms/dwc/dwc_translations.rdf"/>
<rdf:type rdf:resource="http://www.w3.org/1999/02/22-rdf-syntax-ns#Property"/>
</skos:Concept>
<skos:Concept rdf:about="http://rs.tdwg.org/dwc/terms/scientificName">
<skos:prefLabel xml:lang="en">Scientific Name</skos:prefLabel>
<skos:definition xml:lang="en">The full scientific name, with
			authorship and date information if known. When forming part of an
			Identification, this should be the name in lowest level taxonomic
			rank that can be determined. This term should not contain
			identification qualifications, which should instead be supplied in
			the IdentificationQualifier term.</skos:definition>
<skos:example xml:lang="en">Examples:
			"Coleoptera" (order),
			"Vespertilionidae" (family), "Manis" (genus),
			"Ctenomys sociabilis"
			(genus + specificEpithet), "Ambystoma tigrinum
			diaboli" (genus +
			specificEpithet + infraspecificEpithet),
			"Roptrocerus typographi
			(Györfi, 1952)" (genus + specificEpithet +
			scientificNameAuthorship),
			"Quercus agrifolia var. oxyadenia (Torr.)
			J.T. Howell" (genus +
			specificEpithet + taxonRank +
			infraspecificEpithet +
			scientificNameAuthorship)
		</skos:example>
<skos:prefLabel xml:lang="es">Nombre científico</skos:prefLabel>
<skos:definition xml:lang="es">El nombre científico completo, con
			información de autoría y fecha si se conoce. Al formar parte de una
			identificación, este debe ser el nombre en el nivel taxonómico de
			menor nivel que pueda ser determinado. Este elemento no debe contener
			requisitos de identificación, estos deberían ser suministrados en el
			elemento Calificador Identificación. </skos:definition>
<skos:example xml:lang="es">Ejemplo: "Coleoptera" (Orden),
			"Vespertilionidae" (Familia), "Manis" (Género), "Ctenomys sociabilis"
			(Género + Epíteto Específico), "Ambystoma tigrinum diaboli" (Género +
			Epíteto Específico + Epíteto Infraespecífico), "Roptrocerus
			typographi (Györfi, 1952)" (Género + Epíteto Específico + Autoría
			Nombre Científico), "Quercus agrifolia var. oxyadenia (Torr.) J.T.
			Howell" (Género + Epíteto Específico + Nivel Taxón + Epíteto
			Infraspecífico + Autoría Nombre Científico)</skos:example>
<skos:prefLabel xml:lang="zh-Hans">学名</skos:prefLabel>
<skos:definition xml:lang="zh-Hans">完整学名（如果知道的话，包含作者和日期信息）。当形成部分的个体身份时，学名应该是可以被确定的最低分类等级的名称。这个名称不应该包含个体身份资格，身份资格应该在“鉴定合格者”中提供。</skos:definition>
<skos:example xml:lang="zh-Hans"/>
<skos:prefLabel xml:lang="ja"/>
<skos:definition xml:lang="ja">わかるのであれば著者と日付付きの、完全なる学名。系統の同定の際には、最も下位の階層の系統名を付けるべきである。このタームにはIdentificationQualifierに対応する情報を記載すべきではない。</skos:definition>
<skos:example xml:lang="ja"/>
<skos:inScheme rdf:resource="http://rs.gbif.org/terms/dwc/dwc_translations.rdf"/>
<rdf:type rdf:resource="http://www.w3.org/1999/02/22-rdf-syntax-ns#Property"/>
</skos:Concept>
<skos:Concept rdf:about="http://rs.tdwg.org/dwc/terms/scientificNameAuthorship">
<skos:prefLabel xml:lang="en">Scientific Name Authorship
		</skos:prefLabel>
<skos:definition xml:lang="en">The authorship information for the
			scientificName formatted according to the conventions of the
			applicable nomenclaturalCode.</skos:definition>
<skos:example xml:lang="en">Example: "(Torr.)
			J.T. Howell",
			"(Martinovský) Tzvelev", "(Györfi, 1952)"
		</skos:example>
<skos:prefLabel xml:lang="es">Autoría del nombre científico</skos:prefLabel>
<skos:definition xml:lang="es">La información de autoría del Nombre
			Científico formateado de acuerdo a las convenciones del Código
			Nomenclatural aplicable. </skos:definition>
<skos:example xml:lang="es">Ejemplo: "(Torr.) J.T. Howell",
			"(Martinovský) Tzvelev", "(Györfi, 1952)"</skos:example>
<skos:prefLabel xml:lang="zh-Hans">学名作者</skos:prefLabel>
<skos:definition xml:lang="zh-Hans">学名的作者信息，以命名准则适用的协定作为格式。</skos:definition>
<skos:example xml:lang="zh-Hans"/>
<skos:prefLabel xml:lang="ja"/>
<skos:definition xml:lang="ja">適用されたnomenclaturalCodeの慣例にしたがってフォーマットされた学名の、著者情報。</skos:definition>
<skos:example xml:lang="ja"/>
<skos:inScheme rdf:resource="http://rs.gbif.org/terms/dwc/dwc_translations.rdf"/>
<rdf:type rdf:resource="http://www.w3.org/1999/02/22-rdf-syntax-ns#Property"/>
</skos:Concept>
<skos:Concept rdf:about="http://rs.tdwg.org/dwc/terms/scientificNameID">
<skos:prefLabel xml:lang="en">Scientific Name ID</skos:prefLabel>
<skos:definition xml:lang="en">An identifier for the
			nomenclatural
			(not taxonomic) details of a scientific name.
		</skos:definition>
<skos:example xml:lang="en">Example:
			"urn:lsid:ipni.org:names:37829-1:1.3"</skos:example>
<skos:prefLabel xml:lang="es">ID del nombre científico</skos:prefLabel>
<skos:definition xml:lang="es">Un identificador de los detalles de la
			nomenclatura (no taxonómica) de un nombre científico. </skos:definition>
<skos:example xml:lang="es">Ejemplo:
			"urn:lsid:ipni.org:names:37829-1:1.3"</skos:example>
<skos:prefLabel xml:lang="zh-Hans">学名编号</skos:prefLabel>
<skos:definition xml:lang="zh-Hans">关于学名的系统命名（不是分类学）细节的标识符。</skos:definition>
<skos:example xml:lang="zh-Hans"/>
<skos:prefLabel xml:lang="ja"/>
<skos:definition xml:lang="ja">学名について、命名規則に関する（分類上の問題ではない）詳細についてのID。</skos:definition>
<skos:example xml:lang="ja"/>
<skos:inScheme rdf:resource="http://rs.gbif.org/terms/dwc/dwc_translations.rdf"/>
<rdf:type rdf:resource="http://www.w3.org/1999/02/22-rdf-syntax-ns#Property"/>
</skos:Concept>
<skos:Concept rdf:about="http://rs.tdwg.org/dwc/terms/sex">
<skos:prefLabel xml:lang="en">Sex</skos:prefLabel>
<skos:definition xml:lang="en">The sex of the biological
			individual(s) represented in the Occurrence. Recommended best
			practice is to use a controlled vocabulary.</skos:definition>
<skos:example xml:lang="en">Examples: "female",
			"hermaphrodite", "8
			males, 4 females"</skos:example>
<skos:prefLabel xml:lang="es">Sexo</skos:prefLabel>
<skos:definition xml:lang="es">El sexo del individuo(s) biológico(s)
			representado en el Registro Biológico. La práctica recomendada es el
			uso de un lenguaje controlado. </skos:definition>
<skos:example xml:lang="es">Ejemplo: "hembra", "hermafrodita", "8
			machos, 4 hembras"</skos:example>
<skos:prefLabel xml:lang="zh-Hans">性别</skos:prefLabel>
<skos:definition xml:lang="zh-Hans">事件中生物个体所表现的性别。建议最佳做法是使用一个控制性词汇。</skos:definition>
<skos:example xml:lang="zh-Hans"/>
<skos:prefLabel xml:lang="ja"/>
<skos:definition xml:lang="ja">その出来事を代表する生物個体の性別。管理された語彙の使用を推奨。</skos:definition>
<skos:example xml:lang="ja"/>
<skos:inScheme rdf:resource="http://rs.gbif.org/terms/dwc/dwc_translations.rdf"/>
<rdf:type rdf:resource="http://www.w3.org/1999/02/22-rdf-syntax-ns#Property"/>
</skos:Concept>
<skos:Concept rdf:about="http://rs.tdwg.org/dwc/terms/specificEpithet">
<skos:prefLabel xml:lang="en">Specific Epithet</skos:prefLabel>
<skos:definition xml:lang="en">The name of the first or species
			epithet of the scientificName.</skos:definition>
<skos:example xml:lang="en">Example: "concolor",
			"gottschei"</skos:example>
<skos:prefLabel xml:lang="es">Epíteto específico</skos:prefLabel>
<skos:definition xml:lang="es">El nombre del epíteto específico de
			Nombre Científico. </skos:definition>
<skos:example xml:lang="es">Ejemplo: "concolor", "gottschei"</skos:example>
<skos:prefLabel xml:lang="zh-Hans">具体别名</skos:prefLabel>
<skos:definition xml:lang="zh-Hans">学名的第一个名字或物种别名。</skos:definition>
<skos:example xml:lang="zh-Hans"/>
<skos:prefLabel xml:lang="ja"/>
<skos:definition xml:lang="ja">種名（種の形容辞）。</skos:definition>
<skos:example xml:lang="ja"/>
<skos:inScheme rdf:resource="http://rs.gbif.org/terms/dwc/dwc_translations.rdf"/>
<rdf:type rdf:resource="http://www.w3.org/1999/02/22-rdf-syntax-ns#Property"/>
</skos:Concept>
<skos:Concept rdf:about="http://rs.tdwg.org/dwc/terms/startDayOfYear">
<skos:prefLabel xml:lang="en">Start Day Of Year</skos:prefLabel>
<skos:definition xml:lang="en">The earliest ordinal day of the
			year on
			which the Event occurred (1 for January 1, 365 for December
			31, except
			in a leap year, in which case it is 366).</skos:definition>
<skos:example xml:lang="en">Examples: "1" (=1
			Jan), "366" (=31 Dec),
			"365" (=30 Dec in a leap year, 31 Dec in a
			non-leap year)</skos:example>
<skos:prefLabel xml:lang="es">Día inicial del año</skos:prefLabel>
<skos:definition xml:lang="es">El primer día ordinal del año en que
			ocurrió el evento (1 para el 1º de enero, 365 para el 31 de
			diciembre, excepto en un año bisiesto, en cuyo caso es 366). </skos:definition>
<skos:example xml:lang="es">Ejemplo: "1" (=1 ene), "366" (=31 dic),
			"365" (=30 dic en año bisiesto, 31 dic en un año no bisiesto)</skos:example>
<skos:prefLabel xml:lang="zh-Hans">一年中的开始日</skos:prefLabel>
<skos:definition xml:lang="zh-Hans">事件发生年的最早天数（1代表1月1日，365代表12月31日，除非在闰年中366代表12月31日）。</skos:definition>
<skos:example xml:lang="zh-Hans"/>
<skos:prefLabel xml:lang="ja"/>
<skos:definition xml:lang="ja">イベントが生じた年の最も早い日付（1月1日は1、12月31日は365とする。ただし、閏年以外。閏年の場合は12月31日が366となる）</skos:definition>
<skos:example xml:lang="ja"/>
<skos:inScheme rdf:resource="http://rs.gbif.org/terms/dwc/dwc_translations.rdf"/>
<rdf:type rdf:resource="http://www.w3.org/1999/02/22-rdf-syntax-ns#Property"/>
</skos:Concept>
<skos:Concept rdf:about="http://rs.tdwg.org/dwc/terms/stateProvince">
<skos:prefLabel xml:lang="en">State Province</skos:prefLabel>
<skos:definition xml:lang="en">The name of the next smaller
			administrative region than country (state, province, canton,
			department, region, etc.) in which the Location occurs.
		</skos:definition>
<skos:example xml:lang="en">Examples: "Montana",
			"Minas Gerais",
			"Córdoba"</skos:example>
<skos:prefLabel xml:lang="es">Estado provincia</skos:prefLabel>
<skos:definition xml:lang="es">El nombre de la siguiente región
			administrativa de menor jerarquía que País (estado, provincia,
			cantón, departamento, región, etc.) de la ubicación. </skos:definition>
<skos:example xml:lang="es">Ejemplo: "Montana", "Minas Gerais",
			"Córdoba"</skos:example>
<skos:prefLabel xml:lang="zh-Hans">州/省</skos:prefLabel>
<skos:definition xml:lang="zh-Hans">事件发生地的州/省名称，与国家（州，省，部，地区等）相比下一较小的行政区域。</skos:definition>
<skos:example xml:lang="zh-Hans"/>
<skos:prefLabel xml:lang="ja"/>
<skos:definition xml:lang="ja">その位置が存在する、国の下位の行政区分（州、県、小郡、省、区など）の名前。</skos:definition>
<skos:example xml:lang="ja"/>
<skos:inScheme rdf:resource="http://rs.gbif.org/terms/dwc/dwc_translations.rdf"/>
<rdf:type rdf:resource="http://www.w3.org/1999/02/22-rdf-syntax-ns#Property"/>
</skos:Concept>
<skos:Concept rdf:about="http://rs.tdwg.org/dwc/terms/subgenus">
<skos:prefLabel xml:lang="en">Subgenus</skos:prefLabel>
<skos:definition xml:lang="en">The full scientific name of the
			subgenus in which the taxon is classified. Values should include the
			genus to avoid homonym confusion.</skos:definition>
<skos:example xml:lang="en">Example: "Strobus
			(Pinus)", "Puma (Puma)"
			"Loligo (Amerigo)", "Hieracium subgen.
			Pilosella"</skos:example>
<skos:prefLabel xml:lang="es">Subgénero</skos:prefLabel>
<skos:definition xml:lang="es">El nombre científico completo del
			subgénero en el que se clasifica el taxón. Los valores deben incluir
			el género para evitar la confusión de homonimia. </skos:definition>
<skos:example xml:lang="es">Ejemplo: "Strobus (Pinus)", "Puma (Puma)"
			"Loligo (Amerigo)", "Hieracium subgen. Pilosella"</skos:example>
<skos:prefLabel xml:lang="zh-Hans">亚属</skos:prefLabel>
<skos:definition xml:lang="zh-Hans">分类单元所属亚属的完整学名。值应该包含属以避免同音混淆。</skos:definition>
<skos:example xml:lang="zh-Hans"/>
<skos:prefLabel xml:lang="ja"/>
<skos:definition xml:lang="ja">その分類群が位置づけられている、亜属のフルネーム。同音異義語との混乱を避けるため、属名も記載しなくてはいけない。</skos:definition>
<skos:example xml:lang="ja"/>
<skos:inScheme rdf:resource="http://rs.gbif.org/terms/dwc/dwc_translations.rdf"/>
<rdf:type rdf:resource="http://www.w3.org/1999/02/22-rdf-syntax-ns#Property"/>
</skos:Concept>
<skos:Concept rdf:about="http://rs.tdwg.org/dwc/terms/taxonConceptID">
<skos:prefLabel xml:lang="en">Taxon Concept ID</skos:prefLabel>
<skos:definition xml:lang="en">An identifier for the taxonomic
			concept to which the record refers - not for the nomenclatural
			details of a taxon.</skos:definition>
<skos:example xml:lang="en">Example:
			"8fa58e08-08de-4ac1-b69c-1235340b7001"</skos:example>
<skos:prefLabel xml:lang="es">ID del concepto del taxón</skos:prefLabel>
<skos:definition xml:lang="es">Un identificador para el concepto
			taxonómico al que se refiere el registro, no para los detalles de
			nomenclatura de un taxón. </skos:definition>
<skos:example xml:lang="es">Ejemplo:
			"8fa58e08-08de-4ac1-b69c-1235340b7001"</skos:example>
<skos:prefLabel xml:lang="zh-Hans">类群概念编号</skos:prefLabel>
<skos:definition xml:lang="zh-Hans">涉及分类概念(而非类群命名细节)的记录标识符。</skos:definition>
<skos:example xml:lang="zh-Hans"/>
<skos:prefLabel xml:lang="ja"/>
<skos:definition xml:lang="ja">そのレコードが参照している分類概念（命名規則に関する詳細ではない）のID。</skos:definition>
<skos:example xml:lang="ja"/>
<skos:inScheme rdf:resource="http://rs.gbif.org/terms/dwc/dwc_translations.rdf"/>
<rdf:type rdf:resource="http://www.w3.org/1999/02/22-rdf-syntax-ns#Property"/>
</skos:Concept>
<skos:Concept rdf:about="http://rs.tdwg.org/dwc/terms/taxonID">
<skos:prefLabel xml:lang="en">Taxon ID</skos:prefLabel>
<skos:definition xml:lang="en">An identifier for the set of taxon
			information (data associated with the Taxon class). May be a global
			unique identifier or an identifier specific to the data set.
		</skos:definition>
<skos:example xml:lang="en">Examples:
			"8fa58e08-08de-4ac1-b69c-1235340b7001", "32567",
			"http://species.gbif.org/abies_alba_1753",
			"urn:lsid:gbif.org:usages:32567"</skos:example>
<skos:prefLabel xml:lang="es">ID del taxón</skos:prefLabel>
<skos:definition xml:lang="es">Un identificador para el conjunto de
			información del taxón (datos asociados a la clase del Taxón). Puede
			ser un identificador único global o un identificador específico para
			el conjunto de datos. </skos:definition>
<skos:example xml:lang="es">Ejemplo:
			"8fa58e08-08de-4ac1-b69c-1235340b7001", "32567",
			"http://species.gbif.org/abies_alba_1753",
			"urn:lsid:gbif.org:usages:32567"</skos:example>
<skos:prefLabel xml:lang="zh-Hans">类群编号</skos:prefLabel>
<skos:definition xml:lang="zh-Hans">类群信息集（与类群相关的数据）标识符。可能是一个全局唯一的标识符或者一个特定数据集的标识符。</skos:definition>
<skos:example xml:lang="zh-Hans"/>
<skos:prefLabel xml:lang="ja"/>
<skos:definition xml:lang="ja">分類情報（分類群の階層に関連するデータ）セットのID。GUIDまたは、そのデータセットに固有のID。</skos:definition>
<skos:example xml:lang="ja"/>
<skos:inScheme rdf:resource="http://rs.gbif.org/terms/dwc/dwc_translations.rdf"/>
<rdf:type rdf:resource="http://www.w3.org/1999/02/22-rdf-syntax-ns#Property"/>
</skos:Concept>
<skos:Concept rdf:about="http://rs.tdwg.org/dwc/terms/taxonomicStatus">
<skos:prefLabel xml:lang="en">Taxonomic Status</skos:prefLabel>
<skos:definition xml:lang="en">The status of the use of the
			scientificName as a label for a taxon. Requires taxonomic opinion to
			define the scope of a taxon. Rules of priority then are used to
			define the taxonomic status of the nomenclature contained in that
			scope, combined with the experts opinion. It must be linked to a
			specific taxonomic reference that defines the concept. Recommended
			best practice is to use a controlled vocabulary.</skos:definition>
<skos:example xml:lang="en">Example: "invalid",
			"misapplied", "homotypic
			synonym", "accepted"</skos:example>
<skos:prefLabel xml:lang="es">Estado taxonómico</skos:prefLabel>
<skos:definition xml:lang="es">El estado de la utilización de Nombre
			Científico como una etiqueta para un taxón. Requiere opinión
			taxonómica para definir el alcance de un taxón. Dado lo anterior, se
			utilizan reglas de prioridad para definir el estatus taxonómico de la
			nomenclatura contenida en ese enfoque, junto con la opinión de los
			expertos. Debe estar vinculado a una referencia sobre taxonomía
			específica que defina el concepto. La práctica recomendada es el uso
			de un lenguaje controlado. </skos:definition>
<skos:example xml:lang="es">Ejemplo: "inválido", "mal aplicado",
			"sinonimia homotípica", "aceptado"</skos:example>
<skos:prefLabel xml:lang="zh-Hans">分类状态</skos:prefLabel>
<skos:definition xml:lang="zh-Hans">作为类群标签的学名的使用情况。需要分类意见确定类群的范围。然后使用优先规则来定义包含在范围内的分类命名状态，同时参考专家意见。必须与定义概念的特定分类参考相联系。建议最佳做法是使用一个控制性词汇。</skos:definition>
<skos:example xml:lang="zh-Hans"/>
<skos:prefLabel xml:lang="ja"/>
<skos:definition xml:lang="ja">系統のラベルであるscientificNameについての使用状況。系統のスコープを定義するには系統的な意見が必要である。そのスコープについての命名規約取り決めの優先順位は専門家の意見を考慮して決定される。その概念を定義した系統に関する文献へのリンクを指定する必要がある。管理された語彙の使用を推奨。</skos:definition>
<skos:example xml:lang="ja"/>
<skos:inScheme rdf:resource="http://rs.gbif.org/terms/dwc/dwc_translations.rdf"/>
<rdf:type rdf:resource="http://www.w3.org/1999/02/22-rdf-syntax-ns#Property"/>
</skos:Concept>
<skos:Concept rdf:about="http://rs.tdwg.org/dwc/terms/taxonRank">
<skos:prefLabel xml:lang="en">Taxon Rank</skos:prefLabel>
<skos:definition xml:lang="en">The taxonomic rank of the most
			specific name in the scientificName. Recommended best practice is to
			use a controlled vocabulary.</skos:definition>
<skos:example xml:lang="en">Examples:
			"subspecies", "varietas", "forma",
			"species", "genus"
		</skos:example>
<skos:prefLabel xml:lang="es">Nivel del taxón</skos:prefLabel>
<skos:definition xml:lang="es">La clasificación taxonómica del nombre
			más específico en el Nombre Científico. La práctica recomendada es el
			uso de un lenguaje controlado. </skos:definition>
<skos:example xml:lang="es">Ejemplo: "subespecie", "varietas", "forma",
			"especie", "género"</skos:example>
<skos:prefLabel xml:lang="zh-Hans">类群排名</skos:prefLabel>
<skos:definition xml:lang="zh-Hans">学名中最具体名称的分类排名。建议最佳做法是使用一个控制性词汇。</skos:definition>
<skos:example xml:lang="zh-Hans"/>
<skos:prefLabel xml:lang="ja"/>
<skos:definition xml:lang="ja">学名における、最も特有な名前の分類階層。管理された語彙の使用を推奨。</skos:definition>
<skos:example xml:lang="ja"/>
<skos:inScheme rdf:resource="http://rs.gbif.org/terms/dwc/dwc_translations.rdf"/>
<rdf:type rdf:resource="http://www.w3.org/1999/02/22-rdf-syntax-ns#Property"/>
</skos:Concept>
<skos:Concept rdf:about="http://rs.tdwg.org/dwc/terms/taxonRemarks">
<skos:prefLabel xml:lang="en">Taxon Remarks</skos:prefLabel>
<skos:definition xml:lang="en">Comments or notes about the taxon
			or
			name.</skos:definition>
<skos:example xml:lang="en">Example: "this name
			is a misspelling in
			common use"</skos:example>
<skos:prefLabel xml:lang="es">Comentarios del taxón</skos:prefLabel>
<skos:definition xml:lang="es">Comentarios o anotaciones sobre el
			taxón o nombre. </skos:definition>
<skos:example xml:lang="es">Ejemplo: "este nombre está mal escrito en
			uso común"</skos:example>
<skos:prefLabel xml:lang="zh-Hans">类群备注</skos:prefLabel>
<skos:definition xml:lang="zh-Hans">关于类群或者名称的评论或注释。</skos:definition>
<skos:example xml:lang="zh-Hans"/>
<skos:prefLabel xml:lang="ja"/>
<skos:definition xml:lang="ja">分類や名前についてのコメントまたは注釈。</skos:definition>
<skos:example xml:lang="ja"/>
<skos:inScheme rdf:resource="http://rs.gbif.org/terms/dwc/dwc_translations.rdf"/>
<rdf:type rdf:resource="http://www.w3.org/1999/02/22-rdf-syntax-ns#Property"/>
</skos:Concept>
<skos:Concept rdf:about="http://rs.tdwg.org/dwc/terms/typeStatus">
<skos:prefLabel xml:lang="en">Type Status</skos:prefLabel>
<skos:definition xml:lang="en">A list (concatenated and
			separated) of
			nomenclatural types (type status, typified scientific
			name,
			publication) applied to the subject.</skos:definition>
<skos:example xml:lang="en">Example: "holotype
			of Ctenomys sociabilis.
			Pearson O. P., and M. I. Christie. 1985.
			Historia Natural, 5(37):388"</skos:example>
<skos:prefLabel xml:lang="es">Estado del tipo</skos:prefLabel>
<skos:definition xml:lang="es">Una lista (concatenada y separada) de
			los tipos de nomenclatura (estado del tipo, nombre científico
			tipificado, publicación) aplicados al sujeto. </skos:definition>
<skos:example xml:lang="es">Ejemplo: "holotipo de Ctenomys sociabilis.
			Pearson O. P., y M. I. Christie. 1985. Historia Natural, 5(37):388"</skos:example>
<skos:prefLabel xml:lang="zh-Hans">类型状态</skos:prefLabel>
<skos:definition xml:lang="zh-Hans">适用于主题的命名类型（状态类型，典型学名，出版物）列表(连接的或分开的)。</skos:definition>
<skos:example xml:lang="zh-Hans"/>
<skos:prefLabel xml:lang="ja"/>
<skos:definition xml:lang="ja">対象に適用された命名タイプ（タイプの状態、典型的な学名、出版物）のリスト。</skos:definition>
<skos:example xml:lang="ja"/>
<skos:inScheme rdf:resource="http://rs.gbif.org/terms/dwc/dwc_translations.rdf"/>
<rdf:type rdf:resource="http://www.w3.org/1999/02/22-rdf-syntax-ns#Property"/>
</skos:Concept>
<skos:Concept rdf:about="http://rs.tdwg.org/dwc/terms/verbatimCoordinates">
<skos:prefLabel xml:lang="en">Verbatim Coordinates</skos:prefLabel>
<skos:definition xml:lang="en">The verbatim original spatial
			coordinates of the Location. The coordinate ellipsoid, geodeticDatum,
			or full Spatial Reference System (SRS) for these coordinates should
			be stored in verbatimSRS and the coordinate system should be stored
			in verbatimCoordinateSystem.</skos:definition>
<skos:example xml:lang="en">Examples: "41 05 54S
			121 05 34W", "17T 630000
			4833400"</skos:example>
<skos:prefLabel xml:lang="es">Coordenadas originales</skos:prefLabel>
<skos:definition xml:lang="es">Las coordenadas espaciales originales
			textuales de la ubicación. El elipsoide de las coordenadas, Datum
			Geodésico, o el sistema de referencia espacial (SRS) completo para
			estas coordenadas se deben almacenar en SRS Original y el sistema de
			coordenadas debe ser almacenado en Sistema Coordenadas Original. </skos:definition>
<skos:example xml:lang="es">Ejemplo: "41 05 54S 121 05 34W", "17T 630000
			4833400"</skos:example>
<skos:prefLabel xml:lang="zh-Hans">逐字坐标</skos:prefLabel>
<skos:definition xml:lang="zh-Hans">逐字表示的地点的原始空间坐标。椭球坐标，大地基准，或这些坐标的完整空间参考系统（SRS）应该保存在“逐字空间参考系统”，坐标系统应该保存在“逐字坐标系统”。</skos:definition>
<skos:example xml:lang="zh-Hans"/>
<skos:prefLabel xml:lang="ja"/>
<skos:definition xml:lang="ja">場所に関する逐語的な空間座標。楕円体、経緯度原点、空間参照システムによる座標はverbatimSRSおよび座標システムはverbatimCoordinateSystemに保存されるべきである。</skos:definition>
<skos:example xml:lang="ja"/>
<skos:inScheme rdf:resource="http://rs.gbif.org/terms/dwc/dwc_translations.rdf"/>
<rdf:type rdf:resource="http://www.w3.org/1999/02/22-rdf-syntax-ns#Property"/>
</skos:Concept>
<skos:Concept rdf:about="http://rs.tdwg.org/dwc/terms/verbatimCoordinateSystem">
<skos:prefLabel xml:lang="en">Verbatim Coordinate System
		</skos:prefLabel>
<skos:definition xml:lang="en">The spatial coordinate system for
			the
			verbatimLatitude and verbatimLongitude or the verbatimCoordinates
			of
			the Location. Recommended best practice is to use a controlled
			vocabulary.</skos:definition>
<skos:example xml:lang="en">Examples: "decimal
			degrees", "degrees decimal
			minutes", "degrees minutes seconds", "UTM"
		</skos:example>
<skos:prefLabel xml:lang="es">Sistema original de coordenadas</skos:prefLabel>
<skos:definition xml:lang="es">El sistema de coordenadas espaciales
			para Latitud Original y Longitud Original o Coordenadas Originales de
			la ubicación. La práctica recomendada es el uso de un lenguaje
			controlado.  </skos:definition>
<skos:example xml:lang="es">Ejemplo: "grados decimales", "minutos grados
			decimales", "segundos grados decimales", "UTM"</skos:example>
<skos:prefLabel xml:lang="zh-Hans">逐字坐标系统</skos:prefLabel>
<skos:definition xml:lang="zh-Hans">逐字表示的地点的经纬度或坐标的空间坐标系统。建议最佳做法是使用一个控制性词汇。</skos:definition>
<skos:example xml:lang="zh-Hans"/>
<skos:prefLabel xml:lang="ja"/>
<skos:definition xml:lang="ja">その位置の、verbatimLatitudeおよびverbatimLongitude、またはverbatimCoordinatesのための空間座標系。管理された語彙の使用を推奨。</skos:definition>
<skos:example xml:lang="ja"/>
<skos:inScheme rdf:resource="http://rs.gbif.org/terms/dwc/dwc_translations.rdf"/>
<rdf:type rdf:resource="http://www.w3.org/1999/02/22-rdf-syntax-ns#Property"/>
</skos:Concept>
<skos:Concept rdf:about="http://rs.tdwg.org/dwc/terms/verbatimDepth">
<skos:prefLabel xml:lang="en">Verbatim Depth</skos:prefLabel>
<skos:definition xml:lang="en">The original description of the
			depth
			below the local surface.</skos:definition>
<skos:example xml:lang="en">Example: "100-200 m"
		</skos:example>
<skos:prefLabel xml:lang="es">Profundidad original</skos:prefLabel>
<skos:definition xml:lang="es">La descripción original de la
			profundidad bajo la superficie local. </skos:definition>
<skos:example xml:lang="es">Ejemplo: "100-200 m"</skos:example>
<skos:prefLabel xml:lang="zh-Hans">逐字深度</skos:prefLabel>
<skos:definition xml:lang="zh-Hans">地表以下深度的原始描述。</skos:definition>
<skos:example xml:lang="zh-Hans"/>
<skos:prefLabel xml:lang="ja"/>
<skos:definition xml:lang="ja">地表下の深度の大元の記載。</skos:definition>
<skos:example xml:lang="ja"/>
<skos:inScheme rdf:resource="http://rs.gbif.org/terms/dwc/dwc_translations.rdf"/>
<rdf:type rdf:resource="http://www.w3.org/1999/02/22-rdf-syntax-ns#Property"/>
</skos:Concept>
<skos:Concept rdf:about="http://rs.tdwg.org/dwc/terms/verbatimElevation">
<skos:prefLabel xml:lang="en">Verbatim Elevation</skos:prefLabel>
<skos:definition xml:lang="en">The original description of the
			elevation (altitude, usually above sea level) of the Location.
		</skos:definition>
<skos:example xml:lang="en">Example: "100-200 m"
		</skos:example>
<skos:prefLabel xml:lang="es">Elevación original</skos:prefLabel>
<skos:definition xml:lang="es">La descripción original de la
			elevación (altitud, por lo general por encima del nivel del mar) de
			la Ubicación. </skos:definition>
<skos:example xml:lang="es">Ejemplo: "100-200 m"</skos:example>
<skos:prefLabel xml:lang="zh-Hans">逐字海拔</skos:prefLabel>
<skos:definition xml:lang="zh-Hans">海拔（通常是海平面以上的高度）位置的原始描述。</skos:definition>
<skos:example xml:lang="zh-Hans"/>
<skos:prefLabel xml:lang="ja"/>
<skos:definition xml:lang="ja">その位置の標高（高度、大抵の場合は海抜）の大元の記載。</skos:definition>
<skos:example xml:lang="ja"/>
<skos:inScheme rdf:resource="http://rs.gbif.org/terms/dwc/dwc_translations.rdf"/>
<rdf:type rdf:resource="http://www.w3.org/1999/02/22-rdf-syntax-ns#Property"/>
</skos:Concept>
<skos:Concept rdf:about="http://rs.tdwg.org/dwc/terms/verbatimEventDate">
<skos:prefLabel xml:lang="en">Verbatim EventDate</skos:prefLabel>
<skos:definition xml:lang="en">The verbatim original
			representation of
			the date and time information for an Event.
		</skos:definition>
<skos:example xml:lang="en">Examples: "spring
			1910", "Marzo 2002",
			"1999-03-XX", "17IV1934"</skos:example>
<skos:prefLabel xml:lang="es">Fecha original del evento </skos:prefLabel>
<skos:definition xml:lang="es">La representación textual original de
			la información de fecha y tiempo para un evento. </skos:definition>
<skos:example xml:lang="es">Ejemplo: "primavera 1910", "marzo 2002",
			"1999-03-XX", "17IV1934"</skos:example>
<skos:prefLabel xml:lang="zh-Hans">逐字事件日期</skos:prefLabel>
<skos:definition xml:lang="zh-Hans">一次事件的日期时间信息的逐字原始表示。</skos:definition>
<skos:example xml:lang="zh-Hans"/>
<skos:prefLabel xml:lang="ja"/>
<skos:definition xml:lang="ja">あるイベントの日時に関する逐語的な表現。</skos:definition>
<skos:example xml:lang="ja"/>
<skos:inScheme rdf:resource="http://rs.gbif.org/terms/dwc/dwc_translations.rdf"/>
<rdf:type rdf:resource="http://www.w3.org/1999/02/22-rdf-syntax-ns#Property"/>
</skos:Concept>
<skos:Concept rdf:about="http://rs.tdwg.org/dwc/terms/verbatimLatitude">
<skos:prefLabel xml:lang="en">Verbatim Latitude</skos:prefLabel>
<skos:definition xml:lang="en">The verbatim original latitude of
			the
			Location. The coordinate ellipsoid, geodeticDatum, or full
			Spatial
			Reference System (SRS) for these coordinates should be stored
			in
			verbatimSRS and the coordinate system should be stored in
			verbatimCoordinateSystem.</skos:definition>
<skos:example xml:lang="en">Example: "41 05
			54.03S"</skos:example>
<skos:prefLabel xml:lang="es">Latitud original</skos:prefLabel>
<skos:definition xml:lang="es">La latitud original textual de la
			ubicación. El elipsoide de coordenadas, el Datum geodésico o el
			Sistema de Referencia Espacial completo (SRS) para estas coordenadas
			debería ser almacenado en SRS Original y el sistema de coordenadas
			debería ser almacenado en Sistema Original de Coordenadas. </skos:definition>
<skos:example xml:lang="es">Ejemplo: "41 05 56.03S"</skos:example>
<skos:prefLabel xml:lang="zh-Hans">逐字纬度</skos:prefLabel>
<skos:definition xml:lang="zh-Hans">逐字表示的地点的原始纬度。椭球坐标，大地基准，或者这些坐标完整的空间参考系统（SRS）应该存放在“逐字空间参考系统”，坐标系统应该存放在“逐字坐标系统”。</skos:definition>
<skos:example xml:lang="zh-Hans"/>
<skos:prefLabel xml:lang="ja"/>
<skos:definition xml:lang="ja">場所に関する逐語的な緯度。楕円体、経緯度原点、空間参照システムによる座標はverbatimSRSおよび座標システムはverbatimCoordinateSystemに保存されるべきである。</skos:definition>
<skos:example xml:lang="ja"/>
<skos:inScheme rdf:resource="http://rs.gbif.org/terms/dwc/dwc_translations.rdf"/>
<rdf:type rdf:resource="http://www.w3.org/1999/02/22-rdf-syntax-ns#Property"/>
</skos:Concept>
<skos:Concept rdf:about="http://rs.tdwg.org/dwc/terms/verbatimLocality">
<skos:prefLabel xml:lang="en">Verbatim Locality</skos:prefLabel>
<skos:definition xml:lang="en">The original textual description
			of the
			place.</skos:definition>
<skos:example xml:lang="en">Example: "25 km NNE
			Bariloche por R. Nac.
			237"</skos:example>
<skos:prefLabel xml:lang="es">Localidad original</skos:prefLabel>
<skos:definition xml:lang="es">La descripción textual original del
			lugar. </skos:definition>
<skos:example xml:lang="es">Ejemplo: "25 km NNE Bariloche por R.
			Nac.237"</skos:example>
<skos:prefLabel xml:lang="zh-Hans">逐字方位</skos:prefLabel>
<skos:definition xml:lang="zh-Hans">地点的原始文本描述。</skos:definition>
<skos:example xml:lang="zh-Hans"/>
<skos:prefLabel xml:lang="ja"/>
<skos:definition xml:lang="ja">その場所の、文章による記述。</skos:definition>
<skos:example xml:lang="ja"/>
<skos:inScheme rdf:resource="http://rs.gbif.org/terms/dwc/dwc_translations.rdf"/>
<rdf:type rdf:resource="http://www.w3.org/1999/02/22-rdf-syntax-ns#Property"/>
</skos:Concept>
<skos:Concept rdf:about="http://rs.tdwg.org/dwc/terms/verbatimLongitude">
<skos:prefLabel xml:lang="en">Verbatim Longitude</skos:prefLabel>
<skos:definition xml:lang="en">The verbatim original longitude of
			the
			Location. The coordinate ellipsoid, geodeticDatum, or full
			Spatial
			Reference System (SRS) for these coordinates should be stored
			in
			verbatimSRS and the coordinate system should be stored in
			verbatimCoordinateSystem.</skos:definition>
<skos:example xml:lang="en">Example: "121d 10'
			34" W"</skos:example>
<skos:prefLabel xml:lang="es">Longitud original</skos:prefLabel>
<skos:definition xml:lang="es">La longitud original textual de la
			Ubicación. El elipsoide de coordinadas, Datum Geodésico o el Sistema
			de Referencia Espacial completo (SRS) para estas coordenadas debería
			ser almacenado en SRS Original y el sistema de coordenadas debería
			ser almacenado en Sistema Original de Coordenadas. </skos:definition>
<skos:example xml:lang="es">Ejemplo: "121d 10' 34" W"</skos:example>
<skos:prefLabel xml:lang="zh-Hans">逐字经度</skos:prefLabel>
<skos:definition xml:lang="zh-Hans">逐字表述的地点的原始经度。椭球坐标，大地基准，或者这些坐标完整的空间参考系统（SRS）应该存放在“逐字空间参考系统”，坐标系统应该存放在“逐字坐标系统”。</skos:definition>
<skos:example xml:lang="zh-Hans"/>
<skos:prefLabel xml:lang="ja"/>
<skos:definition xml:lang="ja">場所に関する逐語的な経度。楕円体、経緯度原点、空間参照システムによる座標はverbatimSRSおよび座標システムはverbatimCoordinateSystemに保存されるべきである。</skos:definition>
<skos:example xml:lang="ja"/>
<skos:inScheme rdf:resource="http://rs.gbif.org/terms/dwc/dwc_translations.rdf"/>
<rdf:type rdf:resource="http://www.w3.org/1999/02/22-rdf-syntax-ns#Property"/>
</skos:Concept>
<skos:Concept rdf:about="http://rs.tdwg.org/dwc/terms/verbatimSRS">
<skos:prefLabel xml:lang="en">Verbatim SRS</skos:prefLabel>
<skos:definition xml:lang="en">The ellipsoid, geodetic datum, or
			spatial reference system (SRS) upon which coordinates given in
			verbatimLatitude and verbatimLongitude, or verbatimCoordinates are
			based. Recommended best practice is use the EPSG code as a controlled
			vocabulary to provide an SRS, if known. Otherwise use a controlled
			vocabulary for the name or code of the geodetic datum, if known.
			Otherwise use a controlled vocabulary for the name or code of the
			ellipsoid, if known. If none of these is known, use the value
			"unknown".</skos:definition>
<skos:example xml:lang="en">Examples:
			"EPSG:4326", "WGS84", "NAD27",
			"Campo Inchauspe", "European 1950",
			"Clarke 1866"</skos:example>
<skos:prefLabel xml:lang="es">SRS original</skos:prefLabel>
<skos:definition xml:lang="es">El elipsoide, datum geodésico, o
			sistema de referencia espacial (SRS) en el que se basan las
			coordenadas provistas en Latitud Original y Longitud Original o
			Coordenadas Originales. La práctica recomendada es usar el código
			EPSG como un lenguaje controlado para proporcionar un SRS, si se
			conoce. Caso contrario, utilice un lenguaje controlado para el nombre
			o código del datum geodésico, si se conoce. Caso contrario, utilice
			un lenguaje controlado para el nombre o código del elipsoide, si se
			conoce. Si nada de esto se sabe, utilice el valor "desconocido". </skos:definition>
<skos:example xml:lang="es">Ejemplo: "EPSG:4326", "WGS84", "NAD27",
			"Campo Inchauspe", "European 1950", "Clarke 1866"</skos:example>
<skos:prefLabel xml:lang="zh-Hans">逐字空间参考系统</skos:prefLabel>
<skos:definition xml:lang="zh-Hans">椭圆体、大地基准点或空间参考系统的地理坐标以逐字表示的经度和纬度为基础。建议最佳做法是如果已知EPSG编码，使用其作为控制性词汇规定一个空间参考系统。或者使用已知的控制性词汇作为大地基准点的名称或编码。或者使用已知的控制性词汇作为椭圆体的名称或编码。如果这些都未知，则使用“未知”值。</skos:definition>
<skos:example xml:lang="zh-Hans"/>
<skos:prefLabel xml:lang="ja"/>
<skos:definition xml:lang="ja">verbatimLatitudeとverbatimLongitude、verbatimCoordinatesで与えられる地理座標についての楕円体、経緯度原点、空間参照システム。もしわかるのであれば、空間参照システムから提供されるEPSGコードなどの管理された語彙の使用が推奨される。そうでない場合は、経緯度原点の名前またはコードについての管理された語彙の使用が推奨される。それも困難であれば、楕円体についての名前またはコードについての管理された語彙の使用が推奨される。それも無理の場合は、"unknown"を使用する。</skos:definition>
<skos:example xml:lang="ja"/>
<skos:inScheme rdf:resource="http://rs.gbif.org/terms/dwc/dwc_translations.rdf"/>
<rdf:type rdf:resource="http://www.w3.org/1999/02/22-rdf-syntax-ns#Property"/>
</skos:Concept>
<skos:Concept rdf:about="http://rs.tdwg.org/dwc/terms/verbatimTaxonRank">
<skos:prefLabel xml:lang="en">Verbatim Taxon Rank</skos:prefLabel>
<skos:definition xml:lang="en">The taxonomic rank of the most
			specific name in the scientificName as it appears in the original
			record.</skos:definition>
<skos:example xml:lang="en">Examples:
			"Agamospecies", "sub-lesus",
			"prole", "apomict", "nothogrex", "sp.",
			"subsp.", "var."</skos:example>
<skos:prefLabel xml:lang="es">Nivel original del taxón</skos:prefLabel>
<skos:definition xml:lang="es">El nivel taxonómico del nombre más
			específico en un nombre científico tal y como aparece en el registro
			original. </skos:definition>
<skos:example xml:lang="es">Ejemplos: "Agamospecies", "sub-lesus",
			"prole", "apomict", "nothogrex", "sp.", "subsp.", "var."</skos:example>
<skos:prefLabel xml:lang="zh-Hans">逐字分类排名</skos:prefLabel>
<skos:definition xml:lang="zh-Hans">出现在原始记录中的最具体学名的分类排名。</skos:definition>
<skos:example xml:lang="zh-Hans"/>
<skos:prefLabel xml:lang="ja"/>
<skos:definition xml:lang="ja">学名における、最も特有な名前の分類階層（大元の記載に現れているもの）。</skos:definition>
<skos:example xml:lang="ja"/>
<skos:inScheme rdf:resource="http://rs.gbif.org/terms/dwc/dwc_translations.rdf"/>
<rdf:type rdf:resource="http://www.w3.org/1999/02/22-rdf-syntax-ns#Property"/>
</skos:Concept>
<skos:Concept rdf:about="http://rs.tdwg.org/dwc/terms/vernacularName">
<skos:prefLabel xml:lang="en">Vernacular Name</skos:prefLabel>
<skos:definition xml:lang="en">A common or vernacular name.
		</skos:definition>
<skos:example xml:lang="en">Example: "Andean
			Condor", "Condor Andino",
			"American Eagle", "Gänsegeier"
		</skos:example>
<skos:prefLabel xml:lang="es">Nombre común</skos:prefLabel>
<skos:definition xml:lang="es">Un nombre común o vernacular.</skos:definition>
<skos:example xml:lang="es">Ejemplo: "Cóndor Andino", "Águila
			Americana", "Buitre"</skos:example>
<skos:prefLabel xml:lang="zh-Hans">俗名</skos:prefLabel>
<skos:definition xml:lang="zh-Hans">一个常见或者俗名。</skos:definition>
<skos:example xml:lang="zh-Hans"/>
<skos:prefLabel xml:lang="ja"/>
<skos:definition xml:lang="ja">一般名、あるいは通俗名。</skos:definition>
<skos:example xml:lang="ja"/>
<skos:inScheme rdf:resource="http://rs.gbif.org/terms/dwc/dwc_translations.rdf"/>
<rdf:type rdf:resource="http://www.w3.org/1999/02/22-rdf-syntax-ns#Property"/>
</skos:Concept>
<skos:Concept rdf:about="http://rs.tdwg.org/dwc/terms/waterBody">
<skos:prefLabel xml:lang="en">Water Body</skos:prefLabel>
<skos:definition xml:lang="en">The name of the water body in
			which the
			Location occurs. Recommended best practice is to use a
			controlled
			vocabulary such as the Getty Thesaurus of Geographic
			Names.</skos:definition>
<skos:example xml:lang="en">Example: "Indian
			Ocean", "Baltic Sea"</skos:example>
<skos:prefLabel xml:lang="es">Cuerpo de agua</skos:prefLabel>
<skos:definition xml:lang="es">El nombre del cuerpo de agua en que la
			Ubicación ocurre. Una práctica recomendada es utilizar un vocabulario
			controlado tal como el Tesauro Getty de Nombres Geográficos. </skos:definition>
<skos:example xml:lang="es">Ejemplo: "Océano Índico", "Mar Báltico"</skos:example>
<skos:prefLabel xml:lang="zh-Hans">水体</skos:prefLabel>
<skos:definition xml:lang="zh-Hans">发生地点的水体名称。建议最佳做法是使用一个控制性词汇，如地名盖蒂词库。</skos:definition>
<skos:example xml:lang="zh-Hans"/>
<skos:prefLabel xml:lang="ja"/>
<skos:definition xml:lang="ja">その位置の水塊の名前。 the Getty Thesaurus of
			Geographic Names など、管理された語彙の使用を推奨。</skos:definition>
<skos:example xml:lang="ja"/>
<skos:inScheme rdf:resource="http://rs.gbif.org/terms/dwc/dwc_translations.rdf"/>
<rdf:type rdf:resource="http://www.w3.org/1999/02/22-rdf-syntax-ns#Property"/>
</skos:Concept>
<skos:Concept rdf:about="http://rs.tdwg.org/dwc/terms/year">
<skos:prefLabel xml:lang="en">Year</skos:prefLabel>
<skos:definition xml:lang="en">The four-digit year in which the
			Event
			occurred, according to the Common Era Calendar.</skos:definition>
<skos:example xml:lang="en">Example: "2008"
		</skos:example>
<skos:prefLabel xml:lang="es">Año</skos:prefLabel>
<skos:definition xml:lang="es">Los cuatro dígitos del año en que el
			Evento ocurrió, de acuerdo al Calendario de la Era Común. </skos:definition>
<skos:example xml:lang="es">Ejemplo: "2008"</skos:example>
<skos:prefLabel xml:lang="zh-Hans">年份</skos:prefLabel>
<skos:definition xml:lang="zh-Hans">事件发生的四位公历年份（根据公共纪元日历）。</skos:definition>
<skos:example xml:lang="zh-Hans"/>
<skos:prefLabel xml:lang="ja"/>
<skos:definition xml:lang="ja">イベントが発生した西暦。</skos:definition>
<skos:example xml:lang="ja"/>
<skos:inScheme rdf:resource="http://rs.gbif.org/terms/dwc/dwc_translations.rdf"/>
<rdf:type rdf:resource="http://www.w3.org/1999/02/22-rdf-syntax-ns#Property"/>
</skos:Concept>
</rdf:RDF>
